Adding the proved example about unknot equivalence along with incorporating suggested changes about redundancies

Tangles.thy
@@ -26,11 +26,11 @@ lemma symmetry3: assumes "symp R" shows "symp R^**" using assms symmetry1 symmet
 
 
 (*each  block is a horizontal block built by putting basic tangle bricks next to each other.
-(1) e_vert is the straight line
-(2) e_cup is the up facing cusp
-(3) e_cap is the bottom facing cusp
-(4) e_over is the positive cross
-(5) e_under is the negative cross*)
+(1) (cement vert) is the straight line
+(2) (cement cup) is the up facing cusp
+(3) (cement cap) is the bottom facing cusp
+(4) (cement over) is the positive cross
+(5) (cement under) is the negative cross*)
 
 datatype brick = vert
                 |cup
@@ -48,14 +48,14 @@ where
 "length (cement x) = 1"|
 "length (cons x y) = 1 + (length y)"
 
+(*
 
-
-definition e_vert::block where "e_vert \<equiv> (cement vert)"
-definition e_cup::block where "e_cup \<equiv> (cement cup)"
-definition e_cap::block where "e_cap \<equiv> (cement cap)"
-definition e_over::block where "e_over \<equiv> (cement over)"
-definition e_under::block where "e_under \<equiv> (cement under)"
-
+definition (cement vert)::block where "(cement vert) \<equiv> (cement vert)"
+definition (cement cup)::block where "(cement cup) \<equiv> (cement cup)"
+definition (cement cap)::block where "(cement cap) \<equiv> (cement cap)"
+definition (cement over)::block where "(cement over) \<equiv> (cement over)"
+definition (cement under)::block where "(cement under) \<equiv> (cement under)"
+*)
 
 (*count tells us the number of incoming and outgoing strangs of each block*)
 
@@ -73,21 +73,21 @@ where
 "count (cement x) = (brickcount x)"
 |"count (cons x y) = (fst (brickcount x) + fst (count y), snd (brickcount x) + snd (count y))"
 
-lemma e_vert_count:" count (e_vert) = (1,1)"
-using e_vert_def brickcount.simps(1) count.simps(1) by metis
+lemma cement_vert_count:" count (cement vert) = (1,1)"
+using brickcount.simps(1) count.simps(1) by metis
 
-lemma e_cup_count:" count (e_cup) = (0,2)"
-using e_cup_def brickcount.simps(2) count.simps(1) by metis
+lemma cement_cup_count:" count ((cement cup)) = (0,2)"
+using brickcount.simps(2) count.simps(1) by metis
 
 
-lemma e_cap_count:" count (e_cap) = (2,0)"
-using e_cap_def brickcount.simps(3) count.simps(1) by metis
+lemma cement_cap_count:" count ((cement cap)) = (2,0)"
+using  brickcount.simps(3) count.simps(1) by metis
 
-lemma e_over_count:" count (e_over) = (2,2)"
-using e_over_def brickcount.simps(4) count.simps(1) by metis
+lemma cement_over_count:" count ((cement over)) = (2,2)"
+using brickcount.simps(4) count.simps(1) by metis
 
-lemma e_under_count:" count (e_under) = (2,2)"
-using e_under_def brickcount.simps(5) count.simps(1) by metis
+lemma cement_under_count:" count ((cement under)) = (2,2)"
+using  brickcount.simps(5) count.simps(1) by metis
 
 
 
@@ -186,8 +186,8 @@ by (metis (hide_lams, no_types) add_nonneg_eq_0_iff assms le_neq_trans snd_count
 snd_count_nonnegative)
 
 
-lemma trivial: "(count (vert # e_cup)) = (1,3)"
-apply (simp add: e_cup_def)
+lemma trivial: "(count (vert # (cement cup))) = (1,3)"
+apply (simp)
 done
 
 (*cusp is defined*)
@@ -208,8 +208,8 @@ where
 
 
 lemma cusp_basic: "((cusp x) = False) \<Longrightarrow> 
-((x=e_vert)\<or>(x=e_cap)\<or>(x=e_over)\<or>(x=e_under))\<or>(\<exists>y1.\<exists>y2.\<exists>y3.(x=(y1\<otimes>y2\<otimes>y3)\<and> 
-((y1=e_vert)\<or>(y1=e_cap)\<or>(y1=e_over)\<or>(y1=e_under))\<or>(y2=e_vert)\<or>(y2=e_cap)\<or>(y2=e_over)\<or>(y2=e_under))\<or>((y3=e_vert)\<or>(y3=e_cap)\<or>(y3=e_over)\<or>(y3=e_under)))"
+((x=(cement vert))\<or>(x=(cement cap))\<or>(x=(cement over))\<or>(x=(cement under)))\<or>(\<exists>y1.\<exists>y2.\<exists>y3.(x=(y1\<otimes>y2\<otimes>y3)\<and> 
+((y1=(cement vert))\<or>(y1=(cement cap))\<or>(y1=(cement over))\<or>(y1=(cement under)))\<or>(y2=(cement vert))\<or>(y2=(cement cap))\<or>(y2=(cement over))\<or>(y2=(cement under)))\<or>((y3=(cement vert))\<or>(y3=(cement cap))\<or>(y3=(cement over))\<or>(y3=(cement under))))"
 by metis
 
 
@@ -261,7 +261,7 @@ qed
 
 primrec makestrand:: "nat \<Rightarrow> block"
 where
-"makestrand 0 = e_vert"
+"makestrand 0 = (cement vert)"
 |"makestrand (Suc n) = vert#(makestrand n)"
 
 (*walls are tangle diagrams obtained by placing a horizontal blocks a top each other*)
@@ -330,17 +330,17 @@ done
 
 (*test exercises*)
 
-lemma trivial2: "wall_list (basic e_vert) = []"
+lemma trivial2: "wall_list (basic (cement vert)) = []"
 apply(auto)
 done
 
 
-lemma trivial3: "fst(wall_count (basic e_cap))- snd(wall_count (basic e_vert)) = 1"
-apply(simp add:e_cap_def e_vert_def)
+lemma trivial3: "fst(wall_count (basic (cement cap)))- snd(wall_count (basic (cement vert))) = 1"
+apply(simp)
 done
 
-lemma trivial4: "wall_list ((basic e_cap)\<circ>(basic e_vert)\<circ>(basic e_vert)) = [1,0]"
-apply(simp add: e_cap_def e_vert_def)
+lemma trivial4: "wall_list ((basic (cement cap))\<circ>(basic (cement vert))\<circ>(basic (cement vert))) = [1,0]"
+apply(simp)
 apply(simp add:abs_def)
 done
 
@@ -364,9 +364,9 @@ definition well_defined::"walls \<Rightarrow> bool" where
 + abs(snd(wall_count x)))) = 0)"
 
 typedef diagram = "{(x::walls). well_defined x}"
-apply (rule_tac x = "prod e_cup (basic e_cap)" in exI)
+apply (rule_tac x = "prod (cement cup) (basic (cement cap))" in exI)
 apply(auto)
-apply(simp add:abs_def e_cup_def e_cap_def well_defined_def)
+apply(simp add:abs_def well_defined_def)
 done
 
 (*well_defined properties*)
@@ -542,36 +542,36 @@ of which is defined as a disjunction of many functions.*)
 definition tanglerel_uncross_positiveflip::"diagram \<Rightarrow> diagram \<Rightarrow> bool"
 where
 "tanglerel_uncross_positiveflip x y \<equiv> (\<exists>y1.\<exists>z1.\<exists>z2.\<exists>z3.\<exists>w1.\<exists>w2.\<exists>w3.\<exists>y2.(x = Abs_diagram ((y1)
-\<circ>(basic (z1\<otimes>e_vert\<otimes>e_cup\<otimes>w1)\<circ>(basic (z2\<otimes>e_over\<otimes>e_vert\<otimes>w2))\<circ>(basic (z3\<otimes>e_vert\<otimes>e_cap\<otimes>w3))\<circ>(y2))))\<and>(y = Abs_diagram
+\<circ>(basic (z1\<otimes>(cement vert)\<otimes>(cement cup)\<otimes>w1)\<circ>(basic (z2\<otimes>(cement over)\<otimes>(cement vert)\<otimes>w2))\<circ>(basic (z3\<otimes>(cement vert)\<otimes>(cement cap)\<otimes>w3))\<circ>(y2))))\<and>(y = Abs_diagram
  ((y1)
-\<circ>(basic (z1\<otimes>e_cup\<otimes>e_vert\<otimes>w1))\<circ>(basic (z2\<otimes>e_vert\<otimes>e_over\<otimes>w2))\<circ>(basic (z3\<otimes>e_cap\<otimes>e_vert\<otimes>w3))\<circ>(y2)))\<and>((snd (count z1)) = 
+\<circ>(basic (z1\<otimes>(cement cup)\<otimes>(cement vert)\<otimes>w1))\<circ>(basic (z2\<otimes>(cement vert)\<otimes>(cement over)\<otimes>w2))\<circ>(basic (z3\<otimes>(cement cap)\<otimes>(cement vert)\<otimes>w3))\<circ>(y2)))\<and>((snd (count z1)) = 
 (fst (count z2)))\<and>((snd (count z2)) = (fst (count z3))) \<and> ((snd (count w1)) = (fst
 (count w2)))\<and>((snd (count w2)) = (fst (count w3))))"
 
 definition tanglerel_uncross_positivestraighten::"diagram \<Rightarrow> diagram \<Rightarrow> bool"
 where
 "tanglerel_uncross_positivestraighten x y \<equiv> (\<exists>y1.\<exists>z1.\<exists>z2.\<exists>z3.\<exists>w1.\<exists>w2.\<exists>w3.\<exists>y2.(x = Abs_diagram ((y1)
-\<circ>(basic (z1\<otimes>e_cup\<otimes>e_vert\<otimes>w1)\<circ>(basic (z2\<otimes>e_vert\<otimes>e_over\<otimes>w2))\<circ>(basic (z3\<otimes>e_cap\<otimes>e_vert\<otimes>w3))\<circ>(y2))))\<and>(y = Abs_diagram
+\<circ>(basic (z1\<otimes>(cement cup)\<otimes>(cement vert)\<otimes>w1)\<circ>(basic (z2\<otimes>(cement vert)\<otimes>(cement over)\<otimes>w2))\<circ>(basic (z3\<otimes>(cement cap)\<otimes>(cement vert)\<otimes>w3))\<circ>(y2))))\<and>(y = Abs_diagram
  ((y1)
-\<circ>(basic (z1\<otimes>e_vert\<otimes>w1))\<circ>(basic (z2\<otimes>e_vert\<otimes>w2))\<circ>(basic (z3\<otimes>e_vert\<otimes>w3))\<circ>(y2)))\<and>((snd (count z1)) = 
+\<circ>(basic (z1\<otimes>(cement vert)\<otimes>w1))\<circ>(basic (z2\<otimes>(cement vert)\<otimes>w2))\<circ>(basic (z3\<otimes>(cement vert)\<otimes>w3))\<circ>(y2)))\<and>((snd (count z1)) = 
 (fst (count z2)))\<and>((snd (count z2)) = (fst (count z3))) \<and> ((snd (count w1)) = (fst
 (count w2)))\<and>((snd (count w2)) = (fst (count w3))))"
 
 definition tanglerel_uncross_negativeflip::"diagram \<Rightarrow> diagram \<Rightarrow> bool"
 where
 "tanglerel_uncross_negativeflip x y \<equiv> (\<exists>y1.\<exists>z1.\<exists>z2.\<exists>z3.\<exists>w1.\<exists>w2.\<exists>w3.\<exists>y2.(x = Abs_diagram ((y1)
-\<circ>(basic (z1\<otimes>e_vert\<otimes>e_cup\<otimes>w1)\<circ>(basic (z2\<otimes>e_under\<otimes>e_vert\<otimes>w2))\<circ>(basic (z3\<otimes>e_vert\<otimes>e_cap\<otimes>w3))\<circ>(y2))))\<and>(y = Abs_diagram
+\<circ>(basic (z1\<otimes>(cement vert)\<otimes>(cement cup)\<otimes>w1)\<circ>(basic (z2\<otimes>(cement under)\<otimes>(cement vert)\<otimes>w2))\<circ>(basic (z3\<otimes>(cement vert)\<otimes>(cement cap)\<otimes>w3))\<circ>(y2))))\<and>(y = Abs_diagram
  ((y1)
-\<circ>(basic (z1\<otimes>e_cup\<otimes>e_vert\<otimes>w1))\<circ>(basic (z2\<otimes>e_vert\<otimes>e_under\<otimes>w2))\<circ>(basic (z3\<otimes>e_cap\<otimes>e_vert\<otimes>w3))\<circ>(y2)))\<and>((snd (count z1)) = 
+\<circ>(basic (z1\<otimes>(cement cup)\<otimes>(cement vert)\<otimes>w1))\<circ>(basic (z2\<otimes>(cement vert)\<otimes>(cement under)\<otimes>w2))\<circ>(basic (z3\<otimes>(cement cap)\<otimes>(cement vert)\<otimes>w3))\<circ>(y2)))\<and>((snd (count z1)) = 
 (fst (count z2)))\<and>((snd (count z2)) = (fst (count z3))) \<and> ((snd (count w1)) = (fst
 (count w2)))\<and>((snd (count w2)) = (fst (count w3))))"
 
 definition tanglerel_uncross_negativestraighten::"diagram \<Rightarrow> diagram \<Rightarrow> bool"
 where
 "tanglerel_uncross_negativestraighten x y \<equiv> (\<exists>y1.\<exists>z1.\<exists>z2.\<exists>z3.\<exists>w1.\<exists>w2.\<exists>w3.\<exists>y2.(x = Abs_diagram ((y1)
-\<circ>(basic (z1\<otimes>e_cup\<otimes>e_vert\<otimes>w1)\<circ>(basic (z2\<otimes>e_vert\<otimes>e_under\<otimes>w2))\<circ>(basic (z3\<otimes>e_cap\<otimes>e_vert\<otimes>w3))\<circ>(y2))))\<and>(y = Abs_diagram
+\<circ>(basic (z1\<otimes>(cement cup)\<otimes>(cement vert)\<otimes>w1)\<circ>(basic (z2\<otimes>(cement vert)\<otimes>(cement under)\<otimes>w2))\<circ>(basic (z3\<otimes>(cement cap)\<otimes>(cement vert)\<otimes>w3))\<circ>(y2))))\<and>(y = Abs_diagram
  ((y1)
-\<circ>(basic (z1\<otimes>e_vert\<otimes>w1))\<circ>(basic (z2\<otimes>e_vert\<otimes>w2))\<circ>(basic (z3\<otimes>e_vert\<otimes>w3))\<circ>(y2)))\<and>((snd (count z1)) = 
+\<circ>(basic (z1\<otimes>(cement vert)\<otimes>w1))\<circ>(basic (z2\<otimes>(cement vert)\<otimes>w2))\<circ>(basic (z3\<otimes>(cement vert)\<otimes>w3))\<circ>(y2)))\<and>((snd (count z1)) = 
 (fst (count z2)))\<and>((snd (count z2)) = (fst (count z3))) \<and> ((snd (count w1)) = (fst
 (count w2)))\<and>((snd (count w2)) = (fst (count w3))))"
 
@@ -599,18 +599,18 @@ done
 definition tanglerel_pull_posneg::"diagram \<Rightarrow> diagram \<Rightarrow> bool"
 where
 "tanglerel_pull_posneg x y \<equiv>  \<exists>y1.\<exists>z1.\<exists>z2.\<exists>w1.\<exists>w2.\<exists>y2.((x = Abs_diagram ((y1)
-\<circ>(basic (z1\<otimes>e_over\<otimes>w1)\<circ>(basic (z2\<otimes>e_under\<otimes>w2)))\<circ>(y2)))\<and>(y = Abs_diagram
+\<circ>(basic (z1\<otimes>(cement over)\<otimes>w1)\<circ>(basic (z2\<otimes>(cement under)\<otimes>w2)))\<circ>(y2)))\<and>(y = Abs_diagram
  ((y1)
-\<circ>(basic (z1\<otimes>e_vert\<otimes>e_vert\<otimes>w1))\<circ>(basic (z2\<otimes>e_vert\<otimes>e_vert\<otimes>w2))\<circ>(y2)))
+\<circ>(basic (z1\<otimes>(cement vert)\<otimes>(cement vert)\<otimes>w1))\<circ>(basic (z2\<otimes>(cement vert)\<otimes>(cement vert)\<otimes>w2))\<circ>(y2)))
 \<and>((snd (count z1)) = (fst (count z2))))"
 
 
 definition tanglerel_pull_negpos::"diagram \<Rightarrow> diagram \<Rightarrow> bool"
 where
 "tanglerel_pull_negpos x y \<equiv>  \<exists>y1.\<exists>z1.\<exists>z2.\<exists>w1.\<exists>w2.\<exists>y2.((x = Abs_diagram ((y1)
-\<circ>(basic (z1\<otimes>e_under\<otimes>w1)\<circ>(basic (z2\<otimes>e_over\<otimes>w2)))\<circ>(y2)))\<and>(y = Abs_diagram
+\<circ>(basic (z1\<otimes>(cement under)\<otimes>w1)\<circ>(basic (z2\<otimes>(cement over)\<otimes>w2)))\<circ>(y2)))\<and>(y = Abs_diagram
  ((y1)
-\<circ>(basic (z1\<otimes>e_vert\<otimes>e_vert\<otimes>w1))\<circ>(basic (z2\<otimes>e_vert\<otimes>e_vert\<otimes>w2))\<circ>(y2)))
+\<circ>(basic (z1\<otimes>(cement vert)\<otimes>(cement vert)\<otimes>w1))\<circ>(basic (z2\<otimes>(cement vert)\<otimes>(cement vert)\<otimes>w2))\<circ>(y2)))
 \<and>((snd (count z1)) = (fst (count z2))))"
 
 (*tanglerel_pull definition*)
@@ -624,36 +624,36 @@ where
 definition tanglerel_straighten_topdown::"diagram \<Rightarrow> diagram \<Rightarrow> bool"
 where
 "tanglerel_straighten_topdown x y \<equiv>  \<exists>y1.\<exists>z1.\<exists>z2.\<exists>w1.\<exists>w2.\<exists>y2.((x = Abs_diagram ((y1)
-\<circ>(basic (z1\<otimes>e_vert\<otimes>e_cup\<otimes>w1)\<circ>(basic (z2\<otimes>e_cap\<otimes>e_vert\<otimes>w2)))\<circ>(y2)))\<and>(y = Abs_diagram
+\<circ>(basic (z1\<otimes>(cement vert)\<otimes>(cement cup)\<otimes>w1)\<circ>(basic (z2\<otimes>(cement cap)\<otimes>(cement vert)\<otimes>w2)))\<circ>(y2)))\<and>(y = Abs_diagram
  ((y1)
-\<circ>(basic (z1\<otimes>e_vert\<otimes>w1))\<circ>(basic (z2\<otimes>e_vert\<otimes>w2))\<circ>(y2)))
+\<circ>(basic (z1\<otimes>(cement vert)\<otimes>w1))\<circ>(basic (z2\<otimes>(cement vert)\<otimes>w2))\<circ>(y2)))
 \<and>((snd (count z1)) = (fst (count z2))))"
 
 
 definition tanglerel_straighten_downtop::"diagram \<Rightarrow> diagram \<Rightarrow> bool"
 where
 "tanglerel_straighten_downtop x y \<equiv>  \<exists>y1.\<exists>z1.\<exists>z2.\<exists>w1.\<exists>w2.\<exists>y2.((x = Abs_diagram ((y1)
-\<circ>(basic (z1\<otimes>e_cup\<otimes>e_vert\<otimes>w1)\<circ>(basic (z2\<otimes>e_vert\<otimes>e_cap\<otimes>w2)))\<circ>(y2)))\<and>(y = Abs_diagram
+\<circ>(basic (z1\<otimes>(cement cup)\<otimes>(cement vert)\<otimes>w1)\<circ>(basic (z2\<otimes>(cement vert)\<otimes>(cement cap)\<otimes>w2)))\<circ>(y2)))\<and>(y = Abs_diagram
  ((y1)
-\<circ>(basic (z1\<otimes>e_vert\<otimes>w1))\<circ>(basic (z2\<otimes>e_vert\<otimes>w2))\<circ>(y2)))
+\<circ>(basic (z1\<otimes>(cement vert)\<otimes>w1))\<circ>(basic (z2\<otimes>(cement vert)\<otimes>w2))\<circ>(y2)))
 \<and>((snd (count z1)) = (fst (count z2))))"
 
 
 definition tanglerel_straighten_righttopdown::"diagram \<Rightarrow> diagram \<Rightarrow> bool"
 where
 "tanglerel_straighten_righttopdown x y \<equiv>  \<exists>y1.\<exists>w1.\<exists>w2.\<exists>y2.((x = Abs_diagram ((y1)
-\<circ>(basic (e_vert\<otimes>e_cup\<otimes>w1)\<circ>(basic (e_cap\<otimes>e_vert\<otimes>w2)))\<circ>(y2)))\<and>(y = Abs_diagram
+\<circ>(basic ((cement vert)\<otimes>(cement cup)\<otimes>w1)\<circ>(basic ((cement cap)\<otimes>(cement vert)\<otimes>w2)))\<circ>(y2)))\<and>(y = Abs_diagram
  ((y1)
-\<circ>(basic (e_vert\<otimes>w1))\<circ>(basic (e_vert\<otimes>w2))\<circ>(y2))))
+\<circ>(basic ((cement vert)\<otimes>w1))\<circ>(basic ((cement vert)\<otimes>w2))\<circ>(y2))))
  \<and> ((snd (count w1)) = (fst (count w2)))"
 
 
 definition tanglerel_straighten_rightdowntop::"diagram \<Rightarrow> diagram \<Rightarrow> bool"
 where
 "tanglerel_straighten_rightdowntop x y \<equiv>  \<exists>y1.\<exists>w1.\<exists>w2.\<exists>y2.((x = Abs_diagram ((y1)
-\<circ>(basic (e_cup\<otimes>e_vert\<otimes>w1)\<circ>(basic (e_vert\<otimes>e_cap\<otimes>w2)))\<circ>(y2)))\<and>(y = Abs_diagram
+\<circ>(basic ((cement cup)\<otimes>(cement vert)\<otimes>w1)\<circ>(basic ((cement vert)\<otimes>(cement cap)\<otimes>w2)))\<circ>(y2)))\<and>(y = Abs_diagram
  ((y1)
-\<circ>(basic (e_vert\<otimes>w1))\<circ>(basic (e_vert\<otimes>w2))\<circ>(y2))))
+\<circ>(basic ((cement vert)\<otimes>w1))\<circ>(basic ((cement vert)\<otimes>w2))\<circ>(y2))))
  \<and> ((snd (count w1)) = (fst (count w2)))"
 
 
@@ -661,18 +661,18 @@ where
 definition tanglerel_straighten_lefttopdown::"diagram \<Rightarrow> diagram \<Rightarrow> bool"
 where
 "tanglerel_straighten_lefttopdown x y \<equiv>  \<exists>y1.\<exists>z1.\<exists>z2.\<exists>y2.((x = Abs_diagram ((y1)
-\<circ>(basic (z1\<otimes>e_cup\<otimes>e_vert)\<circ>(basic (z2\<otimes>e_vert\<otimes>e_cap)))\<circ>(y2)))\<and>(y = Abs_diagram
+\<circ>(basic (z1\<otimes>(cement cup)\<otimes>(cement vert))\<circ>(basic (z2\<otimes>(cement vert)\<otimes>(cement cap))))\<circ>(y2)))\<and>(y = Abs_diagram
  ((y1)
-\<circ>(basic (z1\<otimes>e_vert))\<circ>(basic (z2\<otimes>e_vert))\<circ>(y2)))
+\<circ>(basic (z1\<otimes>(cement vert)))\<circ>(basic (z2\<otimes>(cement vert)))\<circ>(y2)))
 \<and>((snd (count z1)) = (fst (count z2))))"
 
 
 definition tanglerel_straighten_leftdowntop::"diagram \<Rightarrow> diagram \<Rightarrow> bool"
 where
 "tanglerel_straighten_leftdowntop x y \<equiv>  \<exists>y1.\<exists>z1.\<exists>z2.\<exists>y2.((x = Abs_diagram ((y1)
-\<circ>(basic (z1\<otimes>e_vert\<otimes>e_cup)\<circ>(basic (z2\<otimes>e_cap\<otimes>e_vert)))\<circ>(y2)))\<and>(y = Abs_diagram
+\<circ>(basic (z1\<otimes>(cement vert)\<otimes>(cement cup))\<circ>(basic (z2\<otimes>(cement cap)\<otimes>(cement vert))))\<circ>(y2)))\<and>(y = Abs_diagram
  ((y1)
-\<circ>(basic (z1\<otimes>e_vert))\<circ>(basic (z2\<otimes>e_vert))\<circ>(y2))))
+\<circ>(basic (z1\<otimes>(cement vert)))\<circ>(basic (z2\<otimes>(cement vert)))\<circ>(y2))))
 \<and>((snd (count z1)) = (fst (count z2)))"
 
 (*definition straighten*)
@@ -689,18 +689,18 @@ where
 definition tanglerel_swing_pos::"diagram \<Rightarrow> diagram \<Rightarrow> bool"
 where
 "tanglerel_swing_pos x y \<equiv> \<exists>y1.\<exists>z1.\<exists>z2.\<exists>z3.\<exists>w1.\<exists>w2.\<exists>w3.\<exists>y2.((x = Abs_diagram ((y1)
-\<circ>(basic (z1\<otimes>e_over\<otimes>e_vert\<otimes>w1)\<circ>(basic (z2\<otimes>e_vert\<otimes>e_over\<otimes>w2))\<circ>(basic (z3\<otimes>e_over\<otimes>e_vert\<otimes>w3))\<circ>(y2))))\<and>(y = Abs_diagram
+\<circ>(basic (z1\<otimes>(cement over)\<otimes>(cement vert)\<otimes>w1)\<circ>(basic (z2\<otimes>(cement vert)\<otimes>(cement over)\<otimes>w2))\<circ>(basic (z3\<otimes>(cement over)\<otimes>(cement vert)\<otimes>w3))\<circ>(y2))))\<and>(y = Abs_diagram
  ((y1)
-\<circ>(basic (z1\<otimes>e_vert\<otimes>e_over\<otimes>w1)\<circ>(basic (z2\<otimes>e_over\<otimes>e_vert\<otimes>w2))\<circ>(basic (z3\<otimes>e_vert\<otimes>e_over\<otimes>w3))\<circ>(y2))))
+\<circ>(basic (z1\<otimes>(cement vert)\<otimes>(cement over)\<otimes>w1)\<circ>(basic (z2\<otimes>(cement over)\<otimes>(cement vert)\<otimes>w2))\<circ>(basic (z3\<otimes>(cement vert)\<otimes>(cement over)\<otimes>w3))\<circ>(y2))))
 \<and>((snd (count z1)) = (fst (count z2)))\<and>((snd (count z2)) = (fst (count z3)))
  \<and> ((snd (count w1)) = (fst (count w2)))\<and>((snd (count w2)) = (fst (count w3))))"
 
 definition tanglerel_swing_neg::"diagram \<Rightarrow> diagram \<Rightarrow> bool"
 where
 "tanglerel_swing_neg x y \<equiv> \<exists>y1.\<exists>z1.\<exists>z2.\<exists>z3.\<exists>w1.\<exists>w2.\<exists>w3.\<exists>y2.((x = Abs_diagram ((y1)
-\<circ>(basic (z1\<otimes>e_under\<otimes>e_vert\<otimes>w1)\<circ>(basic (z2\<otimes>e_vert\<otimes>e_under\<otimes>w2))\<circ>(basic (z3\<otimes>e_under\<otimes>e_vert\<otimes>w3))\<circ>(y2))))\<and>(y = Abs_diagram
+\<circ>(basic (z1\<otimes>(cement under)\<otimes>(cement vert)\<otimes>w1)\<circ>(basic (z2\<otimes>(cement vert)\<otimes>(cement under)\<otimes>w2))\<circ>(basic (z3\<otimes>(cement under)\<otimes>(cement vert)\<otimes>w3))\<circ>(y2))))\<and>(y = Abs_diagram
  ((y1)
-\<circ>(basic (z1\<otimes>e_vert\<otimes>e_under\<otimes>w1)\<circ>(basic (z2\<otimes>e_under\<otimes>e_vert\<otimes>w2))\<circ>(basic (z3\<otimes>e_vert\<otimes>e_under\<otimes>w3))\<circ>(y2)))))
+\<circ>(basic (z1\<otimes>(cement vert)\<otimes>(cement under)\<otimes>w1)\<circ>(basic (z2\<otimes>(cement under)\<otimes>(cement vert)\<otimes>w2))\<circ>(basic (z3\<otimes>(cement vert)\<otimes>(cement under)\<otimes>w3))\<circ>(y2)))))
 \<and>((snd (count z1)) = (fst (count z2)))\<and>((snd (count z2)) = (fst (count z3)))
  \<and> ((snd (count w1)) = (fst (count w2)))\<and>((snd (count w2)) = (fst (count w3)))"
 
@@ -717,8 +717,8 @@ definition tanglerel_rotate_toppos::"diagram \<Rightarrow> diagram \<Rightarrow>
 where
 "tanglerel_rotate_toppos x y \<equiv>  \<exists>y1.\<exists>z1.\<exists>z2.\<exists>w1.\<exists>w2.\<exists>y2.((x = Abs_diagram
  ((y1)
-\<circ>(basic (z1\<otimes>e_vert\<otimes>e_over\<otimes>w1))\<circ>(basic (z2\<otimes>e_cap\<otimes>e_vert\<otimes>w2))\<circ>(y2)))\<and> ((y = Abs_diagram ((y1)
-\<circ>(basic (z1\<otimes>e_under\<otimes>e_vert\<otimes>w1)\<circ>(basic (z2\<otimes>e_vert\<otimes>e_cap\<otimes>w2)))\<circ>(y2))))
+\<circ>(basic (z1\<otimes>(cement vert)\<otimes>(cement over)\<otimes>w1))\<circ>(basic (z2\<otimes>(cement cap)\<otimes>(cement vert)\<otimes>w2))\<circ>(y2)))\<and> ((y = Abs_diagram ((y1)
+\<circ>(basic (z1\<otimes>(cement under)\<otimes>(cement vert)\<otimes>w1)\<circ>(basic (z2\<otimes>(cement vert)\<otimes>(cement cap)\<otimes>w2)))\<circ>(y2))))
 \<and>((snd (count z1)) = (fst (count z2)))
 \<and>((snd (count w1)) = (fst (count w2))))"
 
@@ -727,8 +727,8 @@ definition tanglerel_rotate_topneg::"diagram \<Rightarrow> diagram \<Rightarrow>
 where
 "tanglerel_rotate_topneg x y \<equiv>  \<exists>y1.\<exists>z1.\<exists>z2.\<exists>w1.\<exists>w2.\<exists>y2.((x = Abs_diagram
  ((y1)
-\<circ>(basic (z1\<otimes>e_vert\<otimes>e_under\<otimes>w1))\<circ>(basic (z2\<otimes>e_cap\<otimes>e_vert\<otimes>w2))\<circ>(y2)))\<and> ((y = Abs_diagram ((y1)
-\<circ>(basic (z1\<otimes>e_over\<otimes>e_vert\<otimes>w1)\<circ>(basic (z2\<otimes>e_vert\<otimes>e_cap\<otimes>w2)))\<circ>(y2))))
+\<circ>(basic (z1\<otimes>(cement vert)\<otimes>(cement under)\<otimes>w1))\<circ>(basic (z2\<otimes>(cement cap)\<otimes>(cement vert)\<otimes>w2))\<circ>(y2)))\<and> ((y = Abs_diagram ((y1)
+\<circ>(basic (z1\<otimes>(cement over)\<otimes>(cement vert)\<otimes>w1)\<circ>(basic (z2\<otimes>(cement vert)\<otimes>(cement cap)\<otimes>w2)))\<circ>(y2))))
 \<and>((snd (count z1)) = (fst (count z2)))
 \<and>((snd (count w1)) = (fst (count w2))))"
 
@@ -736,8 +736,8 @@ definition tanglerel_rotate_downpos::"diagram \<Rightarrow> diagram \<Rightarrow
 where
 "tanglerel_rotate_downpos x y \<equiv>  \<exists>y1.\<exists>z1.\<exists>z2.\<exists>w1.\<exists>w2.\<exists>y2.((x = Abs_diagram
  ((y1)
-\<circ>(basic (z1\<otimes>e_cap\<otimes>e_vert\<otimes>w1))\<circ>(basic (z2\<otimes>e_vert\<otimes>e_over\<otimes>w2))\<circ>(y2)))\<and> ((y = Abs_diagram ((y1)
-\<circ>(basic (z1\<otimes>e_vert\<otimes>e_cap\<otimes>w1)\<circ>(basic (z2\<otimes>e_under\<otimes>e_vert\<otimes>w2)))\<circ>(y2))))
+\<circ>(basic (z1\<otimes>(cement cap)\<otimes>(cement vert)\<otimes>w1))\<circ>(basic (z2\<otimes>(cement vert)\<otimes>(cement over)\<otimes>w2))\<circ>(y2)))\<and> ((y = Abs_diagram ((y1)
+\<circ>(basic (z1\<otimes>(cement vert)\<otimes>(cement cap)\<otimes>w1)\<circ>(basic (z2\<otimes>(cement under)\<otimes>(cement vert)\<otimes>w2)))\<circ>(y2))))
 \<and>((snd (count z1)) = (fst (count z2)))
 \<and>((snd (count w1)) = (fst (count w2))))"
 
@@ -747,8 +747,8 @@ where
 "tanglerel_rotate_downneg x y \<equiv>  \<exists>y1.\<exists>z1.\<exists>z2.
 \<exists>w1.\<exists>w2.\<exists>y2.
 ((x = Abs_diagram ((y1)
-\<circ>(basic (z1\<otimes>e_cap\<otimes>e_vert\<otimes>w1))\<circ>(basic (z2\<otimes>e_vert\<otimes>e_under\<otimes>w2))\<circ>(y2)))\<and> ((y = Abs_diagram ((y1)
-\<circ>(basic (z1\<otimes>e_vert\<otimes>e_cap\<otimes>w1)\<circ>(basic (z2\<otimes>e_over\<otimes>e_vert\<otimes>w2)))\<circ>(y2))))
+\<circ>(basic (z1\<otimes>(cement cap)\<otimes>(cement vert)\<otimes>w1))\<circ>(basic (z2\<otimes>(cement vert)\<otimes>(cement under)\<otimes>w2))\<circ>(y2)))\<and> ((y = Abs_diagram ((y1)
+\<circ>(basic (z1\<otimes>(cement vert)\<otimes>(cement cap)\<otimes>w1)\<circ>(basic (z2\<otimes>(cement over)\<otimes>(cement vert)\<otimes>w2)))\<circ>(y2))))
 \<and>((snd (count z1)) = (fst (count z2)))
 \<and>((snd (count w1)) = (fst (count w2))))"
 
@@ -779,7 +779,7 @@ where
 "strands (x#ys) = (if (x= vert) then (strands ys) else False)"
 
 
-lemma strands_test: "strands (vert#cup#vert#e_vert) = False" using e_vert_def strands_def brickstrand_def
+lemma strands_test: "strands (vert#cup#vert#(cement vert)) = False" using strands_def brickstrand_def
 compose_def by auto
 
 (*Compress -  Compress has two levels of equivalences. It is a composition of Compress_null, compbelow
@@ -802,7 +802,7 @@ definition tanglerel_compbelow_right::"diagram \<Rightarrow> diagram \<Rightarro
 where
 "tanglerel_compbelow_right x y \<equiv>  \<exists>w1.\<exists>w2.\<exists>y2.\<exists>A.\<exists>B.((x= Abs_diagram
  ((basic (A\<otimes>w1))\<circ>(basic (B\<otimes>w2))\<circ>(y2)))\<and> (y = Abs_diagram (
-(basic w1)\<circ>(basic (B\<otimes>w2))\<circ>(y2)))
+(basic w1)\<circ>(basic (A\<otimes>w2))\<circ>(y2)))
 \<and>((snd (count w1)) = (fst (count w2)))
 \<and> (strands B)
 \<and> ((fst (count A)) = 0))"
@@ -832,7 +832,7 @@ where
 "tanglerel_compbelow_bottomleft x y \<equiv>  \<exists>z2.\<exists>A.\<exists>B.\<exists>y2.((x = Abs_diagram
  ((basic (A))\<circ>(basic (z2\<otimes>B))\<circ>(y2)))\<and> 
 (y = Abs_diagram (
-(basic (A\<otimes>z2))\<circ>(y2)))
+(basic (z2 \<otimes> A))\<circ>(y2)))
 \<and>(0 = (fst (count z2)))
 \<and>(strands B))"
 
@@ -864,6 +864,7 @@ where
 "tanglerel_compbelow x y \<equiv> 
 (tanglerel_compbelow_right x y) \<or> (tanglerel_compbelow_left x y)
 \<or> (tanglerel_compbelow_centerleft x y) \<or> (tanglerel_compbelow_centerright x y)
+\<or> (tanglerel_compbelow_bottomright x y) \<or> (tanglerel_compbelow_bottomleft x y)
 "
 
 (*comp above*)
@@ -1026,6 +1027,10 @@ lemma framed_reflective: "framed_tanglerel_equiv x x" unfolding framed_tanglerel
 lemma tangle_symmetry:"symp tanglerel_equiv" using tanglerel_symp symmetry3 
 by (metis (full_types) tanglerel_equiv_def)
 
+
+lemma tangle_symmetry2:"(tanglerel_equiv x y)\<Longrightarrow> (tanglerel_equiv y x)" using tangle_symmetry sympD
+ by metis
+
 lemma framed_tangle_symmetry:"symp framed_tanglerel_equiv" using framed_tanglerel_symp symmetry3 
 by (metis (full_types) framed_tanglerel_equiv_def)
 
@@ -1052,18 +1057,16 @@ qed
 lemma strand_makestrand: " strands (makestrand n)" 
 apply(induct_tac n)
 apply(auto)
-apply(simp add:e_vert_def)
 done
 
 lemma test_00: "(makestrand (n+1)) = vert#(makestrand n)" by auto
 
-lemma test_0: "(makestrand (n+1)) = e_vert\<otimes>(makestrand n)" using e_vert_def test_00 append_Nil by metis
+lemma test_0: "(makestrand (n+1)) = (cement vert)\<otimes>(makestrand n)" using test_00 append_Nil by metis
 
 
-lemma test_1: "(makestrand (n+1)) = (makestrand n)\<otimes>e_vert" 
+lemma test_1: "(makestrand (n+1)) = (makestrand n)\<otimes>(cement vert)" 
 apply(induct_tac n)
 apply(auto)
-apply(simp add:e_vert_def)
 apply (metis Tangles.append.append_Nil leftright_associativity)
 done
 
@@ -1077,18 +1080,16 @@ definition sndcount:: convert  where "(sndcount x) = (nat (snd (count x)))"
 lemma makestrand_fstequality:"(fst (count (makestrand n))) = (int n)+1" 
 apply (induct_tac n)
 apply(auto)
-apply(simp add: e_vert_def)
 done
 
 lemma makestrand_sndequality:"(snd (count (makestrand n))) = (int n)+1" 
 apply (induct_tac n)
 apply(auto)
-apply(simp add: e_vert_def)
 done
 
 lemma makestrand_fstsndequality:"(fst (count (makestrand n))) = (snd (count (makestrand n)))" 
 apply (induct_tac n)
-apply(auto simp add:e_vert_def)
+apply(auto)
 done
 
 lemma nat_int:" ((int n)\<ge> 0)" by auto
@@ -1273,7 +1274,7 @@ qed
 theorem metaequivalence_left: 
 assumes "(snd (count y1))>1"
 and "w4 = makestrand  (nat ((snd (count y1)) + (-2)))"
-shows "tanglerel_equiv (Abs_diagram ((x1)\<circ>(basic (e_cup\<otimes>y1))\<circ>(basic (e_vert\<otimes>e_cap\<otimes>w4))\<circ>z1))
+shows "tanglerel_equiv (Abs_diagram ((x1)\<circ>(basic ((cement cup)\<otimes>y1))\<circ>(basic ((cement vert)\<otimes>(cement cap)\<otimes>w4))\<circ>z1))
              (Abs_diagram (x1 \<circ> basic y1 \<circ>z1))" 
 proof-
 let ?z4 = "makestrand (nat ((snd (count y1)) + (-2))+1)"                                                                                           
@@ -1350,35 +1351,35 @@ have step1:
 
 have w_subst: "w4 = (makestrand ?k)" using assms by auto
 
-have step2_subresult0: "(makestrand (?k+1)) = (e_vert\<otimes>(makestrand ?k))" 
- apply(simp add: e_vert_def)
+have step2_subresult0: "(makestrand (?k+1)) = ((cement vert)\<otimes>(makestrand ?k))" 
+ apply(simp)
  done
 
-have step2_subresult1:"?z4 = e_vert\<otimes>(makestrand ?k)" using C step2_subresult0 by auto
+have step2_subresult1:"?z4 = (cement vert)\<otimes>(makestrand ?k)" using C step2_subresult0 by auto
 
 have step2_subresult2: "(Abs_diagram (?x2 \<circ> (basic ?z4) \<circ>(basic ?z4)\<circ>z1)) =
-(Abs_diagram (?x2  \<circ> (basic (e_vert\<otimes>w4))\<circ> (basic (e_vert \<otimes>w4))\<circ>z1))" 
+(Abs_diagram (?x2  \<circ> (basic ((cement vert)\<otimes>w4))\<circ> (basic ((cement vert) \<otimes>w4))\<circ>z1))" 
                         using w_subst step2_subresult1 by auto
 
 have step2_subresult3: "(snd (count w4)) = (fst (count w4))" using makestrand_fstsndequality w_subst
 by auto
 
-let ?x = "(Abs_diagram (?x2 \<circ>(basic (e_cup\<otimes>e_vert\<otimes>w4))\<circ>(basic (e_vert\<otimes>e_cap\<otimes>w4))\<circ>z1))"
-let ?y = "(Abs_diagram (?x2 \<circ>(basic (e_vert\<otimes>w4))\<circ>(basic (e_vert\<otimes>w4))\<circ>z1))"
+let ?x = "(Abs_diagram (?x2 \<circ>(basic ((cement cup)\<otimes>(cement vert)\<otimes>w4))\<circ>(basic ((cement vert)\<otimes>(cement cap)\<otimes>w4))\<circ>z1))"
+let ?y = "(Abs_diagram (?x2 \<circ>(basic ((cement vert)\<otimes>w4))\<circ>(basic ((cement vert)\<otimes>w4))\<circ>z1))"
 
 have step2_subresult4:
-"\<exists>y1.\<exists>y2.\<exists>w1.\<exists>w2.(?x = Abs_diagram (y1 \<circ> (basic (e_cup \<otimes> e_vert \<otimes> w1)) \<circ> (basic (e_vert \<otimes> e_cap \<otimes> w2)) \<circ> y2))"
+"\<exists>y1.\<exists>y2.\<exists>w1.\<exists>w2.(?x = Abs_diagram (y1 \<circ> (basic ((cement cup) \<otimes> (cement vert) \<otimes> w1)) \<circ> (basic ((cement vert) \<otimes> (cement cap) \<otimes> w2)) \<circ> y2))"
   using exI by auto
  
 have step2_subresult5:
-"\<exists>y1.\<exists>y2.\<exists>w1.\<exists>w2.(?y = Abs_diagram (y1 \<circ> (basic (e_vert \<otimes> w1)) \<circ> (basic (e_vert \<otimes> w2)) \<circ> y2))"
+"\<exists>y1.\<exists>y2.\<exists>w1.\<exists>w2.(?y = Abs_diagram (y1 \<circ> (basic ((cement vert) \<otimes> w1)) \<circ> (basic ((cement vert) \<otimes> w2)) \<circ> y2))"
  using exI by auto
 
 have step2_subresult6: 
 " (\<exists>y1.\<exists>w1.\<exists>w2.\<exists>y2.((?x = Abs_diagram ((y1)
-\<circ>(basic (e_cup\<otimes>e_vert\<otimes>w1)\<circ>(basic (e_vert\<otimes>e_cap\<otimes>w2)))\<circ>(y2)))\<and>(?y = Abs_diagram
+\<circ>(basic ((cement cup)\<otimes>(cement vert)\<otimes>w1)\<circ>(basic ((cement vert)\<otimes>(cement cap)\<otimes>w2)))\<circ>(y2)))\<and>(?y = Abs_diagram
  ((y1)
-\<circ>(basic (e_vert\<otimes>w1))\<circ>(basic (e_vert\<otimes>w2))\<circ>(y2))))
+\<circ>(basic ((cement vert)\<otimes>w1))\<circ>(basic ((cement vert)\<otimes>w2))\<circ>(y2))))
  \<and> ((snd (count w1)) = (fst (count w2))))"
 using  step2_subresult3 exI by auto
 
@@ -1389,17 +1390,17 @@ using tanglerel_straighten_rightdowntop_def step2_subresult6 by auto
 have step2_subresult8:"tanglerel ?x ?y" 
 using tanglerel_def tanglerel_straighten_def step2_subresult7 by auto
 
-have step2_subresult9: "tanglerel (Abs_diagram ((?x2) \<circ>(basic (e_cup\<otimes>e_vert\<otimes>w4))\<circ>(basic (e_vert\<otimes>e_cap\<otimes>w4))\<circ>z1)) 
-              (Abs_diagram ((?x2) \<circ>(basic (e_vert\<otimes>w4))\<circ>(basic (e_vert\<otimes>w4))\<circ>z1))"
+have step2_subresult9: "tanglerel (Abs_diagram ((?x2) \<circ>(basic ((cement cup)\<otimes>(cement vert)\<otimes>w4))\<circ>(basic ((cement vert)\<otimes>(cement cap)\<otimes>w4))\<circ>z1)) 
+              (Abs_diagram ((?x2) \<circ>(basic ((cement vert)\<otimes>w4))\<circ>(basic ((cement vert)\<otimes>w4))\<circ>z1))"
                using step2_subresult8 by auto 
 
-have step2_equiv1: "tanglerel_equiv (Abs_diagram (x1\<circ>basic y1\<circ>(basic (e_cup\<otimes>e_vert\<otimes>w4))\<circ>(basic (e_vert\<otimes>e_cap\<otimes>w4))\<circ>z1)) 
-              (Abs_diagram (x1\<circ>basic y1 \<circ>(basic (e_vert\<otimes>w4))\<circ>(basic (e_vert\<otimes>w4))\<circ>z1))"
+have step2_equiv1: "tanglerel_equiv (Abs_diagram (x1\<circ>basic y1\<circ>(basic ((cement cup)\<otimes>(cement vert)\<otimes>w4))\<circ>(basic ((cement vert)\<otimes>(cement cap)\<otimes>w4))\<circ>z1)) 
+              (Abs_diagram (x1\<circ>basic y1 \<circ>(basic ((cement vert)\<otimes>w4))\<circ>(basic ((cement vert)\<otimes>w4))\<circ>z1))"
                using step2_subresult9 compose_leftassociativity r_into_rtranclp 
                tanglerel_equiv_def
                      by metis
 
-have step2: "tanglerel_equiv (Abs_diagram (x1\<circ>basic y1\<circ>(basic (e_cup\<otimes>?z4))\<circ>(basic (e_vert\<otimes>e_cap\<otimes>w4))\<circ>z1)) 
+have step2: "tanglerel_equiv (Abs_diagram (x1\<circ>basic y1\<circ>(basic ((cement cup)\<otimes>?z4))\<circ>(basic ((cement vert)\<otimes>(cement cap)\<otimes>w4))\<circ>z1)) 
               (Abs_diagram (x1\<circ>basic y1 \<circ>(basic ?z4)\<circ>(basic (?z4))\<circ>z1))"
                using  step2_subresult9 compose_leftassociativity r_into_rtranclp 
                tanglerel_equiv_def step2_subresult1 w_subst
@@ -1409,60 +1410,60 @@ have step2: "tanglerel_equiv (Abs_diagram (x1\<circ>basic y1\<circ>(basic (e_cup
 have step3_preliminary1: "fst (count (v\<otimes>w)) = fst (count (cup#(v\<otimes>w)))" using count_def brickcount_def
 by auto
 have step3_preliminary2 : 
-"count ((cup)#(e_cup\<otimes>w4)) = (fst (brickcount (cup)) + fst (count (e_cup\<otimes>w4)),
- snd (brickcount (cup)) + snd (count (e_cup\<otimes>w4)))"
-using count_def e_cup_def by auto
+"count ((cup)#((cement cup)\<otimes>w4)) = (fst (brickcount (cup)) + fst (count ((cement cup)\<otimes>w4)),
+ snd (brickcount (cup)) + snd (count ((cement cup)\<otimes>w4)))"
+using count_def by auto
 have step3_preliminary3: 
-"(e_cup\<otimes>(e_vert\<otimes>w4)) = cup#(e_vert\<otimes>w4)" using e_cup_def append_Nil by metis
+"((cement cup)\<otimes>((cement vert)\<otimes>w4)) = cup#((cement vert)\<otimes>w4)" using append_Nil by metis
 have step3_subresult0 : 
-"fst (count ((cup)#(e_cup\<otimes>w4))) =  (fst (brickcount (cup)) + fst (count (e_cup\<otimes>w4)))"
-using count_def e_cup_def brickcount_def by auto
+"fst (count ((cup)#((cement cup)\<otimes>w4))) =  (fst (brickcount (cup)) + fst (count ((cement cup)\<otimes>w4)))"
+using count_def  brickcount_def by auto
 have step3_preliminary4 : 
-"(fst (brickcount (cup)) + fst (count (e_cup\<otimes>w4))) = fst (count (e_cup\<otimes>w4))"
+"(fst (brickcount (cup)) + fst (count ((cement cup)\<otimes>w4))) = fst (count ((cement cup)\<otimes>w4))"
 using brickcount_def by auto
 
 have step3_preliminary5:
-"fst (count (cup#(e_cup\<otimes>w4))) =  fst (count (e_cup\<otimes>w4))"
+"fst (count (cup#((cement cup)\<otimes>w4))) =  fst (count ((cement cup)\<otimes>w4))"
 using  step3_preliminary4 step3_subresult0 by auto
 
 have step3_preliminary6:
-"fst (count ((e_cup)\<otimes>(e_cup\<otimes>w4))) =  fst (count (cup#(e_cup\<otimes>w4)))"
+"fst (count (((cement cup))\<otimes>((cement cup)\<otimes>w4))) =  fst (count (cup#((cement cup)\<otimes>w4)))"
 using step3_preliminary3 
-by (metis Tangles.append.append_Nil e_cup_def)
+by (metis Tangles.append.append_Nil)
 
 have step3_preliminary7:
-"fst (count ((e_cup)\<otimes>(e_cup\<otimes>w4))) =  fst (count (e_cup\<otimes>w4))"
+"fst (count (((cement cup))\<otimes>((cement cup)\<otimes>w4))) =  fst (count ((cement cup)\<otimes>w4))"
 using step3_preliminary5  step3_preliminary6 
 by auto
 
-have step3_subresult1 :"fst (wall_count (basic (e_cup\<otimes>e_vert\<otimes>w4))) = fst (wall_count (basic (e_vert\<otimes>w4))) " 
+have step3_subresult1 :"fst (wall_count (basic ((cement cup)\<otimes>(cement vert)\<otimes>w4))) = fst (wall_count (basic ((cement vert)\<otimes>w4))) " 
 using wall_count_def step3_preliminary7
  by (metis Tangles.append.append_Nil add_diff_cancel 
-comm_monoid_add_class.add.left_neutral count.simps(2) e_cup_def fst_conv wall_count.simps(1))
+comm_monoid_add_class.add.left_neutral count.simps(2) fst_conv wall_count.simps(1))
 
-have step3_subresult2: "fst (wall_count (basic (e_vert\<otimes>w4))) = snd (count y1)" 
+have step3_subresult2: "fst (wall_count (basic ((cement vert)\<otimes>w4))) = snd (count y1)" 
                using w_subst step2_subresult1 subresult8 by auto
-have step3_subresult3: "fst (wall_count (basic (e_cup\<otimes>e_vert\<otimes>w4))) = snd (count y1)" 
+have step3_subresult3: "fst (wall_count (basic ((cement cup)\<otimes>(cement vert)\<otimes>w4))) = snd (count y1)" 
                using step3_subresult1 step3_subresult2 by auto 
-have step3_subresult4: "fst (wall_count (basic (e_vert\<otimes>w4))) = snd (wall_count ?x2)" 
+have step3_subresult4: "fst (wall_count (basic ((cement vert)\<otimes>w4))) = snd (wall_count ?x2)" 
                using step3_subresult3 subresult0 wall_count_def step3_subresult2 subresult1 by auto 
-have step3_subresult5: "fst (wall_count (basic (e_vert\<otimes>w4))) = snd (wall_count (x1\<circ>(basic y1)))" 
+have step3_subresult5: "fst (wall_count (basic ((cement vert)\<otimes>w4))) = snd (wall_count (x1\<circ>(basic y1)))" 
                using step3_subresult4  wall_count_def by auto
 have step3_subresult6: "fst (brickcount cup) =  0" using brickcount_def by auto
-have step3_subresult7: "fst (count e_cup) =  0" using e_cup_def count_def step3_subresult6 
+have step3_subresult7: "fst (count (cement cup)) =  0" using  count_def step3_subresult6 
 by (metis count.simps(1))
-have step3_subresult8: "strands (vert#e_vert)" using e_vert_def append_def strands_def  brickstrand.simps(1) 
-                        strands.simps(1) strands.simps(2) 
+have step3_subresult8: "strands (vert#(cement vert))" using  append_def strands_def  
+brickstrand.simps(1) strands.simps(1) strands.simps(2) 
                        by metis
-have step3_subresult9: "(vert#e_vert) = (e_vert\<otimes>e_vert)" using append_Nil e_vert_def
+have step3_subresult9: "(vert#(cement vert)) = ((cement vert)\<otimes>(cement vert))" using append_Nil 
                         by metis
-have step3_subresult10: "strands (e_vert\<otimes>e_vert)" using step3_subresult8 step3_subresult9
-                        by auto
-let ?a0 = "(basic (e_vert\<otimes>e_cap\<otimes>w4))\<circ>z1"
-let ?b0 = "(e_vert\<otimes>e_vert)"
-let  ?a = "Abs_diagram ((x1)\<circ>(basic (e_cup\<otimes>y1))\<circ>(basic (?b0\<otimes>(e_vert\<otimes>w4)))\<circ>((basic (e_vert\<otimes>e_cap\<otimes>w4))\<circ>z1))"
+have step3_subresult10: "strands ((cement vert)\<otimes>(cement vert))" using step3_subresult8 step3_subresult9
+     by metis
+let ?a0 = "(basic ((cement vert)\<otimes>(cement cap)\<otimes>w4))\<circ>z1"
+let ?b0 = "((cement vert)\<otimes>(cement vert))"
+let  ?a = "Abs_diagram ((x1)\<circ>(basic ((cement cup)\<otimes>y1))\<circ>(basic (?b0\<otimes>((cement vert)\<otimes>w4)))\<circ>((basic ((cement vert)\<otimes>(cement cap)\<otimes>w4))\<circ>z1))"
 (*check b*)
-let ?b = "Abs_diagram ((x1)\<circ>(basic y1)\<circ>(basic (e_cup \<otimes> (e_vert \<otimes> w4)))\<circ>((basic (e_vert\<otimes>e_cap\<otimes>w4))\<circ>z1))"
+let ?b = "Abs_diagram ((x1)\<circ>(basic y1)\<circ>(basic ((cement cup) \<otimes> ((cement vert) \<otimes> w4)))\<circ>((basic ((cement vert)\<otimes>(cement cap)\<otimes>w4))\<circ>z1))"
 
 have step3_subresult11: "  \<exists>y1.\<exists>w1.\<exists>w2.\<exists>A.\<exists>B.\<exists>y2.(?a = Abs_diagram
  ((y1)\<circ>(basic (A\<otimes>w1))\<circ>(basic (B\<otimes>w2))\<circ>(y2)))"
@@ -1500,44 +1501,46 @@ have step3_subresult17: "tanglerel_equiv ?a ?b"
        by (metis (full_types) r_into_rtranclp)
 
 have step3_subresult18: "tanglerel_equiv 
-(Abs_diagram ((x1)\<circ>(basic (e_cup\<otimes>y1))\<circ>(basic ((e_vert\<otimes>e_vert)\<otimes>(e_vert\<otimes>w4)))\<circ>((basic (e_vert\<otimes>e_cap\<otimes>w4))\<circ>z1)))
-(Abs_diagram ((x1)\<circ>(basic y1)\<circ>(basic (e_cup \<otimes> (e_vert \<otimes> w4)))\<circ>((basic (e_vert\<otimes>e_cap\<otimes>w4))\<circ>z1)))"
+(Abs_diagram ((x1)\<circ>(basic ((cement cup)\<otimes>y1))\<circ>(basic (((cement vert)\<otimes>(cement vert))
+\<otimes>((cement vert)\<otimes>w4)))\<circ>((basic ((cement vert)\<otimes>(cement cap)\<otimes>w4))\<circ>z1)))
+(Abs_diagram ((x1)\<circ>(basic y1)\<circ>(basic ((cement cup) \<otimes> ((cement vert) \<otimes> w4)))\<circ>((basic ((cement vert)
+\<otimes>(cement cap)\<otimes>w4))\<circ>z1)))"
  using step3_subresult17
 by metis
 
 have step3: 
-"tanglerel_equiv (Abs_diagram ((x1)\<circ>(basic (e_cup\<otimes>y1))\<circ>(basic (e_vert\<otimes>e_vert\<otimes>e_vert\<otimes>w4))\<circ>(basic (e_vert\<otimes>e_cap\<otimes>w4))\<circ>z1))
- (Abs_diagram (((x1)\<circ>(basic y1))\<circ>(basic (e_cup \<otimes> ?z4))\<circ> (basic (e_vert\<otimes>e_cap\<otimes>w4))\<circ>z1))" 
+"tanglerel_equiv (Abs_diagram ((x1)\<circ>(basic ((cement cup)\<otimes>y1))\<circ>(basic ((cement vert)\<otimes>(cement vert)\<otimes>(cement vert)\<otimes>w4))\<circ>(basic ((cement vert)\<otimes>(cement cap)\<otimes>w4))\<circ>z1))
+ (Abs_diagram (((x1)\<circ>(basic y1))\<circ>(basic ((cement cup) \<otimes> ?z4))\<circ> (basic ((cement vert)\<otimes>(cement cap)\<otimes>w4))\<circ>z1))" 
 using step3_subresult18 leftright_associativity w_subst step2_subresult1 left_associativity
  compose_leftassociativity
 by auto
 
 (*step 4*)
 
-let ?p = "(x1)\<circ>(basic (e_cup\<otimes>y1))"
-let ?q = "(basic (e_vert\<otimes>e_cap\<otimes>w4))\<circ>z1"
-let ?r = " basic (e_vert \<otimes> e_vert \<otimes> e_vert \<otimes> w4)"
+let ?p = "(x1)\<circ>(basic ((cement cup)\<otimes>y1))"
+let ?q = "(basic ((cement vert)\<otimes>(cement cap)\<otimes>w4))\<circ>z1"
+let ?r = " basic ((cement vert) \<otimes> (cement vert) \<otimes> (cement vert) \<otimes> w4)"
 
-have step4_subresult1: "strands (e_vert \<otimes> e_vert \<otimes> e_vert \<otimes> w4)"
-using assms  Tangles.append.append_Nil e_vert_def preliminary_result3 step2_subresult1 strands.simps(2)
+have step4_subresult1: "strands ((cement vert) \<otimes> (cement vert) \<otimes> (cement vert) \<otimes> w4)"
+using assms  Tangles.append.append_Nil  preliminary_result3 step2_subresult1 strands.simps(2)
 by metis
 
-have step4_subresult2: "snd (count (e_cup\<otimes>y1)) =  snd (count (cup#y1))" 
-using Tangles.append.append_Nil count_def e_cup_def by (metis)
+have step4_subresult2: "snd (count ((cement cup)\<otimes>y1)) =  snd (count (cup#y1))" 
+using Tangles.append.append_Nil count_def  by (metis)
 
 have step4_subresult3: " snd (count (cup#y1)) =  2+ snd (count (y1))"
 using step4_subresult2 count_def brickcount_def by auto
 
-have step4_subresult4: "snd (count (e_cup\<otimes>y1)) > snd (count (y1))"
+have step4_subresult4: "snd (count ((cement cup)\<otimes>y1)) > snd (count (y1))"
 using step4_subresult2 step4_subresult3 add_strict_increasing dbl_def 
 dbl_simps(3) order_refl zero_less_two
 by auto
 
-have step4_subresult5: "snd (count (e_cup\<otimes>y1)) > 1"
+have step4_subresult5: "snd (count ((cement cup)\<otimes>y1)) > 1"
 using step4_subresult4 assms
 by auto
 
-have step4_subresult6: "snd (wall_count ?p) = (snd (count (e_cup\<otimes>y1)))"
+have step4_subresult6: "snd (wall_count ?p) = (snd (count ((cement cup)\<otimes>y1)))"
 using wall_count_def  snd_conv wall_count.simps(1) wall_count_compose
 by auto
 
@@ -1549,14 +1552,14 @@ by auto
 
 have step4_subresult8: 
 "tanglerel_compress_null 
-(Abs_diagram (?p\<circ>(basic (e_vert \<otimes> e_vert \<otimes> e_vert \<otimes> w4))\<circ>?q))
+(Abs_diagram (?p\<circ>(basic ((cement vert) \<otimes> (cement vert) \<otimes> (cement vert) \<otimes> w4))\<circ>?q))
  (Abs_diagram (?p\<circ>?q))"
 using step4_subresult1 step4_subresult7 tanglerel_compress_null_def
-by auto
+by metis
 
 have step4_subresult9: 
 "tanglerel_compress
-(Abs_diagram (?p\<circ>(basic (e_vert \<otimes> e_vert \<otimes> e_vert \<otimes> w4))\<circ>?q))
+(Abs_diagram (?p\<circ>(basic ((cement vert) \<otimes> (cement vert) \<otimes> (cement vert) \<otimes> w4))\<circ>?q))
  (Abs_diagram (?p\<circ>?q))"
 using step4_subresult8 tanglerel_compress_def
 by auto
@@ -1565,7 +1568,7 @@ by auto
 have step4_subresult10: 
 "tanglerel
  (Abs_diagram (?p\<circ>?q))
-(Abs_diagram (?p\<circ>(basic (e_vert \<otimes> e_vert \<otimes> e_vert \<otimes> w4))\<circ>?q))
+(Abs_diagram (?p\<circ>(basic ((cement vert) \<otimes> (cement vert) \<otimes> (cement vert) \<otimes> w4))\<circ>?q))
 "
 using step4_subresult9 step4_subresult8 tanglerel_def
 by auto
@@ -1574,7 +1577,7 @@ by auto
 have step4_subresult11: 
 "tanglerel_equiv
  (Abs_diagram (?p\<circ>?q))
-(Abs_diagram (?p\<circ>(basic (e_vert \<otimes> e_vert \<otimes> e_vert \<otimes> w4))\<circ>?q))
+(Abs_diagram (?p\<circ>(basic ((cement vert) \<otimes> (cement vert) \<otimes> (cement vert) \<otimes> w4))\<circ>?q))
 "
 using step4_subresult10 tanglerel_equiv_def compose_leftassociativity 
 leftright_associativity r_into_rtranclp step3_subresult11 step3_subresult13
@@ -1582,8 +1585,8 @@ by metis
 
 have step4: 
 "tanglerel_equiv
- (Abs_diagram ((x1)\<circ>(basic (e_cup\<otimes>y1))\<circ>(basic (e_vert\<otimes>e_cap\<otimes>w4))\<circ>z1))
-(Abs_diagram ((x1)\<circ>(basic (e_cup\<otimes>y1))\<circ>(basic (e_vert \<otimes> e_vert \<otimes> e_vert \<otimes> w4))\<circ>(basic (e_vert\<otimes>e_cap\<otimes>w4))\<circ>z1))
+ (Abs_diagram ((x1)\<circ>(basic ((cement cup)\<otimes>y1))\<circ>(basic ((cement vert)\<otimes>(cement cap)\<otimes>w4))\<circ>z1))
+(Abs_diagram ((x1)\<circ>(basic ((cement cup)\<otimes>y1))\<circ>(basic ((cement vert) \<otimes> (cement vert) \<otimes> (cement vert) \<otimes> w4))\<circ>(basic ((cement vert)\<otimes>(cement cap)\<otimes>w4))\<circ>z1))
 "
 using step4_subresult10 tanglerel_equiv_def compose_leftassociativity 
 leftright_associativity r_into_rtranclp step3_subresult11 step3_subresult13
@@ -1592,11 +1595,11 @@ by metis
 (*combining steps*)
                       
 have combine_vert: 
-"tanglerel_equiv (Abs_diagram (x1\<circ>basic y1\<circ>(basic (e_cup\<otimes>?z4))\<circ>(basic (e_vert\<otimes>e_cap\<otimes>w4))\<circ>z1)) 
+"tanglerel_equiv (Abs_diagram (x1\<circ>basic y1\<circ>(basic ((cement cup)\<otimes>?z4))\<circ>(basic ((cement vert)\<otimes>(cement cap)\<otimes>w4))\<circ>z1)) 
                             (Abs_diagram (x1 \<circ> basic y1 \<circ>z1))" 
                using step1 step2 rtranclp_trans tanglerel_equiv_def by metis
 
-have combine_cup:"tanglerel_equiv (Abs_diagram ((x1)\<circ>(basic (e_cup\<otimes>y1))\<circ>(basic (e_vert\<otimes>e_vert\<otimes>?z4))\<circ>(basic (e_vert\<otimes>e_cap\<otimes>w4))\<circ>z1))
+have combine_cup:"tanglerel_equiv (Abs_diagram ((x1)\<circ>(basic ((cement cup)\<otimes>y1))\<circ>(basic ((cement vert)\<otimes>(cement vert)\<otimes>?z4))\<circ>(basic ((cement vert)\<otimes>(cement cap)\<otimes>w4))\<circ>z1))
              (Abs_diagram (x1 \<circ> basic y1 \<circ>z1))" 
                using step3 combine_vert tanglerel_equiv_def rtranclp_trans
                 compose_leftassociativity leftright_associativity 
@@ -1605,7 +1608,7 @@ have combine_cup:"tanglerel_equiv (Abs_diagram ((x1)\<circ>(basic (e_cup\<otimes
                by (metis) 
 
 have combine_compress:"tanglerel_equiv
- (Abs_diagram ((x1)\<circ>(basic (e_cup\<otimes>y1))\<circ>(basic (e_vert\<otimes>e_cap\<otimes>w4))\<circ>z1))
+ (Abs_diagram ((x1)\<circ>(basic ((cement cup)\<otimes>y1))\<circ>(basic ((cement vert)\<otimes>(cement cap)\<otimes>w4))\<circ>z1))
              (Abs_diagram (x1 \<circ> basic y1 \<circ>z1))" 
 using combine_cup step4 
 combine_vert tanglerel_equiv_def rtranclp_trans
@@ -1625,11 +1628,11 @@ apply (metis append.append_Nil count.simps(1) count.simps(2))
 apply(auto)
 done
 
-lemma count_cup_rightcompose:" count(v\<otimes>e_cup) = (fst (count v), snd (count v)+2)"
-apply (simp add:count_rightcompose e_cup_def)
+lemma count_cup_rightcompose:" count(v\<otimes>(cement cup)) = (fst (count v), snd (count v)+2)"
+apply (simp add:count_rightcompose)
 done
 
-lemma fstcount_cup_rightcompose:" fst (count(v\<otimes>e_cup)) = fst (count v)"
+lemma fstcount_cup_rightcompose:" fst (count(v\<otimes>(cement cup))) = fst (count v)"
 apply (simp add: count_cup_rightcompose)
 done
 
@@ -1638,7 +1641,7 @@ done
 theorem metaequivalence_right: 
 assumes "(snd (count y1))>1" 
 and "w4 = makestrand  (nat ((snd (count y1)) + (-2)))"
-shows "tanglerel_equiv (Abs_diagram ((x1)\<circ>(basic (y1\<otimes>e_cup))\<circ>(basic (w4\<otimes>e_cap\<otimes>e_vert))\<circ>z1))
+shows "tanglerel_equiv (Abs_diagram ((x1)\<circ>(basic (y1\<otimes>(cement cup)))\<circ>(basic (w4\<otimes>(cement cap)\<otimes>(cement vert)))\<circ>z1))
              (Abs_diagram (x1 \<circ> basic y1 \<circ>z1))" 
 proof-
 let ?k = " (nat ((snd (count y1))+ (-2) ))" 
@@ -1711,33 +1714,33 @@ have step1:
 
 have w_subst: "w4 = (makestrand ?k)" using assms by auto
 
-have step2_subresult0: "(makestrand (?k+1)) = ((makestrand ?k) \<otimes>e_vert)" 
+have step2_subresult0: "(makestrand (?k+1)) = ((makestrand ?k) \<otimes>(cement vert))" 
  by (metis test_00 test_1)
  
-have step2_subresult1:"?z4 = (makestrand ?k)\<otimes>e_vert  " using C step2_subresult0 by auto
+have step2_subresult1:"?z4 = (makestrand ?k)\<otimes>(cement vert)  " using C step2_subresult0 by auto
 
 have step2_subresult2: "(Abs_diagram (?x2 \<circ> (basic ?z4) \<circ>(basic ?z4)\<circ>z1)) =
-(Abs_diagram (?x2  \<circ> (basic (w4\<otimes>e_vert))\<circ> (basic (w4\<otimes>e_vert))\<circ>z1))" 
+(Abs_diagram (?x2  \<circ> (basic (w4\<otimes>(cement vert)))\<circ> (basic (w4\<otimes>(cement vert)))\<circ>z1))" 
                         using w_subst step2_subresult1 by auto
 
 have step2_subresult3: "(snd (count w4)) = (fst (count w4))" using makestrand_fstsndequality w_subst
 by auto
 
-let ?x = "(Abs_diagram (?x2 \<circ>(basic (w4\<otimes>e_vert\<otimes>e_cup))\<circ>(basic (w4\<otimes>e_cap\<otimes>e_vert))\<circ>z1))"
-let ?y = "(Abs_diagram (?x2 \<circ>(basic (w4\<otimes>e_vert))\<circ>(basic (w4\<otimes>e_vert))\<circ>z1))"
+let ?x = "(Abs_diagram (?x2 \<circ>(basic (w4\<otimes>(cement vert)\<otimes>(cement cup)))\<circ>(basic (w4\<otimes>(cement cap)\<otimes>(cement vert)))\<circ>z1))"
+let ?y = "(Abs_diagram (?x2 \<circ>(basic (w4\<otimes>(cement vert)))\<circ>(basic (w4\<otimes>(cement vert)))\<circ>z1))"
 
 have step2_subresult4:
-"\<exists>y1.\<exists>y2.\<exists>w1.\<exists>w2.(?x = Abs_diagram (y1 \<circ> (basic (w1\<otimes>e_vert\<otimes>e_cup)) \<circ> (basic (w2\<otimes>e_cap\<otimes>e_vert)) \<circ> y2))"
+"\<exists>y1.\<exists>y2.\<exists>w1.\<exists>w2.(?x = Abs_diagram (y1 \<circ> (basic (w1\<otimes>(cement vert)\<otimes>(cement cup))) \<circ> (basic (w2\<otimes>(cement cap)\<otimes>(cement vert))) \<circ> y2))"
   using exI by auto
  
 have step2_subresult5:
-"\<exists>y1.\<exists>y2.\<exists>w1.\<exists>w2.(?y = Abs_diagram (y1 \<circ> (basic (w1\<otimes>e_vert)) \<circ> (basic (w2\<otimes>e_vert)) \<circ> y2))"
+"\<exists>y1.\<exists>y2.\<exists>w1.\<exists>w2.(?y = Abs_diagram (y1 \<circ> (basic (w1\<otimes>(cement vert))) \<circ> (basic (w2\<otimes>(cement vert))) \<circ> y2))"
  using exI by auto
 
 have step2_subresult6: 
 " (\<exists>y1.\<exists>w1.\<exists>w2.\<exists>y2.((?x = Abs_diagram ((y1)
-\<circ> (basic (w1\<otimes>e_vert\<otimes>e_cup)) \<circ> (basic (w2\<otimes>e_cap\<otimes>e_vert)) \<circ> y2)))
-\<and>(?y = Abs_diagram (y1 \<circ> (basic (w1\<otimes>e_vert)) \<circ> (basic (w2\<otimes>e_vert)) \<circ> y2))
+\<circ> (basic (w1\<otimes>(cement vert)\<otimes>(cement cup))) \<circ> (basic (w2\<otimes>(cement cap)\<otimes>(cement vert))) \<circ> y2)))
+\<and>(?y = Abs_diagram (y1 \<circ> (basic (w1\<otimes>(cement vert))) \<circ> (basic (w2\<otimes>(cement vert))) \<circ> y2))
  \<and> ((snd (count w1)) = (fst (count w2))))"
 using  step2_subresult3 exI by auto
 
@@ -1750,17 +1753,17 @@ by (metis)
 have step2_subresult8:"tanglerel ?x ?y" 
 using tanglerel_def tanglerel_straighten_def step2_subresult7 by auto
 
-have step2_subresult9: "tanglerel (Abs_diagram ((?x2) \<circ>(basic (w4\<otimes>e_vert\<otimes>e_cup))\<circ>(basic (w4\<otimes>e_cap\<otimes>e_vert))\<circ>z1)) 
-              (Abs_diagram ((?x2) \<circ>(basic (w4\<otimes>e_vert))\<circ>(basic (w4\<otimes>e_vert))\<circ>z1))"
+have step2_subresult9: "tanglerel (Abs_diagram ((?x2) \<circ>(basic (w4\<otimes>(cement vert)\<otimes>(cement cup)))\<circ>(basic (w4\<otimes>(cement cap)\<otimes>(cement vert)))\<circ>z1)) 
+              (Abs_diagram ((?x2) \<circ>(basic (w4\<otimes>(cement vert)))\<circ>(basic (w4\<otimes>(cement vert)))\<circ>z1))"
                using step2_subresult8 by auto 
 
-have step2_equiv1: "tanglerel_equiv (Abs_diagram (x1\<circ>basic y1\<circ>(basic (w4\<otimes>e_vert\<otimes>e_cup))\<circ>(basic (w4\<otimes>e_cap\<otimes>e_vert))\<circ>z1)) 
-              (Abs_diagram (x1\<circ>basic y1 \<circ>(basic (w4\<otimes>e_vert))\<circ>(basic (w4\<otimes>e_vert))\<circ>z1))"
+have step2_equiv1: "tanglerel_equiv (Abs_diagram (x1\<circ>basic y1\<circ>(basic (w4\<otimes>(cement vert)\<otimes>(cement cup)))\<circ>(basic (w4\<otimes>(cement cap)\<otimes>(cement vert)))\<circ>z1)) 
+              (Abs_diagram (x1\<circ>basic y1 \<circ>(basic (w4\<otimes>(cement vert)))\<circ>(basic (w4\<otimes>(cement vert)))\<circ>z1))"
                using step2_subresult9 compose_leftassociativity r_into_rtranclp 
                tanglerel_equiv_def
                      by metis
 
-have step2: "tanglerel_equiv (Abs_diagram (x1\<circ>basic y1\<circ>(basic (?z4\<otimes>e_cup))\<circ>(basic (w4\<otimes>e_cap\<otimes>e_vert))\<circ>z1)) 
+have step2: "tanglerel_equiv (Abs_diagram (x1\<circ>basic y1\<circ>(basic (?z4\<otimes>(cement cup)))\<circ>(basic (w4\<otimes>(cement cap)\<otimes>(cement vert)))\<circ>z1)) 
               (Abs_diagram (x1\<circ>basic y1 \<circ>(basic ?z4)\<circ>(basic (?z4))\<circ>z1))"
                using  step2_subresult9 compose_leftassociativity r_into_rtranclp 
                tanglerel_equiv_def step2_subresult1 w_subst leftright_associativity
@@ -1771,46 +1774,46 @@ have step2: "tanglerel_equiv (Abs_diagram (x1\<circ>basic y1\<circ>(basic (?z4\<
 have step3_preliminary1: "fst (count (v\<otimes>w)) = fst (count (cup#(v\<otimes>w)))" using count_def brickcount_def
 by auto
 have step3_preliminary2 : 
-"count ((w4\<otimes>e_vert)\<otimes>e_cup) = ((fst (count (w4\<otimes>e_vert))), (snd (count (w4\<otimes>e_vert))+2))"
+"count ((w4\<otimes>(cement vert))\<otimes>(cement cup)) = ((fst (count (w4\<otimes>(cement vert)))), (snd (count (w4\<otimes>(cement vert)))+2))"
 using fstcount_cup_rightcompose  count_cup_rightcompose
 by (metis) 
 
 have step3_preliminary3 : 
-"fst (count ((w4\<otimes>e_vert)\<otimes>e_cup)) = (fst (count (w4\<otimes>e_vert)))"
+"fst (count ((w4\<otimes>(cement vert))\<otimes>(cement cup))) = (fst (count (w4\<otimes>(cement vert))))"
 using step3_preliminary2
 by auto
 
 have step3_subresult1 :
-"fst (wall_count (basic ((w4\<otimes>e_vert)\<otimes>e_cup))) = fst (wall_count (basic (w4\<otimes>e_vert))) " 
+"fst (wall_count (basic ((w4\<otimes>(cement vert))\<otimes>(cement cup)))) = fst (wall_count (basic (w4\<otimes>(cement vert)))) " 
 using wall_count_def step3_preliminary3
  by (metis Tangles.append.append_Nil add_diff_cancel 
-comm_monoid_add_class.add.left_neutral count.simps(2) e_cup_def fst_conv wall_count.simps(1))
+comm_monoid_add_class.add.left_neutral count.simps(2) fst_conv wall_count.simps(1))
 
-have step3_subresult2: "fst (wall_count (basic (w4\<otimes>e_vert))) = snd (count y1)" 
+have step3_subresult2: "fst (wall_count (basic (w4\<otimes>(cement vert)))) = snd (count y1)" 
                using w_subst step2_subresult1 subresult8 by auto
-have step3_subresult3: "fst (wall_count (basic ((w4\<otimes>e_vert\<otimes>e_cup)))) = snd (count y1)" 
+have step3_subresult3: "fst (wall_count (basic ((w4\<otimes>(cement vert)\<otimes>(cement cup))))) = snd (count y1)" 
                using step3_subresult1 step3_subresult2 leftright_associativity
                by (auto)
-have step3_subresult4: "fst (wall_count (basic (w4\<otimes>e_vert))) = snd (wall_count ?x2)" 
+have step3_subresult4: "fst (wall_count (basic (w4\<otimes>(cement vert)))) = snd (wall_count ?x2)" 
                using step3_subresult3 subresult0 wall_count_def step3_subresult2 subresult1 by auto 
-have step3_subresult5: "fst (wall_count (basic (w4\<otimes>e_vert))) = snd (wall_count (x1\<circ>(basic y1)))" 
+have step3_subresult5: "fst (wall_count (basic (w4\<otimes>(cement vert)))) = snd (wall_count (x1\<circ>(basic y1)))" 
                using step3_subresult4  wall_count_def by auto
 have step3_subresult6: "fst (brickcount cup) =  0" using brickcount_def by auto
-have step3_subresult7: "fst (count e_cup) =  0" using e_cup_def count_def step3_subresult6 
+have step3_subresult7: "fst (count (cement cup)) =  0" using count_def step3_subresult6 
 by (metis count.simps(1))
-have step3_subresult8: "strands (vert#e_vert)" using e_vert_def append_def strands_def  brickstrand.simps(1) 
+have step3_subresult8: "strands (vert#(cement vert))" using append_def strands_def  brickstrand.simps(1) 
                         strands.simps(1) strands.simps(2) 
                        by metis
-have step3_subresult9: "(vert#e_vert) = (e_vert\<otimes>e_vert)" using append_Nil e_vert_def
+have step3_subresult9: "(vert#(cement vert)) = ((cement vert)\<otimes>(cement vert))" using append_Nil 
                         by metis
-have step3_subresult10: "strands (e_vert\<otimes>e_vert)" using step3_subresult8 step3_subresult9
-                        by auto
+have step3_subresult10: "strands ((cement vert)\<otimes>(cement vert))" using step3_subresult8 step3_subresult9
+                        by metis
 
 (*need to edit from here*)
 
-let  ?a = "Abs_diagram ((x1)\<circ>(basic (y1 \<otimes> e_cup))\<circ>(basic (?z4\<otimes>e_vert\<otimes>e_vert))\<circ>((basic (w4\<otimes>e_cap\<otimes>e_vert))\<circ>z1))"
+let  ?a = "Abs_diagram ((x1)\<circ>(basic (y1 \<otimes> (cement cup)))\<circ>(basic (?z4\<otimes>(cement vert)\<otimes>(cement vert)))\<circ>((basic (w4\<otimes>(cement cap)\<otimes>(cement vert)))\<circ>z1))"
 (*check b*)
-let ?b = "Abs_diagram ((x1)\<circ>(basic y1)\<circ>(basic ((w4\<otimes>e_vert) \<otimes> e_cup))\<circ>((basic (w4\<otimes>e_cap\<otimes>e_vert))\<circ>z1))"
+let ?b = "Abs_diagram ((x1)\<circ>(basic y1)\<circ>(basic ((w4\<otimes>(cement vert)) \<otimes> (cement cup)))\<circ>((basic (w4\<otimes>(cement cap)\<otimes>(cement vert)))\<circ>z1))"
 
 have step3_subresult11: "  \<exists>y1.\<exists>w1.\<exists>w2.\<exists>A.\<exists>B.\<exists>y2.(?a = Abs_diagram
  ((y1)\<circ>(basic (w1 \<otimes>A))\<circ>(basic (w2\<otimes>B))\<circ>(y2)))"
@@ -1825,9 +1828,9 @@ by metis
 (*check relations*)
 
 
-let  ?a = "Abs_diagram ((x1)\<circ>(basic (y1 \<otimes> e_cup))\<circ>(basic (?z4\<otimes>e_vert\<otimes>e_vert))\<circ>((basic (w4\<otimes>e_cap\<otimes>e_vert))\<circ>z1))"
+let  ?a = "Abs_diagram ((x1)\<circ>(basic (y1 \<otimes> (cement cup)))\<circ>(basic (?z4\<otimes>(cement vert)\<otimes>(cement vert)))\<circ>((basic (w4\<otimes>(cement cap)\<otimes>(cement vert)))\<circ>z1))"
 (*check b*)
-let ?b = "Abs_diagram ((x1)\<circ>(basic y1)\<circ>(basic ((w4\<otimes>e_vert) \<otimes> e_cup))\<circ>((basic (w4\<otimes>e_cap\<otimes>e_vert))\<circ>z1))"
+let ?b = "Abs_diagram ((x1)\<circ>(basic y1)\<circ>(basic ((w4\<otimes>(cement vert)) \<otimes> (cement cup)))\<circ>((basic (w4\<otimes>(cement cap)\<otimes>(cement vert)))\<circ>z1))"
 
 have step3_subresult13: " \<exists>y1.\<exists>z1.\<exists>z2.\<exists>A.\<exists>B.\<exists>y2.((?a = Abs_diagram
  ((y1)\<circ>(basic (z1\<otimes>A))\<circ>(basic (z2\<otimes>B))\<circ>(y2)))\<and> (?b = Abs_diagram ((y1)\<circ>
@@ -1856,45 +1859,44 @@ have step3_subresult17: "tanglerel_equiv ?a ?b"
        by (metis (full_types) r_into_rtranclp)
 
 have step3_subresult18: "tanglerel_equiv 
-(Abs_diagram ((x1)\<circ>(basic (y1 \<otimes> e_cup))\<circ>(basic (?z4\<otimes>e_vert\<otimes>e_vert))\<circ>((basic (w4\<otimes>e_cap\<otimes>e_vert))\<circ>z1)))
-(Abs_diagram ((x1)\<circ>(basic y1)\<circ>(basic ((w4\<otimes>e_vert) \<otimes> e_cup))\<circ>((basic (w4\<otimes>e_cap\<otimes>e_vert))\<circ>z1)))"
+(Abs_diagram ((x1)\<circ>(basic (y1 \<otimes> (cement cup)))\<circ>(basic (?z4\<otimes>(cement vert)\<otimes>(cement vert)))\<circ>((basic (w4\<otimes>(cement cap)\<otimes>(cement vert)))\<circ>z1)))
+(Abs_diagram ((x1)\<circ>(basic y1)\<circ>(basic ((w4\<otimes>(cement vert)) \<otimes> (cement cup)))\<circ>((basic (w4\<otimes>(cement cap)\<otimes>(cement vert)))\<circ>z1)))"
  using step3_subresult17
 by metis
 
 have step3: "tanglerel_equiv 
-(Abs_diagram ((x1)\<circ>(basic (y1 \<otimes> e_cup))\<circ>(basic (?z4\<otimes>e_vert\<otimes>e_vert))\<circ>((basic (w4\<otimes>e_cap\<otimes>e_vert))\<circ>z1)))
-(Abs_diagram ((x1)\<circ>(basic y1)\<circ>(basic ((?z4) \<otimes> e_cup))\<circ>((basic (w4\<otimes>e_cap\<otimes>e_vert))\<circ>z1)))"
+(Abs_diagram ((x1)\<circ>(basic (y1 \<otimes> (cement cup)))\<circ>(basic (?z4\<otimes>(cement vert)\<otimes>(cement vert)))\<circ>((basic (w4\<otimes>(cement cap)\<otimes>(cement vert)))\<circ>z1)))
+(Abs_diagram ((x1)\<circ>(basic y1)\<circ>(basic ((?z4) \<otimes> (cement cup)))\<circ>((basic (w4\<otimes>(cement cap)\<otimes>(cement vert)))\<circ>z1)))"
 using step3_subresult18 leftright_associativity w_subst step2_subresult1 left_associativity
  compose_leftassociativity
 by metis
 
 (*step 4*)
 
-let ?p = "(x1)\<circ>(basic (y1 \<otimes> e_cup))"
-let ?q = "(basic (w4\<otimes>e_cap\<otimes>e_vert))\<circ>z1"
-let ?r = " basic (?z4 \<otimes> e_vert \<otimes> e_vert)"
+let ?p = "(x1)\<circ>(basic (y1 \<otimes> (cement cup)))"
+let ?q = "(basic (w4\<otimes>(cement cap)\<otimes>(cement vert)))\<circ>z1"
+let ?r = " basic (?z4 \<otimes> (cement vert) \<otimes> (cement vert))"
 
-have step4_subresult1: "strands (?z4 \<otimes> e_vert \<otimes> e_vert)"
-using assms  Tangles.append.append_Nil e_vert_def preliminary_result3 step2_subresult1 strands.simps(2)
+have step4_subresult1: "strands (?z4 \<otimes> (cement vert) \<otimes> (cement vert))"
+using assms  Tangles.append.append_Nil preliminary_result3 step2_subresult1 strands.simps(2)
 leftright_associativity test_0
 by (metis)
 
-have step4_subresult2: "snd (count (y1\<otimes>e_cup)) =  snd (count (y1)) + 2"
+have step4_subresult2: "snd (count (y1\<otimes>(cement cup))) =  snd (count (y1)) + 2"
 apply (induct_tac y1)
 apply (auto)
-apply(simp add: e_cup_def count_def brickcount_def)
 done
 
-have step4_subresult4: "snd (count (y1 \<otimes> e_cup)) > snd (count (y1))"
+have step4_subresult4: "snd (count (y1 \<otimes> (cement cup))) > snd (count (y1))"
 using step4_subresult2 add_strict_increasing dbl_def 
 dbl_simps(3) order_refl zero_less_two
 by auto
 
-have step4_subresult5: "snd (count (y1 \<otimes> e_cup)) > 1"
+have step4_subresult5: "snd (count (y1 \<otimes> (cement cup))) > 1"
 using step4_subresult4 assms
 by auto
 
-have step4_subresult6: "snd (wall_count ?p) = (snd (count (y1\<otimes>e_cup)))"
+have step4_subresult6: "snd (wall_count ?p) = (snd (count (y1\<otimes>(cement cup))))"
 using wall_count_def  snd_conv wall_count.simps(1) wall_count_compose
 by auto
 
@@ -1906,14 +1908,14 @@ by auto
 
 have step4_subresult8: 
 "tanglerel_compress_null 
-(Abs_diagram (?p\<circ>(basic ((?z4) \<otimes> e_vert \<otimes> e_vert))\<circ>?q))
+(Abs_diagram (?p\<circ>(basic ((?z4) \<otimes> (cement vert) \<otimes> (cement vert)))\<circ>?q))
  (Abs_diagram (?p\<circ>?q))"
 using step4_subresult1 step4_subresult7 tanglerel_compress_null_def
 by metis
 
 have step4_subresult9: 
 "tanglerel_compress
-(Abs_diagram (?p\<circ>(basic ((?z4) \<otimes> e_vert \<otimes> e_vert))\<circ>?q))
+(Abs_diagram (?p\<circ>(basic ((?z4) \<otimes> (cement vert) \<otimes> (cement vert)))\<circ>?q))
  (Abs_diagram (?p\<circ>?q))"
 using step4_subresult8 tanglerel_compress_def
 by auto
@@ -1922,7 +1924,7 @@ by auto
 have step4_subresult10: 
 "tanglerel
  (Abs_diagram (?p\<circ>?q))
-(Abs_diagram (?p\<circ>(basic (?z4 \<otimes> e_vert \<otimes> e_vert))\<circ>?q))
+(Abs_diagram (?p\<circ>(basic (?z4 \<otimes> (cement vert) \<otimes> (cement vert)))\<circ>?q))
 "
 using step4_subresult9 step4_subresult8 tanglerel_def
 by auto
@@ -1931,7 +1933,7 @@ by auto
 have step4_subresult11: 
 "tanglerel_equiv
  (Abs_diagram (?p\<circ>?q))
-(Abs_diagram (?p\<circ>(basic ((?z4) \<otimes> e_vert \<otimes> e_vert))\<circ>?q))
+(Abs_diagram (?p\<circ>(basic ((?z4) \<otimes> (cement vert) \<otimes> (cement vert)))\<circ>?q))
 "
 using step4_subresult10 tanglerel_equiv_def compose_leftassociativity 
 leftright_associativity r_into_rtranclp step3_subresult11 step3_subresult13
@@ -1939,8 +1941,8 @@ by metis
 
 have step4: 
 "tanglerel_equiv
- (Abs_diagram ((x1)\<circ>(basic (y1 \<otimes> e_cup))\<circ>(basic (w4\<otimes>e_cap\<otimes>e_vert))\<circ>z1))
-(Abs_diagram ((x1)\<circ>(basic (y1\<otimes>e_cup))\<circ>(basic (?z4\<otimes>e_vert \<otimes> e_vert))\<circ>(basic (w4\<otimes>e_cap\<otimes>e_vert))\<circ>z1))
+ (Abs_diagram ((x1)\<circ>(basic (y1 \<otimes> (cement cup)))\<circ>(basic (w4\<otimes>(cement cap)\<otimes>(cement vert)))\<circ>z1))
+(Abs_diagram ((x1)\<circ>(basic (y1\<otimes>(cement cup)))\<circ>(basic (?z4\<otimes>(cement vert) \<otimes> (cement vert)))\<circ>(basic (w4\<otimes>(cement cap)\<otimes>(cement vert)))\<circ>z1))
 "
 using step4_subresult10 tanglerel_equiv_def compose_leftassociativity 
 leftright_associativity r_into_rtranclp step3_subresult11 step3_subresult13
@@ -1948,12 +1950,12 @@ by metis
 (*combining steps*)
                    
 have combine_vert: 
-"tanglerel_equiv (Abs_diagram (x1\<circ>basic y1\<circ>(basic (?z4\<otimes>e_cup))\<circ>(basic (w4\<otimes>e_cap\<otimes>e_vert))\<circ>z1))
+"tanglerel_equiv (Abs_diagram (x1\<circ>basic y1\<circ>(basic (?z4\<otimes>(cement cup)))\<circ>(basic (w4\<otimes>(cement cap)\<otimes>(cement vert)))\<circ>z1))
                             (Abs_diagram (x1 \<circ> basic y1 \<circ>z1))" 
                using step1 step2 rtranclp_trans tanglerel_equiv_def by metis
 have combine_cup:
 "tanglerel_equiv 
-(Abs_diagram ((x1)\<circ>(basic (y1 \<otimes> e_cup))\<circ>(basic (?z4\<otimes>e_vert\<otimes>e_vert))\<circ>((basic (w4\<otimes>e_cap\<otimes>e_vert))\<circ>z1)))
+(Abs_diagram ((x1)\<circ>(basic (y1 \<otimes> (cement cup)))\<circ>(basic (?z4\<otimes>(cement vert)\<otimes>(cement vert)))\<circ>((basic (w4\<otimes>(cement cap)\<otimes>(cement vert)))\<circ>z1)))
    (Abs_diagram (x1 \<circ> basic y1 \<circ>z1))" 
                using step3 combine_vert tanglerel_equiv_def rtranclp_trans
                 compose_leftassociativity leftright_associativity 
@@ -1962,13 +1964,14 @@ have combine_cup:
                by (metis) 
 
 have combine_compress:
-"tanglerel_equiv (Abs_diagram ((x1)\<circ>(basic (y1 \<otimes> e_cup))\<circ>(basic (w4\<otimes>e_cap\<otimes>e_vert))\<circ>z1))
+"tanglerel_equiv (Abs_diagram ((x1)\<circ>(basic (y1 \<otimes> (cement cup)))\<circ>(basic (w4\<otimes>(cement cap)\<otimes>(cement vert)))\<circ>z1))
  (Abs_diagram (x1 \<circ> basic y1 \<circ>z1))"
 using  combine_cup step4  rtranclp_trans  combine_vert tanglerel_equiv_def rtranclp_trans
                 compose_leftassociativity leftright_associativity 
                step2 step2_subresult1 step2_subresult2 step3_subresult17 subresult_equiv3 
                w_subst
-           by (metis (full_types) C nat_add_commute r_into_rtranclp step3_subresult16 step4_subresult10 test_0 test_1 wall_count.simps(1))
+           by (metis (full_types) C nat_add_commute r_into_rtranclp step3_subresult16 
+step4_subresult10 test_0 test_1 wall_count.simps(1))
 from combine_compress show ?thesis by simp
 qed
 
@@ -1977,7 +1980,7 @@ qed
 theorem metaequivalence_bottomright: 
 assumes "(fst (count y1))>1"
 and "w4 = makestrand  (nat ((fst (count y1)) + (-2)))" and "well_defined (x1 \<circ> basic y1 \<circ>z1)"
-shows "tanglerel_equiv (Abs_diagram ((x1)\<circ>(basic (w4\<otimes>e_cup\<otimes>e_vert)\<circ>(basic (y1\<otimes>e_cap))\<circ>z1)))     
+shows "tanglerel_equiv (Abs_diagram ((x1)\<circ>(basic (w4\<otimes>(cement cup)\<otimes>(cement vert))\<circ>(basic (y1\<otimes>(cement cap)))\<circ>z1)))     
 (Abs_diagram (x1 \<circ> (basic y1) \<circ>z1))" 
 proof-
 let ?z4 = "makestrand (nat ((fst (wall_count (basic y1))) + (-2))+1)"
@@ -2065,33 +2068,33 @@ have step1:
 (*need to edit from here*)
 have w_subst: "w4 = (makestrand ?k)" using assms by auto
 
-have step2_subresult0: "(makestrand (?k+1)) = ((makestrand ?k) \<otimes>e_vert)" 
+have step2_subresult0: "(makestrand (?k+1)) = ((makestrand ?k) \<otimes>(cement vert))" 
  by (metis test_00 test_1)
  
-have step2_subresult1:"?z4 = (makestrand ?k)\<otimes>e_vert  " using C step2_subresult0 by auto
+have step2_subresult1:"?z4 = (makestrand ?k)\<otimes>(cement vert)  " using C step2_subresult0 by auto
 
 have step2_subresult2: "(Abs_diagram (x1 \<circ> (basic ?z4) \<circ>(basic ?z4)\<circ> (basic y1)\<circ>z1)) =
-(Abs_diagram (x1  \<circ> (basic (w4\<otimes>e_vert))\<circ> (basic (w4\<otimes>e_vert))\<circ>(basic y1)\<circ> z1))" 
+(Abs_diagram (x1  \<circ> (basic (w4\<otimes>(cement vert)))\<circ> (basic (w4\<otimes>(cement vert)))\<circ>(basic y1)\<circ> z1))" 
                         using w_subst step2_subresult1 by auto
 
 have step2_subresult3: "(snd (count w4)) = (fst (count w4))" using makestrand_fstsndequality w_subst
 by auto
 let ?z3 = " (basic y1)\<circ> z1"
-let ?x = "(Abs_diagram (x1 \<circ>(basic (w4\<otimes>e_cup\<otimes>e_vert))\<circ>(basic (w4\<otimes>e_vert\<otimes>e_cap))\<circ>(?z3)))"
-let ?y = "(Abs_diagram (x1 \<circ>(basic (w4\<otimes>e_vert))\<circ>(basic (w4\<otimes>e_vert))\<circ> (?z3)))"
+let ?x = "(Abs_diagram (x1 \<circ>(basic (w4\<otimes>(cement cup)\<otimes>(cement vert)))\<circ>(basic (w4\<otimes>(cement vert)\<otimes>(cement cap)))\<circ>(?z3)))"
+let ?y = "(Abs_diagram (x1 \<circ>(basic (w4\<otimes>(cement vert)))\<circ>(basic (w4\<otimes>(cement vert)))\<circ> (?z3)))"
 
 have step2_subresult4:
-"\<exists>a.\<exists>b.\<exists>c.\<exists>d.(?x = Abs_diagram (a \<circ> (basic (b\<otimes>e_cup\<otimes>e_vert )) \<circ> (basic (c\<otimes>e_vert\<otimes>e_cap)) \<circ> d))"
+"\<exists>a.\<exists>b.\<exists>c.\<exists>d.(?x = Abs_diagram (a \<circ> (basic (b\<otimes>(cement cup)\<otimes>(cement vert) )) \<circ> (basic (c\<otimes>(cement vert)\<otimes>(cement cap))) \<circ> d))"
   using exI by auto
  
 have step2_subresult5:
-"\<exists>a.\<exists>b.\<exists>c.\<exists>d.(?y = Abs_diagram (a \<circ> (basic (b\<otimes>e_vert)) \<circ> (basic (c\<otimes>e_vert)) \<circ> d))"
+"\<exists>a.\<exists>b.\<exists>c.\<exists>d.(?y = Abs_diagram (a \<circ> (basic (b\<otimes>(cement vert))) \<circ> (basic (c\<otimes>(cement vert))) \<circ> d))"
  using exI by auto
 
 have step2_subresult6: 
 " (\<exists>a.\<exists>b.\<exists>c.\<exists>d.((?x = Abs_diagram ((a)
-\<circ> (basic (b\<otimes>e_cup\<otimes>e_vert)) \<circ> (basic (c\<otimes>e_vert\<otimes>e_cap)) \<circ> d)))
-\<and>(?y = Abs_diagram (a \<circ> (basic (b\<otimes>e_vert)) \<circ> (basic (c\<otimes>e_vert)) \<circ> d))
+\<circ> (basic (b\<otimes>(cement cup)\<otimes>(cement vert))) \<circ> (basic (c\<otimes>(cement vert)\<otimes>(cement cap))) \<circ> d)))
+\<and>(?y = Abs_diagram (a \<circ> (basic (b\<otimes>(cement vert))) \<circ> (basic (c\<otimes>(cement vert))) \<circ> d))
  \<and> ((snd (count b)) = (fst (count c))))"
 using  step2_subresult3 step2_subresult4 step2_subresult5 exI 
 by auto
@@ -2107,25 +2110,25 @@ have step2_subresult8:"tanglerel ?x ?y"
 using tanglerel_def tanglerel_straighten_def step2_subresult7 by auto
 
 have step2_subresult9: "tanglerel 
-              (Abs_diagram ((x1) \<circ>(basic (w4\<otimes>e_cup\<otimes>e_vert))\<circ>(basic (w4\<otimes>e_vert\<otimes>e_cap))\<circ>(?z3))) 
-              (Abs_diagram ((x1) \<circ>(basic (w4\<otimes>e_vert))\<circ>(basic (w4\<otimes>e_vert))\<circ>(?z3)))"
+              (Abs_diagram ((x1) \<circ>(basic (w4\<otimes>(cement cup)\<otimes>(cement vert)))\<circ>(basic (w4\<otimes>(cement vert)\<otimes>(cement cap)))\<circ>(?z3))) 
+              (Abs_diagram ((x1) \<circ>(basic (w4\<otimes>(cement vert)))\<circ>(basic (w4\<otimes>(cement vert)))\<circ>(?z3)))"
                using step2_subresult8 by auto
 
 have step2_subresult10: "tanglerel_equiv 
-              (Abs_diagram ((x1) \<circ>(basic (w4\<otimes>e_cup\<otimes>e_vert))\<circ>(basic (w4\<otimes>e_vert\<otimes>e_cap))\<circ>((basic y1)\<circ> z1))) 
-              (Abs_diagram ((x1) \<circ>(basic (w4\<otimes>e_vert))\<circ>(basic (w4\<otimes>e_vert))\<circ>((basic y1)\<circ> z1)))"
+              (Abs_diagram ((x1) \<circ>(basic (w4\<otimes>(cement cup)\<otimes>(cement vert)))\<circ>(basic (w4\<otimes>(cement vert)\<otimes>(cement cap)))\<circ>((basic y1)\<circ> z1))) 
+              (Abs_diagram ((x1) \<circ>(basic (w4\<otimes>(cement vert)))\<circ>(basic (w4\<otimes>(cement vert)))\<circ>((basic y1)\<circ> z1)))"
                using step2_subresult9 compose_leftassociativity r_into_rtranclp 
                tanglerel_equiv_def
                      by metis
 
 have step2_subresult11: "tanglerel_equiv 
-              (Abs_diagram ((x1) \<circ>(basic (w4\<otimes>e_cup\<otimes>e_vert))\<circ>(basic (w4\<otimes>e_vert\<otimes>e_cap))\<circ>(basic y1)\<circ> z1)) 
+              (Abs_diagram ((x1) \<circ>(basic (w4\<otimes>(cement cup)\<otimes>(cement vert)))\<circ>(basic (w4\<otimes>(cement vert)\<otimes>(cement cap)))\<circ>(basic y1)\<circ> z1)) 
               (Abs_diagram ((x1) \<circ>(basic (?z4))\<circ>(basic (?z4))\<circ>((basic y1)\<circ> z1)))"
                using step2_subresult10 step2_subresult1 w_subst
                      by (auto)
 
 have step2: "tanglerel_equiv 
-              (Abs_diagram ((x1) \<circ>(basic (w4\<otimes>e_cup\<otimes>e_vert))\<circ>(basic (?z4\<otimes>e_cap))\<circ>(basic y1)\<circ> z1)) 
+              (Abs_diagram ((x1) \<circ>(basic (w4\<otimes>(cement cup)\<otimes>(cement vert)))\<circ>(basic (?z4\<otimes>(cement cap)))\<circ>(basic y1)\<circ> z1)) 
               (Abs_diagram ((x1) \<circ>(basic (?z4))\<circ>(basic (?z4))\<circ>((basic y1)\<circ> z1)))"
                using step2_subresult11 step2_subresult1 
                    Tangle.abs_eq_iff compose_Nil leftright_associativity 
@@ -2137,22 +2140,22 @@ have step3_subresult1 :
 "snd (count  ?z4) = fst (count y1) " 
 using assms preliminary_result6 subresult8
 by auto
-have step3_subresult2: "snd (count e_cap) = 0" using e_cup_def count_def brickcount_def 
- brickcount.simps(3) count.simps(1) e_cap_def snd_conv
+have step3_subresult2: "snd (count (cement cap)) = 0" using  count_def brickcount_def 
+ brickcount.simps(3) count.simps(1) snd_conv
 by (metis)
 
-have step3_subresult3: "strands (vert#e_vert)" using e_vert_def append_def strands_def  brickstrand.simps(1) 
+have step3_subresult3: "strands (vert#(cement vert))" using append_def strands_def  brickstrand.simps(1) 
                         strands.simps(1) strands.simps(2) 
                        by metis
-have step3_subresult4: "(vert#e_vert) = (e_vert\<otimes>e_vert)" using append_Nil e_vert_def
+have step3_subresult4: "(vert#(cement vert)) = ((cement vert)\<otimes>(cement vert))" using append_Nil 
                         by metis
-have step3_subresult5: "strands (e_vert\<otimes>e_vert)" using step3_subresult3 step3_subresult4
-                        by auto
+have step3_subresult5: "strands ((cement vert)\<otimes>(cement vert))" using step3_subresult3 step3_subresult4
+                        by metis
 
 let  ?a = 
-"Abs_diagram (((x1) \<circ>(basic (w4\<otimes>e_cup\<otimes>e_vert)))\<circ>(basic (?z4\<otimes>e_vert\<otimes>e_vert))\<circ>(basic (y1\<otimes>e_cap))\<circ> z1) "
+"Abs_diagram (((x1) \<circ>(basic (w4\<otimes>(cement cup)\<otimes>(cement vert))))\<circ>(basic (?z4\<otimes>(cement vert)\<otimes>(cement vert)))\<circ>(basic (y1\<otimes>(cement cap)))\<circ> z1) "
 
-let ?b = " (Abs_diagram (((x1) \<circ>(basic (w4\<otimes>e_cup\<otimes>e_vert)))\<circ>(basic (?z4\<otimes>e_cap))\<circ>(basic y1)\<circ> z1)) "
+let ?b = " (Abs_diagram (((x1) \<circ>(basic (w4\<otimes>(cement cup)\<otimes>(cement vert))))\<circ>(basic (?z4\<otimes>(cement cap)))\<circ>(basic y1)\<circ> z1)) "
  
 have step3_subresult6: " \<exists>a1.\<exists>b1.\<exists>b2.\<exists>A.\<exists>B.\<exists>a2.(?a = Abs_diagram
  ((a1)\<circ>(basic (b1\<otimes>A))\<circ>(basic (b2\<otimes>B))\<circ>(a2)))"
@@ -2198,50 +2201,49 @@ have step3_subresult13: "tanglerel_equiv ?a ?b"
        by (metis (full_types) r_into_rtranclp)
 
 have step3: "tanglerel_equiv
-(Abs_diagram (((x1) \<circ>(basic (w4\<otimes>e_cup\<otimes>e_vert)))\<circ>(basic (?z4\<otimes>e_vert\<otimes>e_vert))\<circ>(basic (y1\<otimes>e_cap))\<circ> z1))
-(Abs_diagram (((x1) \<circ>(basic (w4\<otimes>e_cup\<otimes>e_vert)))\<circ>(basic (?z4\<otimes>e_cap))\<circ>(basic y1)\<circ> z1)) "
+(Abs_diagram (((x1) \<circ>(basic (w4\<otimes>(cement cup)\<otimes>(cement vert))))\<circ>(basic (?z4\<otimes>(cement vert)\<otimes>(cement vert)))\<circ>(basic (y1\<otimes>(cement cap)))\<circ> z1))
+(Abs_diagram (((x1) \<circ>(basic (w4\<otimes>(cement cup)\<otimes>(cement vert))))\<circ>(basic (?z4\<otimes>(cement cap)))\<circ>(basic y1)\<circ> z1)) "
  using step3_subresult13 by auto
 
 (*step 4*)
 
-let ?p = "(x1)\<circ>(basic (w4\<otimes>e_cup\<otimes>e_vert))"
-let ?q = "(basic (y1 \<otimes> e_cap))\<circ>z1"
-let ?r = " basic (?z4 \<otimes> e_vert \<otimes> e_vert)"
+let ?p = "(x1)\<circ>(basic (w4\<otimes>(cement cup)\<otimes>(cement vert)))"
+let ?q = "(basic (y1 \<otimes> (cement cap)))\<circ>z1"
+let ?r = " basic (?z4 \<otimes> (cement vert) \<otimes> (cement vert))"
 
-have step4_subresult1: "strands (?z4 \<otimes> e_vert \<otimes> e_vert)"
-using assms  Tangles.append.append_Nil e_vert_def preliminary_result3 step2_subresult1 strands.simps(2)
+have step4_subresult1: "strands (?z4 \<otimes> (cement vert) \<otimes> (cement vert))"
+using assms  Tangles.append.append_Nil  preliminary_result3 step2_subresult1 strands.simps(2)
 leftright_associativity test_0 strand_makestrand wall_count.simps(1)
 by (metis )
 
-have step4_subresult2: "fst (count (y1\<otimes>e_cap)) =  fst (count (y1)) + 2"
+have step4_subresult2: "fst (count (y1\<otimes>(cement cap))) =  fst (count (y1)) + 2"
 apply (induct_tac y1)
 apply (auto)
-apply(simp add: e_cap_def)
 done
 
-have step4_subresult4: "fst (count (y1 \<otimes> e_cap)) = fst (count (y1))+2"
+have step4_subresult4: "fst (count (y1 \<otimes> (cement cap))) = fst (count (y1))+2"
 using step4_subresult2 add_strict_increasing dbl_def 
 dbl_simps(3) order_refl zero_less_two
 by auto
 
-have step4_subresult5: "fst (count (y1 \<otimes> e_cap)) > 1"
+have step4_subresult5: "fst (count (y1 \<otimes> (cement cap))) > 1"
 using step4_subresult4 assms
 by auto
 
-have step4_subresult6: "snd (wall_count ?p) = snd (count (w4\<otimes>e_cup\<otimes>e_vert))"
+have step4_subresult6: "snd (wall_count ?p) = snd (count (w4\<otimes>(cement cup)\<otimes>(cement vert)))"
 using wall_count_def  snd_conv wall_count.simps(1) wall_count_compose
 by auto
 
-have step4_subresult7: "snd (count (x\<otimes>e_vert)) >0 "
-using snd_count_positive e_vert_def brickcount_def count_def 
+have step4_subresult7: "snd (count (x\<otimes>(cement vert))) >0 "
+using snd_count_positive  brickcount_def count_def 
 makestrand.simps(1) makestrand_fstsndequality makestrands_positivelength
 by (metis add_nonneg_eq_0_iff less_le snd_count_additive snd_count_nonnegative)
 
 
-have step4_subresult8: "snd (count ((w4\<otimes>e_cup)\<otimes>e_vert)) > 0"
+have step4_subresult8: "snd (count ((w4\<otimes>(cement cup))\<otimes>(cement vert))) > 0"
 using step4_subresult7
 by (metis add_nonneg_eq_0_iff brick.distinct(1) brickcount_zero_implies_cup count.simps(1) 
-e_vert_def le_neq_trans makestrand.simps(1) makestrand_fstsndequality snd_count_additive snd_count_nonnegative)
+le_neq_trans makestrand.simps(1) makestrand_fstsndequality snd_count_additive snd_count_nonnegative)
 
 
 have step4_subresult9: "snd (wall_count ?p) > 0"
@@ -2272,15 +2274,15 @@ by auto
 
 have step4_subresult13:
 "tanglerel
-(Abs_diagram ((x1)\<circ>(basic (w4\<otimes>e_cup\<otimes>e_vert))\<circ>(basic (?z4 \<otimes> e_vert \<otimes> e_vert))\<circ>(basic (y1 \<otimes> e_cap))\<circ>z1))
- (Abs_diagram ((x1)\<circ>(basic (w4\<otimes>e_cup\<otimes>e_vert))\<circ>(basic (y1 \<otimes> e_cap))\<circ>z1))"
+(Abs_diagram ((x1)\<circ>(basic (w4\<otimes>(cement cup)\<otimes>(cement vert)))\<circ>(basic (?z4 \<otimes> (cement vert) \<otimes> (cement vert)))\<circ>(basic (y1 \<otimes> (cement cap)))\<circ>z1))
+ (Abs_diagram ((x1)\<circ>(basic (w4\<otimes>(cement cup)\<otimes>(cement vert)))\<circ>(basic (y1 \<otimes> (cement cap)))\<circ>z1))"
 using step4_subresult12 
 by (metis compose_leftassociativity tanglerel_def)
 
 have step4: 
 "tanglerel_equiv
-(Abs_diagram ((x1)\<circ>(basic (w4\<otimes>e_cup\<otimes>e_vert))\<circ>(basic (?z4 \<otimes> e_vert \<otimes> e_vert))\<circ>(basic (y1 \<otimes> e_cap))\<circ>z1))
- (Abs_diagram ((x1)\<circ>(basic (w4\<otimes>e_cup\<otimes>e_vert))\<circ>(basic (y1 \<otimes> e_cap))\<circ>z1))"
+(Abs_diagram ((x1)\<circ>(basic (w4\<otimes>(cement cup)\<otimes>(cement vert)))\<circ>(basic (?z4 \<otimes> (cement vert) \<otimes> (cement vert)))\<circ>(basic (y1 \<otimes> (cement cap)))\<circ>z1))
+ (Abs_diagram ((x1)\<circ>(basic (w4\<otimes>(cement cup)\<otimes>(cement vert)))\<circ>(basic (y1 \<otimes> (cement cap)))\<circ>z1))"
 using step4_subresult10 tanglerel_equiv_def compose_leftassociativity 
 leftright_associativity r_into_rtranclp step3_subresult11 step4_subresult12 step4_subresult13
 by (metis (full_types))
@@ -2288,13 +2290,13 @@ by (metis (full_types))
 (*combining steps*)
                       
 have combine_vert: 
-"tanglerel_equiv    (Abs_diagram ((x1) \<circ>(basic (w4\<otimes>e_cup\<otimes>e_vert))\<circ>(basic (?z4\<otimes>e_cap))\<circ>(basic y1)\<circ> z1)) 
+"tanglerel_equiv    (Abs_diagram ((x1) \<circ>(basic (w4\<otimes>(cement cup)\<otimes>(cement vert)))\<circ>(basic (?z4\<otimes>(cement cap)))\<circ>(basic y1)\<circ> z1)) 
                    (Abs_diagram (x1 \<circ> basic y1 \<circ>z1))" 
                using step1 step2 rtranclp_trans tanglerel_equiv_def by metis
 
 have combine_cup:
 "tanglerel_equiv 
-   (Abs_diagram (((x1) \<circ>(basic (w4\<otimes>e_cup\<otimes>e_vert)))\<circ>(basic (?z4\<otimes>e_vert\<otimes>e_vert))\<circ>(basic (y1\<otimes>e_cap))\<circ> z1))
+   (Abs_diagram (((x1) \<circ>(basic (w4\<otimes>(cement cup)\<otimes>(cement vert))))\<circ>(basic (?z4\<otimes>(cement vert)\<otimes>(cement vert)))\<circ>(basic (y1\<otimes>(cement cap)))\<circ> z1))
    (Abs_diagram (x1 \<circ> basic y1 \<circ>z1))" 
                using step3 combine_vert tanglerel_equiv_def rtranclp_trans
                 compose_leftassociativity leftright_associativity 
@@ -2303,9 +2305,9 @@ have combine_cup:
                by (metis) 
 have combine_compress:
 "tanglerel_equiv
-(Abs_diagram ((x1)\<circ>(basic (w4\<otimes>e_cup\<otimes>e_vert))\<circ>(basic (y1 \<otimes> e_cap))\<circ>z1))
+(Abs_diagram ((x1)\<circ>(basic (w4\<otimes>(cement cup)\<otimes>(cement vert)))\<circ>(basic (y1 \<otimes> (cement cap)))\<circ>z1))
  (Abs_diagram ((x1)\<circ>(basic y1)\<circ>z1))"
-using combine_cup step4 rtranclp_trans  combine_cup step4  rtranclp_trans  combine_vert tanglerel_equiv_def 
+using combine_cup step4 rtranclp_trans  combine_cup step4  rtranclp_trans  tanglerel_equiv_def 
                 compose_leftassociativity leftright_associativity 
                step2 step2_subresult1 step2_subresult2  subresult_equiv3 
                w_subst
@@ -2317,7 +2319,7 @@ qed
 theorem metaequivalence_bottomleft: 
 assumes "(fst (count y1))>1"
 and "w4 = makestrand  (nat ((fst (count y1)) + (-2)))" and "well_defined (x1 \<circ> basic y1 \<circ>z1)"
-shows "tanglerel_equiv (Abs_diagram ((x1)\<circ>(basic (e_vert\<otimes>e_cup\<otimes>w4)\<circ>(basic (e_cap\<otimes>y1))\<circ>z1)))    
+shows "tanglerel_equiv (Abs_diagram ((x1)\<circ>(basic ((cement vert)\<otimes>(cement cup)\<otimes>w4)\<circ>(basic ((cement cap)\<otimes>y1))\<circ>z1)))    
  (Abs_diagram (x1 \<circ> (basic y1) \<circ>z1))" 
 proof-
 let ?z4 ="makestrand (nat ((fst (wall_count (basic y1))) + (-2))+1)"
@@ -2403,33 +2405,33 @@ have step1:
 (*need to edit from here*)
 have w_subst: "w4 = (makestrand ?k)" using assms by auto
 
-have step2_subresult0: "(makestrand (?k+1)) = (e_vert\<otimes>(makestrand ?k))" 
+have step2_subresult0: "(makestrand (?k+1)) = ((cement vert)\<otimes>(makestrand ?k))" 
  by (metis test_0)
  
-have step2_subresult1:"?z4 = e_vert \<otimes>(makestrand ?k)  " using C step2_subresult0 by auto
+have step2_subresult1:"?z4 = (cement vert) \<otimes>(makestrand ?k)  " using C step2_subresult0 by auto
                             
 have step2_subresult2: "(Abs_diagram (x1 \<circ> (basic ?z4) \<circ>(basic ?z4)\<circ> (basic y1)\<circ>z1)) =
-(Abs_diagram (x1  \<circ> (basic (e_vert \<otimes>w4))\<circ> (basic (e_vert \<otimes>w4))\<circ>(basic y1)\<circ> z1))" 
+(Abs_diagram (x1  \<circ> (basic ((cement vert) \<otimes>w4))\<circ> (basic ((cement vert) \<otimes>w4))\<circ>(basic y1)\<circ> z1))" 
                         using w_subst step2_subresult1 by auto
 
 have step2_subresult3: "(snd (count w4)) = (fst (count w4))" using makestrand_fstsndequality w_subst
 by auto
 let ?z3 = " (basic y1)\<circ> z1"
-let ?x = "(Abs_diagram (x1 \<circ>(basic (e_vert\<otimes>e_cup\<otimes>w4))\<circ>(basic (e_cap\<otimes>e_vert\<otimes>w4))\<circ>(?z3)))"
-let ?y = "(Abs_diagram (x1 \<circ>(basic (e_vert\<otimes>w4))\<circ>(basic (e_vert\<otimes>w4))\<circ> (?z3)))"
+let ?x = "(Abs_diagram (x1 \<circ>(basic ((cement vert)\<otimes>(cement cup)\<otimes>w4))\<circ>(basic ((cement cap)\<otimes>(cement vert)\<otimes>w4))\<circ>(?z3)))"
+let ?y = "(Abs_diagram (x1 \<circ>(basic ((cement vert)\<otimes>w4))\<circ>(basic ((cement vert)\<otimes>w4))\<circ> (?z3)))"
 
 have step2_subresult4:
-"\<exists>a.\<exists>b.\<exists>c.\<exists>d.(?x = Abs_diagram (a \<circ> (basic (e_vert\<otimes>e_cup\<otimes>b )) \<circ> (basic (e_cap\<otimes>e_vert\<otimes>c)) \<circ> d))"
+"\<exists>a.\<exists>b.\<exists>c.\<exists>d.(?x = Abs_diagram (a \<circ> (basic ((cement vert)\<otimes>(cement cup)\<otimes>b )) \<circ> (basic ((cement cap)\<otimes>(cement vert)\<otimes>c)) \<circ> d))"
   using exI by auto
  
 have step2_subresult5:
-"\<exists>a.\<exists>b.\<exists>c.\<exists>d.(?y = Abs_diagram (a \<circ> (basic (e_vert\<otimes>b)) \<circ> (basic (e_vert\<otimes>c)) \<circ> d))"
+"\<exists>a.\<exists>b.\<exists>c.\<exists>d.(?y = Abs_diagram (a \<circ> (basic ((cement vert)\<otimes>b)) \<circ> (basic ((cement vert)\<otimes>c)) \<circ> d))"
  using exI by auto
 
 have step2_subresult6: 
 " (\<exists>a.\<exists>b.\<exists>c.\<exists>d.((?x = Abs_diagram ((a)
-\<circ> (basic (e_vert\<otimes>e_cup\<otimes>b)) \<circ> (basic (e_cap\<otimes>e_vert\<otimes>c)) \<circ> d)))
-\<and>(?y = Abs_diagram (a \<circ> (basic (e_vert\<otimes>b)) \<circ> (basic (e_vert\<otimes>c)) \<circ> d))
+\<circ> (basic ((cement vert)\<otimes>(cement cup)\<otimes>b)) \<circ> (basic ((cement cap)\<otimes>(cement vert)\<otimes>c)) \<circ> d)))
+\<and>(?y = Abs_diagram (a \<circ> (basic ((cement vert)\<otimes>b)) \<circ> (basic ((cement vert)\<otimes>c)) \<circ> d))
  \<and> ((snd (count b)) = (fst (count c))))"
 using  step2_subresult3 step2_subresult4 step2_subresult5 exI 
 by auto
@@ -2445,25 +2447,25 @@ have step2_subresult8:"tanglerel ?x ?y"
 using tanglerel_def tanglerel_straighten_def step2_subresult7 by auto
 
 have step2_subresult9: "tanglerel 
-              (Abs_diagram ((x1) \<circ>(basic (e_vert\<otimes>e_cup\<otimes>w4))\<circ>(basic (e_cap\<otimes>e_vert\<otimes> w4))\<circ>(?z3))) 
-              (Abs_diagram ((x1) \<circ>(basic (e_vert\<otimes>w4))\<circ>(basic (e_vert \<otimes>w4))\<circ>(?z3)))"
+              (Abs_diagram ((x1) \<circ>(basic ((cement vert)\<otimes>(cement cup)\<otimes>w4))\<circ>(basic ((cement cap)\<otimes>(cement vert)\<otimes> w4))\<circ>(?z3))) 
+              (Abs_diagram ((x1) \<circ>(basic ((cement vert)\<otimes>w4))\<circ>(basic ((cement vert) \<otimes>w4))\<circ>(?z3)))"
                using step2_subresult8 by auto
 
 have step2_subresult10: "tanglerel_equiv 
-              (Abs_diagram ((x1) \<circ>(basic (e_vert\<otimes>e_cup\<otimes>w4))\<circ>(basic (e_cap\<otimes>e_vert\<otimes>w4))\<circ>((basic y1)\<circ> z1))) 
-              (Abs_diagram ((x1) \<circ>(basic (e_vert\<otimes>w4))\<circ>(basic (e_vert\<otimes>w4))\<circ>((basic y1)\<circ> z1)))"
+              (Abs_diagram ((x1) \<circ>(basic ((cement vert)\<otimes>(cement cup)\<otimes>w4))\<circ>(basic ((cement cap)\<otimes>(cement vert)\<otimes>w4))\<circ>((basic y1)\<circ> z1))) 
+              (Abs_diagram ((x1) \<circ>(basic ((cement vert)\<otimes>w4))\<circ>(basic ((cement vert)\<otimes>w4))\<circ>((basic y1)\<circ> z1)))"
                using step2_subresult9 compose_leftassociativity r_into_rtranclp 
                tanglerel_equiv_def
                      by metis
 
 have step2_subresult11: "tanglerel_equiv 
-       (Abs_diagram ((x1) \<circ>(basic (e_vert\<otimes>e_cup\<otimes>w4))\<circ>(basic (e_cap\<otimes>e_vert\<otimes>w4))\<circ>((basic y1)\<circ> z1)))     
+       (Abs_diagram ((x1) \<circ>(basic ((cement vert)\<otimes>(cement cup)\<otimes>w4))\<circ>(basic ((cement cap)\<otimes>(cement vert)\<otimes>w4))\<circ>((basic y1)\<circ> z1)))     
               (Abs_diagram ((x1) \<circ>(basic (?z4))\<circ>(basic (?z4))\<circ>((basic y1)\<circ> z1)))"
                using step2_subresult10 step2_subresult1 w_subst
                      by (auto)
 
 have step2: "tanglerel_equiv 
-       (Abs_diagram ((x1) \<circ>(basic (e_vert\<otimes>e_cup\<otimes>w4))\<circ>(basic (e_cap\<otimes>?z4))\<circ>((basic y1)\<circ> z1)))      
+       (Abs_diagram ((x1) \<circ>(basic ((cement vert)\<otimes>(cement cup)\<otimes>w4))\<circ>(basic ((cement cap)\<otimes>?z4))\<circ>((basic y1)\<circ> z1)))      
          (Abs_diagram ((x1) \<circ>(basic (?z4))\<circ>(basic (?z4))\<circ>((basic y1)\<circ> z1)))"
                using step2_subresult11 step2_subresult1 
                    Tangle.abs_eq_iff compose_Nil leftright_associativity 
@@ -2475,21 +2477,20 @@ have step3_subresult1 :
 "snd (count  ?z4) = fst (count y1) " 
 using assms preliminary_result6 subresult8
 by auto
-have step3_subresult2: "snd (count e_cap) = 0" using e_cup_def count_def brickcount_def 
- brickcount.simps(3) count.simps(1) e_cap_def snd_conv
-by (metis)
+have step3_subresult2: "snd (count (cement cap)) = 0" using  count_def brickcount_def 
+ brickcount.simps(3) count.simps(1) snd_conv by (metis)
 
-have step3_subresult3: "strands (vert#e_vert)" using e_vert_def append_def strands_def  brickstrand.simps(1) 
+have step3_subresult3: "strands (vert#(cement vert))" using  append_def strands_def  brickstrand.simps(1) 
                         strands.simps(1) strands.simps(2) 
                        by metis
-have step3_subresult4: "(vert#e_vert) = (e_vert\<otimes>e_vert)" using append_Nil e_vert_def
+have step3_subresult4: "(vert#(cement vert)) = ((cement vert)\<otimes>(cement vert))" using append_Nil
                         by metis
-have step3_subresult5: "strands (e_vert\<otimes>e_vert)" using step3_subresult3 step3_subresult4
-                        by auto
+have step3_subresult5: "strands ((cement vert)\<otimes>(cement vert))" using step3_subresult3 step3_subresult4
+                        by metis
 
 let  ?a = 
-"Abs_diagram (((x1) \<circ>(basic (e_vert\<otimes>e_cup\<otimes>w4)))\<circ>(basic (e_vert\<otimes>e_vert\<otimes>?z4))\<circ>(basic (e_cap\<otimes>y1))\<circ> z1) "
-let ?b = " (Abs_diagram (((x1) \<circ>(basic (e_vert\<otimes>e_cup\<otimes>w4)))\<circ>(basic (e_cap\<otimes>?z4))\<circ>(basic y1)\<circ> z1)) "
+"Abs_diagram (((x1) \<circ>(basic ((cement vert)\<otimes>(cement cup)\<otimes>w4)))\<circ>(basic ((cement vert)\<otimes>(cement vert)\<otimes>?z4))\<circ>(basic ((cement cap)\<otimes>y1))\<circ> z1) "
+let ?b = " (Abs_diagram (((x1) \<circ>(basic ((cement vert)\<otimes>(cement cup)\<otimes>w4)))\<circ>(basic ((cement cap)\<otimes>?z4))\<circ>(basic y1)\<circ> z1)) "
  
 have step3_subresult6: " \<exists>a1.\<exists>b1.\<exists>b2.\<exists>A.\<exists>B.\<exists>a2.(?a = Abs_diagram
  ((a1)\<circ>(basic (A \<otimes> b1))\<circ>(basic (B \<otimes> b2))\<circ>(a2)))"
@@ -2535,53 +2536,53 @@ have step3_subresult13: "tanglerel_equiv ?a ?b"
        by (metis (full_types) r_into_rtranclp)
 
 have step3: "tanglerel_equiv
-(Abs_diagram (((x1) \<circ>(basic (e_vert\<otimes>e_cup\<otimes>w4)))\<circ>(basic (e_vert\<otimes>e_vert\<otimes>?z4))\<circ>(basic (e_cap\<otimes>y1))\<circ> z1))
-(Abs_diagram (((x1) \<circ>(basic (e_vert\<otimes>e_cup\<otimes>w4)))\<circ>(basic (e_cap \<otimes>?z4))\<circ>(basic y1)\<circ> z1)) "
+(Abs_diagram (((x1) \<circ>(basic ((cement vert)\<otimes>(cement cup)\<otimes>w4)))\<circ>(basic ((cement vert)\<otimes>(cement vert)\<otimes>?z4))\<circ>(basic ((cement cap)\<otimes>y1))\<circ> z1))
+(Abs_diagram (((x1) \<circ>(basic ((cement vert)\<otimes>(cement cup)\<otimes>w4)))\<circ>(basic ((cement cap) \<otimes>?z4))\<circ>(basic y1)\<circ> z1)) "
  using step3_subresult13 by auto
  
-(*"tanglerel_equiv (Abs_diagram ((x1)\<circ>(basic (e_vert\<otimes>e_cup\<otimes>w4)\<circ>(basic (e_vert\<otimes>e_vert\<otimes>?z4))\<circ>
-(basic (e_cap\<otimes>y1))\<circ>z1)))     (Abs_diagram (x1 \<circ> (basic y1) \<circ>z1))*)
+(*"tanglerel_equiv (Abs_diagram ((x1)\<circ>(basic ((cement vert)\<otimes>(cement cup)\<otimes>w4)\<circ>(basic ((cement vert)\<otimes>(cement vert)\<otimes>?z4))\<circ>
+(basic ((cement cap)\<otimes>y1))\<circ>z1)))     (Abs_diagram (x1 \<circ> (basic y1) \<circ>z1))*)
 
 (*step 4*)
 
-let ?p = "(x1)\<circ>(basic (e_vert\<otimes>e_cup\<otimes>w4))"
-let ?q = "(basic (e_cap \<otimes> y1))\<circ>z1"
-let ?r = " basic (e_vert \<otimes> e_vert\<otimes>?z4)"
+let ?p = "(x1)\<circ>(basic ((cement vert)\<otimes>(cement cup)\<otimes>w4))"
+let ?q = "(basic ((cement cap) \<otimes> y1))\<circ>z1"
+let ?r = " basic ((cement vert) \<otimes> (cement vert)\<otimes>?z4)"
 
-have step4_subresult1: "strands (e_vert \<otimes> e_vert\<otimes>?z4)"
-using assms  Tangles.append.append_Nil e_vert_def preliminary_result3 step2_subresult1 strands.simps(2)
+have step4_subresult1: "strands ((cement vert) \<otimes> (cement vert)\<otimes>?z4)"
+using assms  Tangles.append.append_Nil preliminary_result3 step2_subresult1 strands.simps(2)
 leftright_associativity test_0 strand_makestrand wall_count.simps(1)
 by (metis )
 
-have step4_subresult2: "fst (count (e_cap\<otimes>y1)) =  (fst (count e_cap)) + fst (count (y1)) "
+have step4_subresult2: "fst (count ((cement cap)\<otimes>y1)) =  (fst (count (cement cap))) + fst (count (y1)) "
 using fst_count_additive by auto
 
-have step4_subresult3: "fst (count (e_cap)) =  2"
-using e_cap_def count_def brickcount_def 
+have step4_subresult3: "fst (count ((cement cap))) =  2"
+using  count_def brickcount_def 
 by (metis brickcount.simps(3) count.simps(1) fst_conv)
 
-have step4_subresult4: "fst (count (e_cap\<otimes>y1)) = fst (count (y1))+2"
+have step4_subresult4: "fst (count ((cement cap)\<otimes>y1)) = fst (count (y1))+2"
 using step4_subresult2 step4_subresult3 add_strict_increasing dbl_def 
 dbl_simps(3) order_refl zero_less_two
 by auto
 
-have step4_subresult5: "fst (count (e_cap\<otimes>y1)) > 1"
+have step4_subresult5: "fst (count ((cement cap)\<otimes>y1)) > 1"
 using step4_subresult4 assms
 by auto
 
-have step4_subresult6: "snd (wall_count ?p) = snd (count (e_vert\<otimes>e_cup\<otimes>w4))"
+have step4_subresult6: "snd (wall_count ?p) = snd (count ((cement vert)\<otimes>(cement cup)\<otimes>w4))"
 using wall_count_def  snd_conv wall_count.simps(1) wall_count_compose
 by auto
 
-have step4_subresult7: "snd (count (e_vert\<otimes>x)) >0 "
-using snd_count_positive e_vert_def brickcount_def count_def 
+have step4_subresult7: "snd (count ((cement vert)\<otimes>x)) >0 "
+using snd_count_positive  brickcount_def count_def 
 makestrand.simps(1) makestrand_fstsndequality makestrands_positivelength
 by (metis add_nonneg_eq_0_iff antisym_conv1 snd_count_additive snd_count_nonnegative)
 
 
-have step4_subresult8: "snd (count (e_vert\<otimes>(e_cap\<otimes>w4))) > 0"
+have step4_subresult8: "snd (count ((cement vert)\<otimes>((cement cap)\<otimes>w4))) > 0"
 using step4_subresult7
-by (metis add_nonneg_eq_0_iff brickcount.simps(1) count.simps(1) e_vert_def le_neq_trans snd_conv
+by (metis add_nonneg_eq_0_iff brickcount.simps(1) count.simps(1) le_neq_trans snd_conv
  snd_count_additive snd_count_nonnegative zero_neq_one)
 
 have step4_subresult9: "snd (wall_count ?p) > 0"
@@ -2616,15 +2617,15 @@ by auto
 
 have step4_subresult13:
 "tanglerel
-(Abs_diagram ((x1)\<circ>(basic (e_vert\<otimes>e_cup\<otimes>w4))\<circ>(basic (e_vert\<otimes>e_vert\<otimes>?z4))\<circ>(basic (e_cap \<otimes> y1))\<circ>z1))
- (Abs_diagram ((x1)\<circ>(basic (e_vert\<otimes>e_cup\<otimes>w4))\<circ>(basic (e_cap \<otimes> y1))\<circ>z1))"
+(Abs_diagram ((x1)\<circ>(basic ((cement vert)\<otimes>(cement cup)\<otimes>w4))\<circ>(basic ((cement vert)\<otimes>(cement vert)\<otimes>?z4))\<circ>(basic ((cement cap) \<otimes> y1))\<circ>z1))
+ (Abs_diagram ((x1)\<circ>(basic ((cement vert)\<otimes>(cement cup)\<otimes>w4))\<circ>(basic ((cement cap) \<otimes> y1))\<circ>z1))"
 using step4_subresult12  compose_leftassociativity tanglerel_def
 by metis
 
 have step4: 
 "tanglerel_equiv
-(Abs_diagram ((x1)\<circ>(basic (e_vert\<otimes>e_cup\<otimes>w4))\<circ>(basic (e_cap \<otimes> y1))\<circ>z1))
-(Abs_diagram ((x1)\<circ>(basic (e_vert\<otimes>e_cup\<otimes>w4))\<circ>(basic (e_vert\<otimes>e_vert\<otimes>?z4))\<circ>(basic (e_cap \<otimes> y1))\<circ>z1))
+(Abs_diagram ((x1)\<circ>(basic ((cement vert)\<otimes>(cement cup)\<otimes>w4))\<circ>(basic ((cement cap) \<otimes> y1))\<circ>z1))
+(Abs_diagram ((x1)\<circ>(basic ((cement vert)\<otimes>(cement cup)\<otimes>w4))\<circ>(basic ((cement vert)\<otimes>(cement vert)\<otimes>?z4))\<circ>(basic ((cement cap) \<otimes> y1))\<circ>z1))
  "
 using step4_subresult10 tanglerel_equiv_def compose_leftassociativity 
 leftright_associativity r_into_rtranclp step3_subresult11 step4_subresult12 step4_subresult13
@@ -2633,15 +2634,17 @@ by (metis (full_types))
 (*combining steps*)
                       
 have combine_vert: 
-"tanglerel_equiv  (Abs_diagram (((x1) \<circ>(basic (e_vert\<otimes>e_cup\<otimes>w4)))\<circ>(basic (e_cap \<otimes>?z4))\<circ>(basic y1)\<circ> z1))
+"tanglerel_equiv  (Abs_diagram (((x1) \<circ>(basic ((cement vert)\<otimes>(cement cup)\<otimes>w4)))\<circ>(basic ((cement cap) \<otimes>?z4))\<circ>(basic y1)\<circ> z1))
                   (Abs_diagram (x1 \<circ> basic y1 \<circ>z1))" 
                using step1 step2 rtranclp_trans tanglerel_equiv_def Tangle.abs_eq_iff compose_Nil 
                compose_leftassociativity step3_subresult7 step3_subresult8
-               by (metis)
-
+                   by (metis 
+C step2_subresult0 step2_subresult10 step2_subresult2 step2_subresult4 step2_subresult5 test_0 
+test_1 w_subst)
+                     
 have combine_cup:
 "tanglerel_equiv 
- (Abs_diagram (((x1) \<circ>(basic (e_vert\<otimes>e_cup\<otimes>w4)))\<circ>(basic (e_vert\<otimes>e_vert\<otimes>?z4))\<circ>(basic (e_cap\<otimes>y1))\<circ> z1))
+ (Abs_diagram (((x1) \<circ>(basic ((cement vert)\<otimes>(cement cup)\<otimes>w4)))\<circ>(basic ((cement vert)\<otimes>(cement vert)\<otimes>?z4))\<circ>(basic ((cement cap)\<otimes>y1))\<circ> z1))
   (Abs_diagram (x1 \<circ> basic y1 \<circ>z1))" 
                using step3 combine_vert tanglerel_equiv_def rtranclp_trans
                 compose_leftassociativity leftright_associativity 
@@ -2650,9 +2653,9 @@ have combine_cup:
                by (metis) 
 have combine_compress:
 "tanglerel_equiv 
-(Abs_diagram ((x1)\<circ>(basic (e_vert\<otimes>e_cup\<otimes>w4))\<circ>(basic (e_cap \<otimes> y1))\<circ>z1))
+(Abs_diagram ((x1)\<circ>(basic ((cement vert)\<otimes>(cement cup)\<otimes>w4))\<circ>(basic ((cement cap) \<otimes> y1))\<circ>z1))
   (Abs_diagram (x1 \<circ> basic y1 \<circ>z1))"
-using combine_cup step4 rtranclp_trans  combine_cup step4  rtranclp_trans  combine_vert tanglerel_equiv_def 
+using combine_cup step4 rtranclp_trans  combine_cup step4  rtranclp_trans  tanglerel_equiv_def 
                 compose_leftassociativity leftright_associativity 
                step2 step2_subresult1 step2_subresult2  subresult_equiv3 
                w_subst
@@ -2665,17 +2668,17 @@ qed
 theorem metaequivalence_left_drop: 
 assumes "(snd (count y2))>1" and "(z4 = makestrand (nat ((snd (count y2)) + (-2))+1))"
 and "w4 = makestrand  (nat ((snd (count y2)) + (-2)))" and "fst (count y2) = snd (count y1)"
-shows "tanglerel_equiv (Abs_diagram ((x1)\<circ>(basic (e_cup\<otimes>y1))\<circ>(basic (e_vert\<otimes>e_vert\<otimes>y2))\<circ>(basic (e_vert\<otimes>e_cap\<otimes>w4))\<circ>z1))
-             (Abs_diagram (x1 \<circ> (basic y1) \<circ>(basic (e_cup\<otimes>y2))\<circ>(basic (e_vert\<otimes>e_cap\<otimes>w4))\<circ>z1))"
+shows "tanglerel_equiv (Abs_diagram ((x1)\<circ>(basic ((cement cup)\<otimes>y1))\<circ>(basic ((cement vert)\<otimes>(cement vert)\<otimes>y2))\<circ>(basic ((cement vert)\<otimes>(cement cap)\<otimes>w4))\<circ>z1))
+             (Abs_diagram (x1 \<circ> (basic y1) \<circ>(basic ((cement cup)\<otimes>y2))\<circ>(basic ((cement vert)\<otimes>(cement cap)\<otimes>w4))\<circ>z1))"
 proof- 
 have "fst (brickcount cup) = 0" using brickcount_def by auto
-from this have subresult2:"fst (count (e_cup)) = 0" using count_def e_cup_def count.simps(1) 
+from this have subresult2:"fst (count ((cement cup))) = 0" using count_def  count.simps(1) 
 by (metis)
-have subresult3: " strands (e_vert\<otimes>e_vert)" using e_vert_def append_Nil strands_def 
+have subresult3: " strands ((cement vert)\<otimes>(cement vert))" using  append_Nil strands_def 
 by (metis brickstrand.simps(1) strands.simps(1) strands.simps(2))
-let ?a = "(Abs_diagram ((x1)\<circ>(basic (e_cup\<otimes>y1))\<circ>(basic (e_vert\<otimes>e_vert\<otimes>y2))
-\<circ>(basic (e_vert\<otimes>e_cap\<otimes>w4))\<circ>z1))"
-let ?b = "(Abs_diagram ((x1 \<circ> (basic y1)) \<circ>(basic (e_cup\<otimes>y2))\<circ>(basic (e_vert\<otimes>e_cap\<otimes>w4))\<circ>z1))"
+let ?a = "(Abs_diagram ((x1)\<circ>(basic ((cement cup)\<otimes>y1))\<circ>(basic ((cement vert)\<otimes>(cement vert)\<otimes>y2))
+\<circ>(basic ((cement vert)\<otimes>(cement cap)\<otimes>w4))\<circ>z1))"
+let ?b = "(Abs_diagram ((x1 \<circ> (basic y1)) \<circ>(basic ((cement cup)\<otimes>y2))\<circ>(basic ((cement vert)\<otimes>(cement cap)\<otimes>w4))\<circ>z1))"
  have subresult4: "  \<exists>y1.\<exists>w1.\<exists>w2.\<exists>A.\<exists>B.\<exists>y2.((?a = Abs_diagram
  ((y1)\<circ>(basic (A\<otimes>w1))\<circ>(basic (B\<otimes>w2))\<circ>(y2))) \<and>
  (?b = Abs_diagram
@@ -2691,8 +2694,8 @@ from this have "tanglerel_compress ?a ?b" using tanglerel_compress_def by auto
 then have " tanglerel ?a ?b" using tanglerel_def by auto
 then have "tanglerel_equiv ?a ?b" using tanglerel_equiv_def  r_into_rtranclp by (metis)
 then have subresult5: "tanglerel_equiv  
-(Abs_diagram ((x1)\<circ>(basic (e_cup\<otimes>y1))\<circ>(basic (e_vert\<otimes>e_vert\<otimes>y2))\<circ>(basic (e_vert\<otimes>e_cap\<otimes>w4))\<circ>z1))
-(Abs_diagram ((x1 \<circ> (basic y1)) \<circ>(basic (e_cup\<otimes>y2))\<circ>(basic (e_vert\<otimes>e_cap\<otimes>w4))\<circ>z1))"
+(Abs_diagram ((x1)\<circ>(basic ((cement cup)\<otimes>y1))\<circ>(basic ((cement vert)\<otimes>(cement vert)\<otimes>y2))\<circ>(basic ((cement vert)\<otimes>(cement cap)\<otimes>w4))\<circ>z1))
+(Abs_diagram ((x1 \<circ> (basic y1)) \<circ>(basic ((cement cup)\<otimes>y2))\<circ>(basic ((cement vert)\<otimes>(cement cap)\<otimes>w4))\<circ>z1))"
 by auto
 then show ?thesis by (simp add: compose_leftassociativity) 
 qed
@@ -2700,23 +2703,23 @@ qed
 theorem metaequivalence_left_doubledrop: 
 assumes "(snd (count y2))>1"
 and "w4 = makestrand  (nat ((snd (count y2)) + (-2)))" and "fst (count y2) = snd (count y1)"
-shows "tanglerel_equiv (Abs_diagram ((x1)\<circ>(basic (e_cup\<otimes>y1))\<circ>(basic (e_vert\<otimes>e_vert\<otimes>y2))
-            \<circ>(basic (e_vert\<otimes>e_cap\<otimes>w4))\<circ>z1))
+shows "tanglerel_equiv (Abs_diagram ((x1)\<circ>(basic ((cement cup)\<otimes>y1))\<circ>(basic ((cement vert)\<otimes>(cement vert)\<otimes>y2))
+            \<circ>(basic ((cement vert)\<otimes>(cement cap)\<otimes>w4))\<circ>z1))
              (Abs_diagram (x1 \<circ> basic y1\<circ> basic y2\<circ>z1))" 
 proof-
 let ?x = "x1 \<circ> (basic y1)"
 have subresult1: "tanglerel_equiv 
-   (Abs_diagram ((x1 \<circ> (basic y1)) \<circ>(basic (e_cup\<otimes>y2))\<circ>(basic (e_vert\<otimes>e_cap\<otimes>w4))\<circ>z1))
+   (Abs_diagram ((x1 \<circ> (basic y1)) \<circ>(basic ((cement cup)\<otimes>y2))\<circ>(basic ((cement vert)\<otimes>(cement cap)\<otimes>w4))\<circ>z1))
            (Abs_diagram ((x1 \<circ> (basic y1)) \<circ> basic y2 \<circ>z1))"  using assms metaequivalence_left 
              by auto
 have subresult2: "tanglerel_equiv 
- (Abs_diagram ((x1)\<circ>(basic (e_cup\<otimes>y1))\<circ>(basic (e_vert\<otimes>e_vert\<otimes>y2))\<circ>(basic (e_vert\<otimes>e_cap\<otimes>w4))\<circ>z1))
-(Abs_diagram (x1 \<circ> (basic y1) \<circ>(basic (e_cup\<otimes>y2))\<circ>(basic (e_vert\<otimes>e_cap\<otimes>w4))\<circ>z1))"
+ (Abs_diagram ((x1)\<circ>(basic ((cement cup)\<otimes>y1))\<circ>(basic ((cement vert)\<otimes>(cement vert)\<otimes>y2))\<circ>(basic ((cement vert)\<otimes>(cement cap)\<otimes>w4))\<circ>z1))
+(Abs_diagram (x1 \<circ> (basic y1) \<circ>(basic ((cement cup)\<otimes>y2))\<circ>(basic ((cement vert)\<otimes>(cement cap)\<otimes>w4))\<circ>z1))"
          using assms metaequivalence_left_drop compose_leftassociativity 
          by auto
 
 then have "tanglerel_equiv 
- (Abs_diagram ((x1)\<circ>(basic (e_cup\<otimes>y1))\<circ>(basic (e_vert\<otimes>e_vert\<otimes>y2))\<circ>(basic (e_vert\<otimes>e_cap\<otimes>w4))\<circ>z1))
+ (Abs_diagram ((x1)\<circ>(basic ((cement cup)\<otimes>y1))\<circ>(basic ((cement vert)\<otimes>(cement vert)\<otimes>y2))\<circ>(basic ((cement vert)\<otimes>(cement cap)\<otimes>w4))\<circ>z1))
            (Abs_diagram (x1 \<circ> (basic y1) \<circ> basic y2 \<circ>z1))"  using subresult1  rtranclp_trans
            Tangle.abs_eq_iff compose_leftassociativity assms
            by metis
@@ -2729,7 +2732,7 @@ lemma metaequivalence_left_doubledrop_condition:"(
 \<and>(fst (count y2) = snd (count y1)))
 \<Longrightarrow>
 (tanglerel_equiv 
- (Abs_diagram ((x1)\<circ>(basic (e_cup\<otimes>y1))\<circ>(basic (e_vert\<otimes>e_vert\<otimes>y2))\<circ>(basic (e_vert\<otimes>e_cap\<otimes>w4))\<circ>z1))
+ (Abs_diagram ((x1)\<circ>(basic ((cement cup)\<otimes>y1))\<circ>(basic ((cement vert)\<otimes>(cement vert)\<otimes>y2))\<circ>(basic ((cement vert)\<otimes>(cement cap)\<otimes>w4))\<circ>z1))
            (Abs_diagram (x1 \<circ> (basic y1) \<circ> basic y2 \<circ>z1)))"
 using metaequivalence_left_doubledrop by auto
 
@@ -2737,19 +2740,19 @@ theorem metaequivalence_right_drop:
 
 assumes "(snd (count y2))>1" 
 and "w4 = makestrand  (nat ((snd (count y2)) + (-2)))" and "fst (count y2) = snd (count y1)"
-shows "tanglerel_equiv (Abs_diagram ((x1)\<circ>(basic (y1\<otimes>e_cup))\<circ>(basic (y2\<otimes>e_vert\<otimes>e_vert))\<circ>(basic (w4\<otimes>e_cap\<otimes>e_vert))\<circ>z1))
-             (Abs_diagram (x1 \<circ> (basic y1) \<circ>(basic (y2\<otimes>e_cup))\<circ>(basic (w4\<otimes>e_cap\<otimes>e_vert))\<circ>z1))"
+shows "tanglerel_equiv (Abs_diagram ((x1)\<circ>(basic (y1\<otimes>(cement cup)))\<circ>(basic (y2\<otimes>(cement vert)\<otimes>(cement vert)))\<circ>(basic (w4\<otimes>(cement cap)\<otimes>(cement vert)))\<circ>z1))
+             (Abs_diagram (x1 \<circ> (basic y1) \<circ>(basic (y2\<otimes>(cement cup)))\<circ>(basic (w4\<otimes>(cement cap)\<otimes>(cement vert)))\<circ>z1))"
 proof-
 have "fst (brickcount cup) = 0" using brickcount_def by auto
-from this have subresult2:"fst (count (e_cup)) = 0" using count_def e_cup_def count.simps(1) 
+from this have subresult2:"fst (count ((cement cup))) = 0" using count_def  count.simps(1) 
 by (metis)
 
-have subresult3: " strands (e_vert\<otimes>e_vert)" using e_vert_def append_Nil strands_def 
+have subresult3: " strands ((cement vert)\<otimes>(cement vert))" using  append_Nil strands_def 
 by (metis brickstrand.simps(1) strands.simps(1) strands.simps(2))
 
-let ?a = " (Abs_diagram ((x1)\<circ>(basic (y1\<otimes>e_cup))\<circ>(basic (y2\<otimes>e_vert\<otimes>e_vert))\<circ>(basic (w4\<otimes>e_cap\<otimes>e_vert))\<circ>z1))"
+let ?a = " (Abs_diagram ((x1)\<circ>(basic (y1\<otimes>(cement cup)))\<circ>(basic (y2\<otimes>(cement vert)\<otimes>(cement vert)))\<circ>(basic (w4\<otimes>(cement cap)\<otimes>(cement vert)))\<circ>z1))"
 
-let ?b = "(Abs_diagram (x1 \<circ> (basic y1) \<circ>(basic (y2\<otimes>e_cup))\<circ>(basic (w4\<otimes>e_cap\<otimes>e_vert))\<circ>z1))"
+let ?b = "(Abs_diagram (x1 \<circ> (basic y1) \<circ>(basic (y2\<otimes>(cement cup)))\<circ>(basic (w4\<otimes>(cement cap)\<otimes>(cement vert)))\<circ>z1))"
  
 
 have subresult4: "  \<exists>y1.\<exists>w1.\<exists>w2.\<exists>A.\<exists>B.\<exists>y2.((?a = Abs_diagram
@@ -2769,8 +2772,8 @@ from this have "tanglerel_compbelow ?a ?b" using tanglerel_compbelow_def by auto
 from this have "tanglerel_compress ?a ?b" using tanglerel_compress_def by auto
 then have " tanglerel ?a ?b" using tanglerel_def by auto
 then have "tanglerel_equiv ?a ?b" using tanglerel_equiv_def  r_into_rtranclp by (metis)
-then have "tanglerel_equiv (Abs_diagram ((x1)\<circ>(basic (y1\<otimes>e_cup))\<circ>(basic (y2\<otimes>e_vert\<otimes>e_vert))\<circ>(basic (w4\<otimes>e_cap\<otimes>e_vert))\<circ>z1))
-             (Abs_diagram (x1 \<circ> (basic y1) \<circ>(basic (y2\<otimes>e_cup))\<circ>(basic (w4\<otimes>e_cap\<otimes>e_vert))\<circ>z1))"
+then have "tanglerel_equiv (Abs_diagram ((x1)\<circ>(basic (y1\<otimes>(cement cup)))\<circ>(basic (y2\<otimes>(cement vert)\<otimes>(cement vert)))\<circ>(basic (w4\<otimes>(cement cap)\<otimes>(cement vert)))\<circ>z1))
+             (Abs_diagram (x1 \<circ> (basic y1) \<circ>(basic (y2\<otimes>(cement cup)))\<circ>(basic (w4\<otimes>(cement cap)\<otimes>(cement vert)))\<circ>z1))"
 by auto
 from this show ?thesis by auto
 qed
@@ -2778,19 +2781,19 @@ qed
 theorem metaequivalence_right_doubledrop: 
 assumes "(snd (count y2))>1" 
 and "w4 = makestrand  (nat ((snd (count y2)) + (-2)))" and "fst (count y2) = snd (count y1)"
-shows "tanglerel_equiv (Abs_diagram ((x1)\<circ>(basic (y1\<otimes>e_cup))\<circ>(basic (y2\<otimes>e_vert\<otimes>e_vert))\<circ>
-(basic (w4\<otimes>e_cap\<otimes>e_vert))\<circ>z1))
+shows "tanglerel_equiv (Abs_diagram ((x1)\<circ>(basic (y1\<otimes>(cement cup)))\<circ>(basic (y2\<otimes>(cement vert)\<otimes>(cement vert)))\<circ>
+(basic (w4\<otimes>(cement cap)\<otimes>(cement vert)))\<circ>z1))
              (Abs_diagram (x1 \<circ> (basic y1)\<circ> (basic y2)\<circ>z1))" 
 proof-
 let ?x = "x1 \<circ> (basic y1)"
 have subresult1: "tanglerel_equiv 
-   (Abs_diagram ((x1 \<circ> (basic y1)) \<circ>(basic (e_cup\<otimes>y2))\<circ>(basic (e_vert\<otimes>e_cap\<otimes>w4))\<circ>z1))
+   (Abs_diagram ((x1 \<circ> (basic y1)) \<circ>(basic ((cement cup)\<otimes>y2))\<circ>(basic ((cement vert)\<otimes>(cement cap)\<otimes>w4))\<circ>z1))
            (Abs_diagram ((x1 \<circ> (basic y1)) \<circ> basic y2 \<circ>z1))"  using assms metaequivalence_left 
              by auto
-then have " tanglerel_equiv (Abs_diagram ((x1)\<circ>(basic (y1\<otimes>e_cup))\<circ>(basic (y2\<otimes>e_vert\<otimes>e_vert))\<circ>(basic (w4\<otimes>e_cap\<otimes>e_vert))\<circ>z1))
-             (Abs_diagram (x1 \<circ> (basic y1) \<circ>(basic (y2\<otimes>e_cup))\<circ>(basic (w4\<otimes>e_cap\<otimes>e_vert))\<circ>z1))"
+then have " tanglerel_equiv (Abs_diagram ((x1)\<circ>(basic (y1\<otimes>(cement cup)))\<circ>(basic (y2\<otimes>(cement vert)\<otimes>(cement vert)))\<circ>(basic (w4\<otimes>(cement cap)\<otimes>(cement vert)))\<circ>z1))
+             (Abs_diagram (x1 \<circ> (basic y1) \<circ>(basic (y2\<otimes>(cement cup)))\<circ>(basic (w4\<otimes>(cement cap)\<otimes>(cement vert)))\<circ>z1))"
 using metaequivalence_right_drop assms by auto
-from this have  " tanglerel_equiv (Abs_diagram (((x1)\<circ>(basic (y1\<otimes>e_cup)))\<circ>(basic (y2\<otimes>e_vert\<otimes>e_vert))\<circ>(basic (w4\<otimes>e_cap\<otimes>e_vert))\<circ>z1))
+from this have  " tanglerel_equiv (Abs_diagram (((x1)\<circ>(basic (y1\<otimes>(cement cup))))\<circ>(basic (y2\<otimes>(cement vert)\<otimes>(cement vert)))\<circ>(basic (w4\<otimes>(cement cap)\<otimes>(cement vert)))\<circ>z1))
               (Abs_diagram ((x1 \<circ> (basic y1)) \<circ> basic y2 \<circ>z1))" 
                using subresult1  rtranclp_trans
            Tangle.abs_eq_iff compose_leftassociativity assms
@@ -2805,39 +2808,39 @@ assumes "(snd (count y2))>1"
 and "w4 = makestrand  (nat ((snd (count y2)) + (-2)))" 
 and "w5 = makestrand (nat ((snd (count y2))))"
 and "fst (count y2) = snd (count y1)"
-shows "tanglerel_equiv (Abs_diagram ((x1)\<circ>(basic (e_cup\<otimes>y1\<otimes>e_cup))\<circ>(basic (e_vert\<otimes>e_vert\<otimes>y2\<otimes>e_vert\<otimes>e_vert))\<circ>
-(basic (e_vert\<otimes>e_cap\<otimes> w5)) \<circ> (basic (w4\<otimes>e_cap\<otimes>e_vert))\<circ>z1))
+shows "tanglerel_equiv (Abs_diagram ((x1)\<circ>(basic ((cement cup)\<otimes>y1\<otimes>(cement cup)))\<circ>(basic ((cement vert)\<otimes>(cement vert)\<otimes>y2\<otimes>(cement vert)\<otimes>(cement vert)))\<circ>
+(basic ((cement vert)\<otimes>(cement cap)\<otimes> w5)) \<circ> (basic (w4\<otimes>(cement cap)\<otimes>(cement vert)))\<circ>z1))
              (Abs_diagram (x1 \<circ> (basic y1)\<circ> (basic y2)\<circ>z1))" 
 
 proof-
-have subresult1: "tanglerel_equiv (Abs_diagram ((x1)\<circ>(basic (y1\<otimes>e_cup))\<circ>(basic (y2\<otimes>e_vert\<otimes>e_vert))\<circ>
-(basic (w4\<otimes>e_cap\<otimes>e_vert))\<circ>z1))
+have subresult1: "tanglerel_equiv (Abs_diagram ((x1)\<circ>(basic (y1\<otimes>(cement cup)))\<circ>(basic (y2\<otimes>(cement vert)\<otimes>(cement vert)))\<circ>
+(basic (w4\<otimes>(cement cap)\<otimes>(cement vert)))\<circ>z1))
              (Abs_diagram (x1 \<circ> (basic y1)\<circ> (basic y2)\<circ>z1))" using assms metaequivalence_right_doubledrop
              by auto
-let ?p1 = "y1 \<otimes> e_cup"
-let ?p2 = "y2 \<otimes> e_vert \<otimes>e_vert"
-let ?p3 = "(basic (w4 \<otimes> e_cap \<otimes> e_vert))\<circ>z1"
-have  "(snd (count (x\<otimes>e_vert\<otimes>e_vert))) = (snd (count (x\<otimes>e_vert)) + 1)"
-using e_vert_def append_Nil append_Cons brickcount_def count_def 
+let ?p1 = "y1 \<otimes> (cement cup)"
+let ?p2 = "y2 \<otimes> (cement vert) \<otimes>(cement vert)"
+let ?p3 = "(basic (w4 \<otimes> (cement cap) \<otimes> (cement vert)))\<circ>z1"
+have  "(snd (count (x\<otimes>(cement vert)\<otimes>(cement vert)))) = (snd (count (x\<otimes>(cement vert))) + 1)"
+using append_Nil append_Cons brickcount_def count_def 
 by (metis (hide_lams, no_types) brickcount.simps(1) count.simps(1) count_rightcompose
 leftright_associativity snd_conv)
-from this have subresult2:  "(snd (count (y2\<otimes>e_vert\<otimes>e_vert))) = (snd (count (y2)) + 2)"
-using e_vert_def append_Nil  append_Cons brickcount_def count_def
+from this have subresult2:  "(snd (count (y2\<otimes>(cement vert)\<otimes>(cement vert)))) = (snd (count (y2)) + 2)"
+using  append_Nil  append_Cons brickcount_def count_def
 by (metis (hide_lams, no_types) brickcount.simps(1) count.simps(1) count_rightcompose
 dbl_def dbl_simps(3) snd_conv)
-from this have "snd (count (y2 \<otimes> e_vert \<otimes> e_vert)) > (snd (count y2))" by auto
+from this have "snd (count (y2 \<otimes> (cement vert) \<otimes> (cement vert))) > (snd (count y2))" by auto
 from this have step1: "snd (count (?p2)) > 1" using assms  by auto
-have  "(fst (count (x\<otimes>e_vert\<otimes>e_vert))) = (fst (count (x\<otimes>e_vert)) + 1)"
-using e_vert_def append_Nil append_Cons brickcount_def count_def 
+have  "(fst (count (x\<otimes>(cement vert)\<otimes>(cement vert)))) = (fst (count (x\<otimes>(cement vert))) + 1)"
+using  append_Nil append_Cons brickcount_def count_def 
 by (metis (hide_lams, no_types) brickcount.simps(1) count.simps(1) count_rightcompose
 leftright_associativity fst_conv)
-from this have assm2_substep1: "(fst (count (y2\<otimes>e_vert\<otimes>e_vert))) = (fst (count (y2)) + 2)"
-using e_vert_def append_Nil append_Cons brickcount_def count_def
+from this have assm2_substep1: "(fst (count (y2\<otimes>(cement vert)\<otimes>(cement vert)))) = (fst (count (y2)) + 2)"
+using  append_Nil append_Cons brickcount_def count_def
 by (metis (hide_lams, no_types) brickcount.simps(1) count.simps(1) count_rightcompose
 dbl_def dbl_simps(3) fst_conv)
-have "(snd (count (y1\<otimes>e_cup))) = (snd (count y1)) + 2"
-using e_cup_def count_def snd_conv append_Cons count_cup_rightcompose  by auto
-from this have "(snd (count (y1\<otimes>e_cup))) = ((fst (count y2)) +2)" using assms by auto
+have "(snd (count (y1\<otimes>(cement cup)))) = (snd (count y1)) + 2"
+using  count_def snd_conv append_Cons count_cup_rightcompose  by auto
+from this have "(snd (count (y1\<otimes>(cement cup)))) = ((fst (count y2)) +2)" using assms by auto
 from this have step2: "fst (count ?p2) = snd (count ?p1)" using 
 assm2_substep1  by auto
 from subresult2 have "snd (count ?p2) = (snd (count y2)) + 2"  by auto
@@ -2845,20 +2848,20 @@ from this have subresult5: "w5 = makestrand (nat (((snd (count ?p2)) + (-2))))" 
 have subresult3: "(((snd (count ?p2))>1) \<and> (w5= makestrand  (nat ((snd (count ?p2)) + (-2))))
 \<and>(fst (count ?p2) = snd (count ?p1)))"
 using assms step1 step2 subresult5 by auto
-from this have "tanglerel_equiv (Abs_diagram ((x1)\<circ>(basic (e_cup\<otimes>?p1))\<circ>(basic (e_vert\<otimes>e_vert\<otimes>?p2))
-            \<circ>(basic (e_vert\<otimes>e_cap\<otimes>w5))\<circ>?p3))
+from this have "tanglerel_equiv (Abs_diagram ((x1)\<circ>(basic ((cement cup)\<otimes>?p1))\<circ>(basic ((cement vert)\<otimes>(cement vert)\<otimes>?p2))
+            \<circ>(basic ((cement vert)\<otimes>(cement cap)\<otimes>w5))\<circ>?p3))
              (Abs_diagram (x1 \<circ> basic ?p1\<circ> basic ?p2\<circ>?p3))"
  using  metaequivalence_left_doubledrop_condition by auto
-from this have subresult6: "tanglerel_equiv (Abs_diagram ((x1)\<circ>(basic (e_cup\<otimes>y1 \<otimes> e_cup))
-  \<circ>(basic (e_vert\<otimes>e_vert\<otimes>y2 \<otimes> e_vert \<otimes>e_vert))
-            \<circ>(basic (e_vert\<otimes>e_cap\<otimes>w5))\<circ>(basic (w4 \<otimes> e_cap \<otimes> e_vert))\<circ>z1))
-             (Abs_diagram (x1 \<circ> basic (y1 \<otimes> e_cup)\<circ> basic (y2 \<otimes> e_vert \<otimes>e_vert)
-\<circ>(basic (w4 \<otimes> e_cap \<otimes> e_vert))\<circ>z1))"
+from this have subresult6: "tanglerel_equiv (Abs_diagram ((x1)\<circ>(basic ((cement cup)\<otimes>y1 \<otimes> (cement cup)))
+  \<circ>(basic ((cement vert)\<otimes>(cement vert)\<otimes>y2 \<otimes> (cement vert) \<otimes>(cement vert)))
+            \<circ>(basic ((cement vert)\<otimes>(cement cap)\<otimes>w5))\<circ>(basic (w4 \<otimes> (cement cap) \<otimes> (cement vert)))\<circ>z1))
+             (Abs_diagram (x1 \<circ> basic (y1 \<otimes> (cement cup))\<circ> basic (y2 \<otimes> (cement vert) \<otimes>(cement vert))
+\<circ>(basic (w4 \<otimes> (cement cap) \<otimes> (cement vert)))\<circ>z1))"
  using  metaequivalence_left_doubledrop_condition  by auto
  from this have "tanglerel_equiv 
- (Abs_diagram ((x1)\<circ>(basic (e_cup\<otimes>y1 \<otimes> e_cup))
-  \<circ>(basic (e_vert\<otimes>e_vert\<otimes>y2 \<otimes> e_vert \<otimes>e_vert))
-            \<circ>(basic (e_vert\<otimes>e_cap\<otimes>w5))\<circ>(basic (w4 \<otimes> e_cap \<otimes> e_vert))\<circ>z1))
+ (Abs_diagram ((x1)\<circ>(basic ((cement cup)\<otimes>y1 \<otimes> (cement cup)))
+  \<circ>(basic ((cement vert)\<otimes>(cement vert)\<otimes>y2 \<otimes> (cement vert) \<otimes>(cement vert)))
+            \<circ>(basic ((cement vert)\<otimes>(cement cap)\<otimes>w5))\<circ>(basic (w4 \<otimes> (cement cap) \<otimes> (cement vert)))\<circ>z1))
  (Abs_diagram (x1 \<circ> (basic y1)\<circ> (basic y2)\<circ>z1))"
 using subresult1 rtranclp_trans Tangle.abs_eq_iff by (metis)
 from this  show ?thesis by (simp)
@@ -2868,27 +2871,27 @@ theorem metaequivalence_top_drop: assumes "(snd (count y1))>1"
 and "w4 = makestrand  (nat ((snd (count y1)) + (-2)))" 
 and "w5 = makestrand (nat ((snd (count y1))))"
 and "fst (count y2) = snd (count y1)"
-shows "tanglerel_equiv (Abs_diagram ((x1)\<circ>(basic (e_cup\<otimes>y1\<otimes>e_cup))\<circ>
-(basic (e_vert\<otimes>e_cap\<otimes> w5)) \<circ> (basic (w4\<otimes>e_cap\<otimes>e_vert))\<circ>z1))
+shows "tanglerel_equiv (Abs_diagram ((x1)\<circ>(basic ((cement cup)\<otimes>y1\<otimes>(cement cup)))\<circ>
+(basic ((cement vert)\<otimes>(cement cap)\<otimes> w5)) \<circ> (basic (w4\<otimes>(cement cap)\<otimes>(cement vert)))\<circ>z1))
              (Abs_diagram (x1 \<circ> (basic y1)\<circ> z1))" 
 proof-
 from metaequivalence_right and assms have subresult1: "tanglerel_equiv 
-      (Abs_diagram ((x1)\<circ>(basic (y1\<otimes>e_cup))\<circ>(basic (w4\<otimes>e_cap\<otimes>e_vert))\<circ>z1))
+      (Abs_diagram ((x1)\<circ>(basic (y1\<otimes>(cement cup)))\<circ>(basic (w4\<otimes>(cement cap)\<otimes>(cement vert)))\<circ>z1))
              (Abs_diagram (x1 \<circ> (basic y1)\<circ>z1))" by auto
-let ?y2 = "y1 \<otimes> e_cup"
-let ?z2 = "(basic (w4\<otimes>e_cap\<otimes>e_vert))\<circ>z1"
+let ?y2 = "y1 \<otimes> (cement cup)"
+let ?z2 = "(basic (w4\<otimes>(cement cap)\<otimes>(cement vert)))\<circ>z1"
 have subresult2:"(snd (count (?y2))) = (snd (count y1)) + 2"
-using e_cup_def count_def snd_conv append_Cons count_cup_rightcompose by auto
+using  count_def snd_conv append_Cons count_cup_rightcompose by auto
 from this and assms have subresult3:"(snd (count (?y2))) >1" by auto
 from subresult2 have subresult4: "w5 = makestrand (nat (snd (count ?y2) + (-2)))" using assms by auto
 from this and assms and subresult3 and metaequivalence_left have "tanglerel_equiv 
-      (Abs_diagram ((x1)\<circ>(basic (e_cup\<otimes>?y2))\<circ>(basic (e_vert\<otimes>e_cap\<otimes> w5))\<circ>?z2))
+      (Abs_diagram ((x1)\<circ>(basic ((cement cup)\<otimes>?y2))\<circ>(basic ((cement vert)\<otimes>(cement cap)\<otimes> w5))\<circ>?z2))
                (Abs_diagram ((x1)\<circ>(basic (?y2))\<circ>?z2))" by auto
 from this have "tanglerel_equiv 
-      (Abs_diagram ((x1)\<circ>(basic (e_cup\<otimes>y1\<otimes>e_cup))\<circ>(basic (e_vert\<otimes>e_cap\<otimes> w5))\<circ>(basic (w4\<otimes>e_cap\<otimes>e_vert))\<circ>z1))
-               (Abs_diagram ((x1)\<circ>(basic (y1 \<otimes> e_cup))\<circ>(basic (w4\<otimes>e_cap\<otimes>e_vert))\<circ>z1))" by auto
+      (Abs_diagram ((x1)\<circ>(basic ((cement cup)\<otimes>y1\<otimes>(cement cup)))\<circ>(basic ((cement vert)\<otimes>(cement cap)\<otimes> w5))\<circ>(basic (w4\<otimes>(cement cap)\<otimes>(cement vert)))\<circ>z1))
+               (Abs_diagram ((x1)\<circ>(basic (y1 \<otimes> (cement cup)))\<circ>(basic (w4\<otimes>(cement cap)\<otimes>(cement vert)))\<circ>z1))" by auto
 from this and subresult1 have "tanglerel_equiv 
-      (Abs_diagram ((x1)\<circ>(basic (e_cup\<otimes>y1\<otimes>e_cup))\<circ>(basic (e_vert\<otimes>e_cap\<otimes> w5))\<circ>(basic (w4\<otimes>e_cap\<otimes>e_vert))\<circ>z1))
+      (Abs_diagram ((x1)\<circ>(basic ((cement cup)\<otimes>y1\<otimes>(cement cup)))\<circ>(basic ((cement vert)\<otimes>(cement cap)\<otimes> w5))\<circ>(basic (w4\<otimes>(cement cap)\<otimes>(cement vert)))\<circ>z1))
             (Abs_diagram (x1 \<circ> (basic y1)\<circ> z1))" using rtranclp_trans Tangle.abs_eq_iff 
 by metis
 then show ?thesis by simp
@@ -2898,34 +2901,36 @@ theorem metaequivalence_bottom_doubledrag: assumes "(fst (count y1))>1"
 and "w4 = makestrand  (nat ((fst (count y1)) + (-2)))" 
 and "w5 = makestrand (nat ((fst (count y1))))"
 and "well_defined (x1 \<circ> basic y1 \<circ> z1)" 
-shows "tanglerel_equiv (Abs_diagram ((x1)\<circ>  (basic (w4\<otimes>e_cup\<otimes>e_vert)) \<circ>
-(basic (e_vert\<otimes>e_cup\<otimes>w5))\<circ>(basic (e_cap\<otimes>y1\<otimes>e_cap))\<circ>z1))
+shows "tanglerel_equiv (Abs_diagram ((x1)\<circ>  (basic (w4\<otimes>(cement cup)\<otimes>(cement vert))) \<circ>
+(basic ((cement vert)\<otimes>(cement cup)\<otimes>w5))\<circ>(basic ((cement cap)\<otimes>y1\<otimes>(cement cap)))\<circ>z1))
              (Abs_diagram (x1 \<circ> (basic y1)\<circ> z1))" 
 proof-
 have "(fst (count y1))>1" using assms by auto
 also have  "w4 = makestrand  (nat ((fst (count y1)) + (-2)))" using assms by auto
  have "well_defined (x1 \<circ> basic y1 \<circ> z1)"  using assms by auto
 from assms and metaequivalence_bottomright have subresult1: "tanglerel_equiv 
-      (Abs_diagram ((x1)\<circ>(basic (w4\<otimes>e_cup\<otimes>e_vert))\<circ>(basic (y1\<otimes>e_cap))\<circ>z1))
+      (Abs_diagram ((x1)\<circ>(basic (w4\<otimes>(cement cup)\<otimes>(cement vert)))\<circ>(basic (y1\<otimes>(cement cap)))\<circ>z1))
              (Abs_diagram (x1 \<circ> (basic y1)\<circ>z1))"  
 by auto
-let ?y2 = "y1 \<otimes> e_cap"
-let ?x2 = "x1\<circ>(basic (w4\<otimes>e_cup\<otimes>e_vert))"
+let ?y2 = "y1 \<otimes> (cement cap)"
+let ?x2 = "x1\<circ>(basic (w4\<otimes>(cement cup)\<otimes>(cement vert)))"
 have subresult2:"(fst (count (?y2))) = (fst (count y1)) + 2"
-using e_cup_def count_def fst_conv append_Cons count_cup_rightcompose by (metis brickcount.simps(3) count.simps(1) e_cap_def fst_count_additive)
+using count_def fst_conv append_Cons count_cup_rightcompose by (metis brickcount.simps(3) count.simps(1)
+ fst_count_additive)
 from this and assms have subresult3:"(fst (count (?y2))) >1" by auto
-have subresult4: " snd (count (y1\<otimes>e_cap)) = snd (count y1)" using e_cap_def count_def snd_conv append_Cons count_cup_rightcompose
+have subresult4: " snd (count (y1\<otimes>(cement cap))) = snd (count y1)" using 
+ count_def snd_conv append_Cons count_cup_rightcompose
 by (metis (hide_lams, no_types) brickcount.simps(3) comm_monoid_add_class.add.right_neutral 
 count.simps(1) snd_count_additive)
-have "snd (count (w4\<otimes>e_cup\<otimes>e_vert)) = snd (count w4) + snd (count e_cup) +
-snd (count e_vert)" using leftright_associativity snd_count_additive by (auto)
-from this have subresult5: "snd (count (w4\<otimes>e_cup\<otimes>e_vert)) = snd (count w4) +3"
-using count_def e_cup_def e_vert_def snd_conv by (metis ab_semigroup_add_class.add_ac(1) 
+have "snd (count (w4\<otimes>(cement cup)\<otimes>(cement vert))) = snd (count w4) + snd (count (cement cup)) +
+snd (count (cement vert))" using leftright_associativity snd_count_additive by (auto)
+from this have subresult5: "snd (count (w4\<otimes>(cement cup)\<otimes>(cement vert))) = snd (count w4) +3"
+using count_def  snd_conv by (metis ab_semigroup_add_class.add_ac(1) 
 brickcount.simps(1) brickcount.simps(2) count.simps(1) inc.simps(2) numeral_inc)
-have "fst (count (w4\<otimes>e_cup\<otimes>e_vert)) =  fst (count w4) + fst (count e_cup) + fst( count e_vert)"
+have "fst (count (w4\<otimes>(cement cup)\<otimes>(cement vert))) =  fst (count w4) + fst (count (cement cup)) + fst( count (cement vert))"
 using leftright_associativity fst_count_additive by auto
-from this have subresult6: "fst (count (w4\<otimes>e_cup\<otimes>e_vert)) =  fst (count w4) + 1"
-using count_def e_cup_def e_vert_def fst_conv brickcount.simps(1) count.simps(1) fst_count_additive 
+from this have subresult6: "fst (count (w4\<otimes>(cement cup)\<otimes>(cement vert))) =  fst (count w4) + 1"
+using count_def  fst_conv brickcount.simps(1) count.simps(1) fst_count_additive 
 fstcount_cup_rightcompose
  by (metis (full_types))
 have "(snd (count (makestrand n))) = (int n)+1"  using makestrand_sndequality by auto
@@ -2939,24 +2944,24 @@ from this and subresult7
 from this have subresult8: "fst (count w4) = fst (count y1) + (-1)" by auto
 from this and makestrand_fstsndequality and assms have " snd (count w4) =  fst (count y1) + (-1)"
 by auto
-from this and subresult5 have "snd (count (w4\<otimes>e_cup\<otimes>e_vert)) = fst (count y1) + (-1) + 3" by auto
-from this and subresult2 have subresult9: "snd (count (w4\<otimes>e_cup\<otimes>e_vert)) = fst (count (y1\<otimes>e_cap))" by auto
-from subresult8 and subresult6 have subresult10: "fst (count (w4\<otimes>e_cup\<otimes>e_vert)) = fst (count y1)" by auto
+from this and subresult5 have "snd (count (w4\<otimes>(cement cup)\<otimes>(cement vert))) = fst (count y1) + (-1) + 3" by auto
+from this and subresult2 have subresult9: "snd (count (w4\<otimes>(cement cup)\<otimes>(cement vert))) = fst (count (y1\<otimes>(cement cap)))" by auto
+from subresult8 and subresult6 have subresult10: "fst (count (w4\<otimes>(cement cup)\<otimes>(cement vert))) = fst (count y1)" by auto
 from subresult2 have subresult11: "w5 = makestrand (nat (fst (count ?y2) + (-2)))" using assms by auto
 have subresult12: "fst (wall_count ((basic y1)\<circ>z1)) = snd(wall_count x1)" 
 using assms diagram_fst_equals_snd by metis
 have  "fst (wall_count ((basic y1)\<circ>z1)) = fst(count y1)" using wall_count_def compose_def by auto
 from this and subresult12 have "snd(wall_count x1) = (fst (count y1))" by simp
-from this and subresult10 have subresult13: "snd(wall_count x1) = (fst (count (w4\<otimes>e_cup\<otimes>e_vert)))" by auto
+from this and subresult10 have subresult13: "snd(wall_count x1) = (fst (count (w4\<otimes>(cement cup)\<otimes>(cement vert))))" by auto
 have subresult14:"snd (wall_count (x1\<circ>(basic y1))) = fst(wall_count z1)" 
 using assms diagram_fst_equals_snd by (metis compose_leftassociativity)
 have "snd (wall_count (x1\<circ>(basic y1))) = snd (count y1)" using wall_count_def compose_def by (metis snd_conv wall_count.simps(1) wall_count_compose)
 from subresult14 and this have subresult15: "fst(wall_count z1) =  snd (count y1)" by simp
 from this and subresult4 have subresult16: "fst(wall_count z1) = snd (count ?y2)" by simp
 
-have "(fst (wall_count ((basic (w4\<otimes>e_cup\<otimes>e_vert))\<circ>(basic ?y2)\<circ>z1))) = fst (count (w4\<otimes>e_cup\<otimes>e_vert))"
+have "(fst (wall_count ((basic (w4\<otimes>(cement cup)\<otimes>(cement vert)))\<circ>(basic ?y2)\<circ>z1))) = fst (count (w4\<otimes>(cement cup)\<otimes>(cement vert)))"
 by auto
-from this and  subresult13 have subresult17: "snd(wall_count x1) = (fst (wall_count ((basic (w4\<otimes>e_cup\<otimes>e_vert))\<circ>(basic ?y2)\<circ>z1)))"
+from this and  subresult13 have subresult17: "snd(wall_count x1) = (fst (wall_count ((basic (w4\<otimes>(cement cup)\<otimes>(cement vert)))\<circ>(basic ?y2)\<circ>z1)))"
 by auto
 
 have  "list_sum (wall_list (?y2*z1)) = 0" using subresult16 
@@ -2965,10 +2970,10 @@ compose_Nil diagram_list_sum_zero diagram_wall_list_zero list_sum.simps(2)
 list_sum_append monoid_add_class.add.left_neutral subresult15 wall_list.simps(2) 
 wall_list_compose wall_list_list_sum_non_negative)
 from this have subresult18: " list_sum (wall_list ((basic ?y2)\<circ>z1)) = 0" by auto
-from subresult9 have "snd (count (w4\<otimes>e_cup\<otimes>e_vert)) = (fst (wall_count (((basic ?y2)\<circ>z1))))"
+from subresult9 have "snd (count (w4\<otimes>(cement cup)\<otimes>(cement vert))) = (fst (wall_count (((basic ?y2)\<circ>z1))))"
 by (metis fst_conv wall_count.simps(1) wall_count_compose)
 from this and subresult18
-have "list_sum (wall_list ((w4\<otimes>e_cup\<otimes>e_vert)*((basic ?y2)\<circ>z1))) = 0"
+have "list_sum (wall_list ((w4\<otimes>(cement cup)\<otimes>(cement vert))*((basic ?y2)\<circ>z1))) = 0"
 using 
 add_nonneg_eq_0_iff assms(4) 
 compose_Nil diagram_list_sum_zero diagram_wall_list_zero list_sum.simps(2) 
@@ -2976,17 +2981,17 @@ list_sum_append monoid_add_class.add.left_neutral subresult15 wall_list.simps(2)
 wall_list_compose wall_list_list_sum_non_negative
 by (metis `fst (wall_count (basic y1 \<circ> z1)) = fst (count y1)` `
 snd (wall_count x1) = fst (count y1)` diff_self subresult16 subresult9)
-from this have subresult19: "list_sum (wall_list ((basic (w4\<otimes>e_cup\<otimes>e_vert))\<circ>((basic ?y2)\<circ>z1))) = 0"
+from this have subresult19: "list_sum (wall_list ((basic (w4\<otimes>(cement cup)\<otimes>(cement vert)))\<circ>((basic ?y2)\<circ>z1))) = 0"
 by auto
 
 from diagram_list_sum_subsequence have subresult20: " ((list_sum (wall_list x1) = 0)
 \<and>((list_sum (wall_list ((basic y1)\<circ>z1)))=0))" using assms by metis
-have "list_sum (wall_list ((x1)\<circ>(basic (w4\<otimes>e_cup\<otimes>e_vert))\<circ>(basic (y1\<otimes>e_cap))\<circ>z1)) = 
-list_sum (wall_list ((x1))) + list_sum (wall_list ((basic (w4\<otimes>e_cup\<otimes>e_vert))\<circ>(basic (y1\<otimes>e_cap))\<circ>z1))
-+ abs ((fst (wall_count ((basic (w4\<otimes>e_cup\<otimes>e_vert))\<circ>(basic (y1\<otimes>e_cap))\<circ>z1))) - (snd (wall_count x1)))"
+have "list_sum (wall_list ((x1)\<circ>(basic (w4\<otimes>(cement cup)\<otimes>(cement vert)))\<circ>(basic (y1\<otimes>(cement cap)))\<circ>z1)) = 
+list_sum (wall_list ((x1))) + list_sum (wall_list ((basic (w4\<otimes>(cement cup)\<otimes>(cement vert)))\<circ>(basic (y1\<otimes>(cement cap)))\<circ>z1))
++ abs ((fst (wall_count ((basic (w4\<otimes>(cement cup)\<otimes>(cement vert)))\<circ>(basic (y1\<otimes>(cement cap)))\<circ>z1))) - (snd (wall_count x1)))"
 using wall_list_list_sum_compose by auto
 from this and subresult19 and subresult20 and subresult17 
-have subresult21: "list_sum (wall_list ((x1)\<circ>(basic (w4\<otimes>e_cup\<otimes>e_vert))\<circ>(basic (y1\<otimes>e_cap))\<circ>z1)) =0"
+have subresult21: "list_sum (wall_list ((x1)\<circ>(basic (w4\<otimes>(cement cup)\<otimes>(cement vert)))\<circ>(basic (y1\<otimes>(cement cap)))\<circ>z1)) =0"
 by (metis diff_self monoid_add_class.add.right_neutral wall_list_list_sum_abs)
 
 have subresult22:" (fst (wall_count ((x1)\<circ>(basic y1)\<circ>z1))) = fst(wall_count x1)" using wall_count_def
@@ -3000,35 +3005,35 @@ compose_Cons by (metis snd_conv wall_count_compose)
  have "abs( snd(wall_count (x1 \<circ>(basic y1)\<circ>z1))) = 0" using well_defined_snd_wall_count assms  
 by metis
 from subresult24 and this have subresult25:"abs (snd(wall_count z1)) = 0"  by auto
-have subresult26:" (fst (wall_count (((x1)\<circ>(basic (w4\<otimes>e_cup\<otimes>e_vert))\<circ>(basic (y1\<otimes>e_cap))\<circ>z1))))
+have subresult26:" (fst (wall_count (((x1)\<circ>(basic (w4\<otimes>(cement cup)\<otimes>(cement vert)))\<circ>(basic (y1\<otimes>(cement cap)))\<circ>z1))))
 = fst(wall_count x1)" 
 using wall_count_def compose_Cons by (metis fst_conv wall_count_compose)
 from this and subresult23 
-have subresult27:" abs (fst (wall_count (((x1)\<circ>(basic (w4\<otimes>e_cup\<otimes>e_vert))\<circ>(basic (y1\<otimes>e_cap))\<circ>z1)))) = 0" by auto
-have subresult28:" (snd (wall_count (((x1)\<circ>(basic (w4\<otimes>e_cup\<otimes>e_vert))\<circ>(basic (y1\<otimes>e_cap))\<circ>z1))))
+have subresult27:" abs (fst (wall_count (((x1)\<circ>(basic (w4\<otimes>(cement cup)\<otimes>(cement vert)))\<circ>(basic (y1\<otimes>(cement cap)))\<circ>z1)))) = 0" by auto
+have subresult28:" (snd (wall_count (((x1)\<circ>(basic (w4\<otimes>(cement cup)\<otimes>(cement vert)))\<circ>(basic (y1\<otimes>(cement cap)))\<circ>z1))))
 = snd (wall_count z1)" 
 using wall_count_def compose_Cons
  by (metis snd_conv wall_count_compose)
 from subresult24  and subresult25 and subresult28 and subresult21 have subresult29:
-" abs (snd (wall_count (((x1)\<circ>(basic (w4\<otimes>e_cup\<otimes>e_vert))\<circ>(basic (y1\<otimes>e_cap))\<circ>z1))))= 0" by auto
+" abs (snd (wall_count (((x1)\<circ>(basic (w4\<otimes>(cement cup)\<otimes>(cement vert)))\<circ>(basic (y1\<otimes>(cement cap)))\<circ>z1))))= 0" by auto
 from subresult27 and subresult29 and subresult21 have subresult30: "well_defined  
-(((x1)\<circ>(basic (w4\<otimes>e_cup\<otimes>e_vert))\<circ>(basic (y1\<otimes>e_cap))\<circ>z1))" 
+(((x1)\<circ>(basic (w4\<otimes>(cement cup)\<otimes>(cement vert)))\<circ>(basic (y1\<otimes>(cement cap)))\<circ>z1))" 
 using monoid_add_class.add.left_neutral well_defined_def
 by (auto)
 from this and assms and subresult3 and metaequivalence_bottomleft and subresult30
 have "tanglerel_equiv 
-      (Abs_diagram ((?x2)\<circ>(basic (e_vert\<otimes>e_cup\<otimes> w5))\<circ>(basic (e_cap\<otimes>?y2))\<circ>z1))
+      (Abs_diagram ((?x2)\<circ>(basic ((cement vert)\<otimes>(cement cup)\<otimes> w5))\<circ>(basic ((cement cap)\<otimes>?y2))\<circ>z1))
                (Abs_diagram ((?x2)\<circ>(basic (?y2))\<circ>z1))"
 using compose_leftassociativity subresult11
 by (metis)
 from this have "tanglerel_equiv
- (Abs_diagram ((x1)\<circ>(basic (w4\<otimes>e_cup\<otimes>e_vert))\<circ>(basic (e_vert\<otimes>e_cup\<otimes> w5))\<circ>(basic (e_cap\<otimes>y1\<otimes>e_cap))\<circ>z1))  
-       (Abs_diagram ((x1)\<circ>(basic (w4\<otimes>e_cup\<otimes>e_vert))\<circ>(basic (y1\<otimes>e_cap))\<circ>z1))" 
+ (Abs_diagram ((x1)\<circ>(basic (w4\<otimes>(cement cup)\<otimes>(cement vert)))\<circ>(basic ((cement vert)\<otimes>(cement cup)\<otimes> w5))\<circ>(basic ((cement cap)\<otimes>y1\<otimes>(cement cap)))\<circ>z1))  
+       (Abs_diagram ((x1)\<circ>(basic (w4\<otimes>(cement cup)\<otimes>(cement vert)))\<circ>(basic (y1\<otimes>(cement cap)))\<circ>z1))" 
 using compose_leftassociativity by auto
  
 
 from this and subresult1 have "tanglerel_equiv 
- (Abs_diagram ((x1)\<circ>(basic (w4\<otimes>e_cup\<otimes>e_vert))\<circ>(basic (e_vert\<otimes>e_cup\<otimes> w5))\<circ>(basic (e_cap\<otimes>y1\<otimes>e_cap))\<circ>z1))   
+ (Abs_diagram ((x1)\<circ>(basic (w4\<otimes>(cement cup)\<otimes>(cement vert)))\<circ>(basic ((cement vert)\<otimes>(cement cup)\<otimes> w5))\<circ>(basic ((cement cap)\<otimes>y1\<otimes>(cement cap)))\<circ>z1))   
           (Abs_diagram (x1 \<circ> (basic y1)\<circ> z1))" using rtranclp_trans Tangle.abs_eq_iff 
 by metis
 then show ?thesis by simp
@@ -3039,23 +3044,23 @@ theorem metaequivalence_positive_cross: assumes "(fst (count y1))>1" and "(snd (
 and "w4 = makestrand  (nat ((fst (count y1)) + (-2)))" 
 and "w5 = makestrand (nat ((snd (count y2)) + (-2)))"
 and "well_defined (x1 \<circ> basic y1 \<circ> basic y2 \<circ>z1)" 
-shows "tanglerel_equiv (Abs_diagram ((x1)\<circ>  (basic (e_vert\<otimes>e_cup\<otimes>w4)) \<circ>
-(basic (e_cap\<otimes>y1))\<circ>(basic (y2\<otimes>e_cup))\<circ>(basic (w5\<otimes>e_cap\<otimes>e_vert))\<circ>z1))
+shows "tanglerel_equiv (Abs_diagram ((x1)\<circ>  (basic ((cement vert)\<otimes>(cement cup)\<otimes>w4)) \<circ>
+(basic ((cement cap)\<otimes>y1))\<circ>(basic (y2\<otimes>(cement cup)))\<circ>(basic (w5\<otimes>(cement cap)\<otimes>(cement vert)))\<circ>z1))
              (Abs_diagram (x1 \<circ> (basic y1)\<circ> (basic y2)\<circ>z1))" 
 proof-
-have subresult: "tanglerel_equiv (Abs_diagram ((x1)\<circ>  (basic (e_vert\<otimes>e_cup\<otimes>w4)) \<circ>
-(basic (e_cap\<otimes>y1))\<circ>(basic y2)\<circ>z1))
+have subresult: "tanglerel_equiv (Abs_diagram ((x1)\<circ>  (basic ((cement vert)\<otimes>(cement cup)\<otimes>w4)) \<circ>
+(basic ((cement cap)\<otimes>y1))\<circ>(basic y2)\<circ>z1))
              (Abs_diagram (x1 \<circ> (basic y1)\<circ> (basic y2)\<circ>z1))" using assms metaequivalence_bottomleft
 by auto
-let ?x2 = "(x1)\<circ>(basic (e_vert\<otimes>e_cup\<otimes>w4)) \<circ>(basic (e_cap\<otimes>y1))"
-have "tanglerel_equiv (Abs_diagram (?x2\<circ>(basic (y2\<otimes>e_cup))\<circ>(basic (w5\<otimes>e_cap\<otimes>e_vert))\<circ>z1))
+let ?x2 = "(x1)\<circ>(basic ((cement vert)\<otimes>(cement cup)\<otimes>w4)) \<circ>(basic ((cement cap)\<otimes>y1))"
+have "tanglerel_equiv (Abs_diagram (?x2\<circ>(basic (y2\<otimes>(cement cup)))\<circ>(basic (w5\<otimes>(cement cap)\<otimes>(cement vert)))\<circ>z1))
            (Abs_diagram (?x2\<circ>(basic y2)\<circ>z1))" using assms metaequivalence_right by (metis (full_types))
-from this have "tanglerel_equiv (Abs_diagram ((x1)\<circ>(basic (e_vert\<otimes>e_cup\<otimes>w4)) \<circ>(basic (e_cap\<otimes>y1))
-\<circ>(basic (y2\<otimes>e_cup))\<circ>(basic (w5\<otimes>e_cap\<otimes>e_vert))\<circ>z1))
-           (Abs_diagram ((x1)\<circ>(basic (e_vert\<otimes>e_cup\<otimes>w4)) \<circ>(basic (e_cap\<otimes>y1))\<circ>(basic y2)\<circ>z1))"
+from this have "tanglerel_equiv (Abs_diagram ((x1)\<circ>(basic ((cement vert)\<otimes>(cement cup)\<otimes>w4)) \<circ>(basic ((cement cap)\<otimes>y1))
+\<circ>(basic (y2\<otimes>(cement cup)))\<circ>(basic (w5\<otimes>(cement cap)\<otimes>(cement vert)))\<circ>z1))
+           (Abs_diagram ((x1)\<circ>(basic ((cement vert)\<otimes>(cement cup)\<otimes>w4)) \<circ>(basic ((cement cap)\<otimes>y1))\<circ>(basic y2)\<circ>z1))"
 using compose_leftassociativity by (auto)
-from this and subresult have " tanglerel_equiv  (Abs_diagram ((x1)\<circ>(basic (e_vert\<otimes>e_cup\<otimes>w4)) \<circ>(basic (e_cap\<otimes>y1))
-\<circ>(basic (y2\<otimes>e_cup))\<circ>(basic (w5\<otimes>e_cap\<otimes>e_vert))\<circ>z1))
+from this and subresult have " tanglerel_equiv  (Abs_diagram ((x1)\<circ>(basic ((cement vert)\<otimes>(cement cup)\<otimes>w4)) \<circ>(basic ((cement cap)\<otimes>y1))
+\<circ>(basic (y2\<otimes>(cement cup)))\<circ>(basic (w5\<otimes>(cement cap)\<otimes>(cement vert)))\<circ>z1))
              (Abs_diagram (x1 \<circ> (basic y1)\<circ> (basic y2)\<circ>z1))"
 using rtranclp_trans Tangle.abs_eq_iff by metis
 from this show ?thesis by simp
@@ -3065,28 +3070,23 @@ theorem metaequivalence_negative_cross: assumes "(fst (count y1))>1" and "(snd (
 and "w4 = makestrand  (nat ((fst (count y1)) + (-2)))" 
 and "w5 = makestrand (nat ((snd (count y2)) + (-2)))"
 and "well_defined (x1 \<circ> basic y1 \<circ> basic y2 \<circ>z1)" 
-shows "tanglerel_equiv (Abs_diagram ((x1)\<circ>  (basic (w4\<otimes>e_cup\<otimes>e_vert)) \<circ>
-(basic (y1 \<otimes>e_cap))\<circ>(basic (e_cup\<otimes>y2))\<circ>(basic (e_vert\<otimes>e_cap\<otimes>w5))\<circ>z1))
+shows "tanglerel_equiv (Abs_diagram ((x1)\<circ>  (basic (w4\<otimes>(cement cup)\<otimes>(cement vert))) \<circ>
+(basic (y1 \<otimes>(cement cap)))\<circ>(basic ((cement cup)\<otimes>y2))\<circ>(basic ((cement vert)\<otimes>(cement cap)\<otimes>w5))\<circ>z1))
              (Abs_diagram (x1 \<circ> (basic y1)\<circ> (basic y2)\<circ>z1))" 
 proof-
-have subresult: "tanglerel_equiv (Abs_diagram ((x1)\<circ>  (basic (w4\<otimes>e_cup\<otimes>e_vert)) \<circ>
-(basic (y1\<otimes>e_cap))\<circ>(basic y2)\<circ>z1))
+have subresult: "tanglerel_equiv (Abs_diagram ((x1)\<circ>  (basic (w4\<otimes>(cement cup)\<otimes>(cement vert))) \<circ>
+(basic (y1\<otimes>(cement cap)))\<circ>(basic y2)\<circ>z1))
              (Abs_diagram (x1 \<circ> (basic y1)\<circ> (basic y2)\<circ>z1))" using assms metaequivalence_bottomright
 by auto
-let ?x2 = "(x1)\<circ>(basic (w4\<otimes>e_cup\<otimes>e_vert)) \<circ>(basic (y1 \<otimes>e_cap))"
-have "tanglerel_equiv (Abs_diagram (?x2\<circ>(basic (e_cup\<otimes>y2))\<circ>(basic (e_vert\<otimes>e_cap\<otimes>w5))\<circ>z1))
+let ?x2 = "(x1)\<circ>(basic (w4\<otimes>(cement cup)\<otimes>(cement vert))) \<circ>(basic (y1 \<otimes>(cement cap)))"
+have "tanglerel_equiv (Abs_diagram (?x2\<circ>(basic ((cement cup)\<otimes>y2))\<circ>(basic ((cement vert)\<otimes>(cement cap)\<otimes>w5))\<circ>z1))
            (Abs_diagram (?x2\<circ>(basic y2)\<circ>z1))" using assms metaequivalence_left by (metis (full_types))
-from this have  "tanglerel_equiv (Abs_diagram ((x1)\<circ>(basic (w4\<otimes>e_cup\<otimes>e_vert)) \<circ>(basic (y1 \<otimes>e_cap))
-\<circ>(basic (e_cup\<otimes>y2))\<circ>(basic (e_vert\<otimes>e_cap\<otimes>w5))\<circ>z1))
-           (Abs_diagram ((x1)\<circ>(basic (w4\<otimes>e_cup\<otimes>e_vert)) \<circ>(basic (y1 \<otimes>e_cap))\<circ>(basic y2)\<circ>z1))"
+from this have  "tanglerel_equiv (Abs_diagram ((x1)\<circ>(basic (w4\<otimes>(cement cup)\<otimes>(cement vert))) \<circ>(basic (y1 \<otimes>(cement cap)))
+\<circ>(basic ((cement cup)\<otimes>y2))\<circ>(basic ((cement vert)\<otimes>(cement cap)\<otimes>w5))\<circ>z1))
+           (Abs_diagram ((x1)\<circ>(basic (w4\<otimes>(cement cup)\<otimes>(cement vert))) \<circ>(basic (y1 \<otimes>(cement cap)))\<circ>(basic y2)\<circ>z1))"
 using compose_leftassociativity by auto
-from subresult and this have                              
-
-
-
-
-" tanglerel_equiv (Abs_diagram ((x1)\<circ>(basic (w4\<otimes>e_cup\<otimes>e_vert)) \<circ>(basic (y1 \<otimes>e_cap))
-\<circ>(basic (e_cup\<otimes>y2))\<circ>(basic (e_vert\<otimes>e_cap\<otimes>w5))\<circ>z1))
+from subresult and this have " tanglerel_equiv (Abs_diagram ((x1)\<circ>(basic (w4\<otimes>(cement cup)\<otimes>(cement vert))) \<circ>(basic (y1 \<otimes>(cement cap)))
+\<circ>(basic ((cement cup)\<otimes>y2))\<circ>(basic ((cement vert)\<otimes>(cement cap)\<otimes>w5))\<circ>z1))
            (Abs_diagram ((x1)\<circ>(basic y1)\<circ>(basic y2)\<circ>z1))"
 using Tangle.abs_eq_iff by (metis)
 from this show ?thesis by simp
@@ -3099,152 +3099,154 @@ and "w4 = makestrand  (nat ((snd (count y3)) + (-2)))"
 and "w5 = makestrand (nat ((snd (count y3))))"
 and "fst (count y2) = snd (count y1)"
 and "(fst (count y3)) = (snd (count y2))"
-shows "tanglerel_equiv (Abs_diagram ((x1)\<circ>(basic (e_cup\<otimes>y1\<otimes>e_cup))\<circ>(basic (e_vert\<otimes>e_vert\<otimes>y2\<otimes>e_vert\<otimes>e_vert))\<circ>
-(basic (e_vert\<otimes>e_vert\<otimes>y3\<otimes>e_vert\<otimes>e_vert))\<circ>(basic (e_vert\<otimes>e_cap\<otimes> w5)) \<circ> (basic (w4\<otimes>e_cap\<otimes>e_vert))\<circ>z1))
+shows "tanglerel_equiv (Abs_diagram ((x1)\<circ>(basic ((cement cup)\<otimes>y1\<otimes>(cement cup)))\<circ>(basic ((cement vert)\<otimes>(cement vert)\<otimes>y2\<otimes>(cement vert)\<otimes>(cement vert)))\<circ>
+(basic ((cement vert)\<otimes>(cement vert)\<otimes>y3\<otimes>(cement vert)\<otimes>(cement vert)))\<circ>(basic ((cement vert)\<otimes>(cement cap)\<otimes> w5)) \<circ> (basic (w4\<otimes>(cement cap)\<otimes>(cement vert)))\<circ>z1))
              (Abs_diagram (x1 \<circ> (basic y1)\<circ>(basic y2)\<circ>(basic y3)\<circ>z1))" 
 proof-
 let ?x2 = "x1\<circ> (basic y1)"
-have  "tanglerel_equiv (Abs_diagram (?x2\<circ>(basic (e_cup\<otimes>y2\<otimes>e_cup))\<circ>
-(basic (e_vert\<otimes>e_vert\<otimes>y3\<otimes>e_vert\<otimes>e_vert))\<circ>(basic (e_vert\<otimes>e_cap\<otimes> w5)) \<circ> (basic (w4\<otimes>e_cap\<otimes>e_vert))\<circ>z1))
+have  "tanglerel_equiv (Abs_diagram (?x2\<circ>(basic ((cement cup)\<otimes>y2\<otimes>(cement cup)))\<circ>
+(basic ((cement vert)\<otimes>(cement vert)\<otimes>y3\<otimes>(cement vert)\<otimes>(cement vert)))\<circ>(basic ((cement vert)\<otimes>(cement cap)\<otimes> w5)) \<circ> (basic (w4\<otimes>(cement cap)\<otimes>(cement vert)))\<circ>z1))
              (Abs_diagram (?x2\<circ>(basic y2)\<circ>(basic y3)\<circ>z1))" 
 using metaequivalence_both_doubledrop assms by auto
 from this have subresult1:
-"tanglerel_equiv (Abs_diagram (x1\<circ> (basic y1)\<circ>(basic (e_cup\<otimes>y2\<otimes>e_cup))\<circ>
-(basic (e_vert\<otimes>e_vert\<otimes>y3\<otimes>e_vert\<otimes>e_vert))\<circ>(basic (e_vert\<otimes>e_cap\<otimes> w5)) \<circ> (basic (w4\<otimes>e_cap\<otimes>e_vert))\<circ>z1))
+"tanglerel_equiv (Abs_diagram (x1\<circ> (basic y1)\<circ>(basic ((cement cup)\<otimes>y2\<otimes>(cement cup)))\<circ>
+(basic ((cement vert)\<otimes>(cement vert)\<otimes>y3\<otimes>(cement vert)\<otimes>(cement vert)))\<circ>(basic ((cement vert)\<otimes>(cement cap)\<otimes> w5)) \<circ> (basic (w4\<otimes>(cement cap)\<otimes>(cement vert)))\<circ>z1))
              (Abs_diagram (x1\<circ> (basic y1)\<circ>(basic y2)\<circ>(basic y3)\<circ>z1))" using compose_leftassociativity 
 by simp
-have subresult2: "fst (count e_cup) = 0" using e_cup_def 
+have subresult2: "fst (count (cement cup)) = 0" using 
 count_def add_left_cancel comm_monoid_add_class.add.right_neutral fst_count_additive fstcount_cup_rightcompose
 by (auto)
-let ?z2 = "(basic (e_vert\<otimes>e_vert\<otimes>y3\<otimes>e_vert\<otimes>e_vert))\<circ>(basic (e_vert\<otimes>e_cap\<otimes> w5)) 
-\<circ> (basic (w4\<otimes>e_cap\<otimes>e_vert))\<circ>z1"
-let ?w2 = "y2 \<otimes> e_cup"
+let ?z2 = "(basic ((cement vert)\<otimes>(cement vert)\<otimes>y3\<otimes>(cement vert)\<otimes>(cement vert)))\<circ>(basic ((cement vert)\<otimes>(cement cap)\<otimes> w5)) 
+\<circ> (basic (w4\<otimes>(cement cap)\<otimes>(cement vert)))\<circ>z1"
+let ?w2 = "y2 \<otimes> (cement cup)"
 have "fst (count ?w2) = fst (count y2)" using fstcount_cup_rightcompose by auto
 from this and assms have subresult3:"fst (count ?w2) = snd (count y1)" by auto
 
-let ?B = "e_vert \<otimes> e_vert"
+let ?B = "(cement vert) \<otimes> (cement vert)"
 have subresult4: "strands ?B"
-using Tangles.append.append_Nil e_vert_def makestrand.simps(1) strand_makestrand strands.simps(2)
+using Tangles.append.append_Nil  makestrand.simps(1) strand_makestrand strands.simps(2)
  by (metis)
 from subresult4 and subresult2 and subresult3 and exI have 
-"(strands ?B) \<and> (fst (count ?w2) = snd (count y1)) \<and> (fst (count e_cup) = 0)"
+"(strands ?B) \<and> (fst (count ?w2) = snd (count y1)) \<and> (fst (count (cement cup)) = 0)"
 by auto
 from this and exI and tanglerel_compbelow_centerright_def have 
 "tanglerel_compbelow_centerright 
-(Abs_diagram (x1 \<circ> (basic (e_cup \<otimes> y1)) \<circ> (basic (?B\<otimes> ?w2)) \<circ> ?z2))
-(Abs_diagram (x1 \<circ> (basic ( y1)) \<circ> (basic (e_cup \<otimes> ?w2)) \<circ> ?z2))"
+(Abs_diagram (x1 \<circ> (basic ((cement cup) \<otimes> y1)) \<circ> (basic (?B\<otimes> ?w2)) \<circ> ?z2))
+(Abs_diagram (x1 \<circ> (basic ( y1)) \<circ> (basic ((cement cup) \<otimes> ?w2)) \<circ> ?z2))"
 by metis
 from this and compose_leftassociativity and leftright_associativity have 
 "tanglerel_compbelow_centerright 
- (Abs_diagram ((x1)\<circ>(basic (e_cup\<otimes>y1))\<circ>(basic (e_vert\<otimes>e_vert\<otimes>y2\<otimes>e_cup))\<circ>
-(basic (e_vert\<otimes>e_vert\<otimes>y3\<otimes>e_vert\<otimes>e_vert))\<circ>(basic (e_vert\<otimes>e_cap\<otimes> w5)) \<circ> (basic (w4\<otimes>e_cap\<otimes>e_vert))
+ (Abs_diagram ((x1)\<circ>(basic ((cement cup)\<otimes>y1))\<circ>(basic ((cement vert)\<otimes>(cement vert)\<otimes>y2\<otimes>(cement cup)))\<circ>
+(basic ((cement vert)\<otimes>(cement vert)\<otimes>y3\<otimes>(cement vert)\<otimes>(cement vert)))\<circ>(basic ((cement vert)\<otimes>(cement cap)\<otimes> w5)) \<circ> (basic (w4\<otimes>(cement cap)\<otimes>(cement vert)))
 \<circ>z1))
- (Abs_diagram (x1\<circ>(basic y1)\<circ>(basic (e_cup\<otimes>y2\<otimes>e_cup))\<circ>
-(basic (e_vert\<otimes>e_vert\<otimes>y3\<otimes>e_vert\<otimes>e_vert))\<circ>(basic (e_vert\<otimes>e_cap\<otimes> w5)) \<circ> (basic (w4\<otimes>e_cap\<otimes>e_vert))\<circ>z1))"
+ (Abs_diagram (x1\<circ>(basic y1)\<circ>(basic ((cement cup)\<otimes>y2\<otimes>(cement cup)))\<circ>
+(basic ((cement vert)\<otimes>(cement vert)\<otimes>y3\<otimes>(cement vert)\<otimes>(cement vert)))\<circ>(basic ((cement vert)\<otimes>(cement cap)\<otimes> w5)) \<circ> (basic (w4\<otimes>(cement cap)\<otimes>(cement vert)))\<circ>z1))"
 by auto
 from this have
 "tanglerel_compbelow 
- (Abs_diagram ((x1)\<circ>(basic (e_cup\<otimes>y1))\<circ>(basic (e_vert\<otimes>e_vert\<otimes>y2\<otimes>e_cup))\<circ>
-(basic (e_vert\<otimes>e_vert\<otimes>y3\<otimes>e_vert\<otimes>e_vert))\<circ>(basic (e_vert\<otimes>e_cap\<otimes> w5)) \<circ> (basic (w4\<otimes>e_cap\<otimes>e_vert))
+ (Abs_diagram ((x1)\<circ>(basic ((cement cup)\<otimes>y1))\<circ>(basic ((cement vert)\<otimes>(cement vert)\<otimes>y2\<otimes>(cement cup)))\<circ>
+(basic ((cement vert)\<otimes>(cement vert)\<otimes>y3\<otimes>(cement vert)\<otimes>(cement vert)))\<circ>(basic ((cement vert)\<otimes>(cement cap)\<otimes> w5)) \<circ> (basic (w4\<otimes>(cement cap)\<otimes>(cement vert)))
 \<circ>z1))
- (Abs_diagram (x1\<circ>(basic y1)\<circ>(basic (e_cup\<otimes>y2\<otimes>e_cup))\<circ>
-(basic (e_vert\<otimes>e_vert\<otimes>y3\<otimes>e_vert\<otimes>e_vert))\<circ>(basic (e_vert\<otimes>e_cap\<otimes> w5)) \<circ> (basic (w4\<otimes>e_cap\<otimes>e_vert))\<circ>z1))"
+ (Abs_diagram (x1\<circ>(basic y1)\<circ>(basic ((cement cup)\<otimes>y2\<otimes>(cement cup)))\<circ>
+(basic ((cement vert)\<otimes>(cement vert)\<otimes>y3\<otimes>(cement vert)\<otimes>(cement vert)))\<circ>(basic ((cement vert)\<otimes>(cement cap)\<otimes> w5)) \<circ> (basic (w4\<otimes>(cement cap)\<otimes>(cement vert)))\<circ>z1))"
 using tanglerel_compbelow_def by auto
 from this have 
 "tanglerel_compress
- (Abs_diagram ((x1)\<circ>(basic (e_cup\<otimes>y1))\<circ>(basic (e_vert\<otimes>e_vert\<otimes>y2\<otimes>e_cup))\<circ>
-(basic (e_vert\<otimes>e_vert\<otimes>y3\<otimes>e_vert\<otimes>e_vert))\<circ>(basic (e_vert\<otimes>e_cap\<otimes> w5)) \<circ> (basic (w4\<otimes>e_cap\<otimes>e_vert))
+ (Abs_diagram ((x1)\<circ>(basic ((cement cup)\<otimes>y1))\<circ>(basic ((cement vert)\<otimes>(cement vert)\<otimes>y2\<otimes>(cement cup)))\<circ>
+(basic ((cement vert)\<otimes>(cement vert)\<otimes>y3\<otimes>(cement vert)\<otimes>(cement vert)))\<circ>(basic ((cement vert)\<otimes>(cement cap)\<otimes> w5)) \<circ> (basic (w4\<otimes>(cement cap)\<otimes>(cement vert)))
 \<circ>z1))
- (Abs_diagram (x1\<circ>(basic y1)\<circ>(basic (e_cup\<otimes>y2\<otimes>e_cup))\<circ>
-(basic (e_vert\<otimes>e_vert\<otimes>y3\<otimes>e_vert\<otimes>e_vert))\<circ>(basic (e_vert\<otimes>e_cap\<otimes> w5)) \<circ> (basic (w4\<otimes>e_cap\<otimes>e_vert))\<circ>z1))"
+ (Abs_diagram (x1\<circ>(basic y1)\<circ>(basic ((cement cup)\<otimes>y2\<otimes>(cement cup)))\<circ>
+(basic ((cement vert)\<otimes>(cement vert)\<otimes>y3\<otimes>(cement vert)\<otimes>(cement vert)))\<circ>(basic ((cement vert)\<otimes>(cement cap)\<otimes> w5)) \<circ> (basic (w4\<otimes>(cement cap)\<otimes>(cement vert)))\<circ>z1))"
 using tanglerel_compress_def by auto
 from this have
 "tanglerel
-(Abs_diagram ((x1)\<circ>(basic (e_cup\<otimes>y1))\<circ>(basic (e_vert\<otimes>e_vert\<otimes>y2\<otimes>e_cup))\<circ>
-(basic (e_vert\<otimes>e_vert\<otimes>y3\<otimes>e_vert\<otimes>e_vert))\<circ>(basic (e_vert\<otimes>e_cap\<otimes> w5)) \<circ> (basic (w4\<otimes>e_cap\<otimes>e_vert))
+(Abs_diagram ((x1)\<circ>(basic ((cement cup)\<otimes>y1))\<circ>(basic ((cement vert)\<otimes>(cement vert)\<otimes>y2\<otimes>(cement cup)))\<circ>
+(basic ((cement vert)\<otimes>(cement vert)\<otimes>y3\<otimes>(cement vert)\<otimes>(cement vert)))\<circ>(basic ((cement vert)\<otimes>(cement cap)\<otimes> w5)) \<circ> (basic (w4\<otimes>(cement cap)\<otimes>(cement vert)))
 \<circ>z1))
- (Abs_diagram (x1\<circ>(basic y1)\<circ>(basic (e_cup\<otimes>y2\<otimes>e_cup))\<circ>
-(basic (e_vert\<otimes>e_vert\<otimes>y3\<otimes>e_vert\<otimes>e_vert))\<circ>(basic (e_vert\<otimes>e_cap\<otimes> w5)) \<circ> (basic (w4\<otimes>e_cap\<otimes>e_vert))\<circ>z1))"
+ (Abs_diagram (x1\<circ>(basic y1)\<circ>(basic ((cement cup)\<otimes>y2\<otimes>(cement cup)))\<circ>
+(basic ((cement vert)\<otimes>(cement vert)\<otimes>y3\<otimes>(cement vert)\<otimes>(cement vert)))\<circ>(basic ((cement vert)\<otimes>(cement cap)\<otimes> w5)) \<circ> (basic (w4\<otimes>(cement cap)\<otimes>(cement vert)))\<circ>z1))"
 using tanglerel_def by auto
 from this have 
 "tanglerel_equiv
-(Abs_diagram ((x1)\<circ>(basic (e_cup\<otimes>y1))\<circ>(basic (e_vert\<otimes>e_vert\<otimes>y2\<otimes>e_cup))\<circ>
-(basic (e_vert\<otimes>e_vert\<otimes>y3\<otimes>e_vert\<otimes>e_vert))\<circ>(basic (e_vert\<otimes>e_cap\<otimes> w5)) \<circ> (basic (w4\<otimes>e_cap\<otimes>e_vert))
+(Abs_diagram ((x1)\<circ>(basic ((cement cup)\<otimes>y1))\<circ>(basic ((cement vert)\<otimes>(cement vert)\<otimes>y2\<otimes>(cement cup)))\<circ>
+(basic ((cement vert)\<otimes>(cement vert)\<otimes>y3\<otimes>(cement vert)\<otimes>(cement vert)))\<circ>(basic ((cement vert)\<otimes>(cement cap)\<otimes> w5)) \<circ> (basic (w4\<otimes>(cement cap)\<otimes>(cement vert)))
 \<circ>z1))
- (Abs_diagram (x1\<circ>(basic y1)\<circ>(basic (e_cup\<otimes>y2\<otimes>e_cup))\<circ>
-(basic (e_vert\<otimes>e_vert\<otimes>y3\<otimes>e_vert\<otimes>e_vert))\<circ>(basic (e_vert\<otimes>e_cap\<otimes> w5)) \<circ> (basic (w4\<otimes>e_cap\<otimes>e_vert))\<circ>z1))"
+ (Abs_diagram (x1\<circ>(basic y1)\<circ>(basic ((cement cup)\<otimes>y2\<otimes>(cement cup)))\<circ>
+(basic ((cement vert)\<otimes>(cement vert)\<otimes>y3\<otimes>(cement vert)\<otimes>(cement vert)))\<circ>(basic ((cement vert)\<otimes>(cement cap)\<otimes> w5)) \<circ> (basic (w4\<otimes>(cement cap)\<otimes>(cement vert)))\<circ>z1))"
 using tanglerel_equiv_def r_into_rtranclp by metis
 from this and subresult1 and r_into_rtranclp rtranclp_trans have subresult5:
 "tanglerel_equiv
-(Abs_diagram ((x1)\<circ>(basic (e_cup\<otimes>y1))\<circ>(basic (e_vert\<otimes>e_vert\<otimes>y2\<otimes>e_cup))\<circ>
-(basic (e_vert\<otimes>e_vert\<otimes>y3\<otimes>e_vert\<otimes>e_vert))\<circ>(basic (e_vert\<otimes>e_cap\<otimes> w5)) \<circ> (basic (w4\<otimes>e_cap\<otimes>e_vert))
+(Abs_diagram ((x1)\<circ>(basic ((cement cup)\<otimes>y1))\<circ>(basic ((cement vert)\<otimes>(cement vert)\<otimes>y2\<otimes>(cement cup)))\<circ>
+(basic ((cement vert)\<otimes>(cement vert)\<otimes>y3\<otimes>(cement vert)\<otimes>(cement vert)))\<circ>(basic ((cement vert)\<otimes>(cement cap)\<otimes> w5)) \<circ> (basic (w4\<otimes>(cement cap)\<otimes>(cement vert)))
 \<circ>z1))
 (Abs_diagram (x1\<circ>(basic y1)\<circ>(basic y2)\<circ>(basic y3)\<circ>z1))"
 by (metis Tangle.abs_eq_iff compose_Nil)
 
-have "snd (count (e_cup \<otimes> y1)) = 2 + snd (count y1)" using snd_count_additive 
+have "snd (count ((cement cup) \<otimes> y1)) = 2 + snd (count y1)" using snd_count_additive 
 comm_semiring_1_class.normalizing_semiring_rules(24) count_cup_rightcompose snd_conv 
 snd_count_additive by metis
-from this and assms have subresult6: "snd (count (e_cup \<otimes> y1)) = 2 + fst (count y2)" by auto
+from this and assms have subresult6: "snd (count ((cement cup) \<otimes> y1)) = 2 + fst (count y2)" by auto
 
-let ?subs1 = "(e_cup \<otimes> y1)"
-let ?subs2 = " (e_vert \<otimes> e_vert \<otimes> y2)"
-have " fst (count (e_vert \<otimes> e_vert \<otimes> y2)) = 2 + fst (count y2)"
-using fst_count_additive e_vert_count by auto 
+let ?subs1 = "((cement cup) \<otimes> y1)"
+let ?subs2 = " ((cement vert) \<otimes> (cement vert) \<otimes> y2)"
+have " fst (count ((cement vert) \<otimes> (cement vert) \<otimes> y2)) = 2 + fst (count y2)"
+using fst_count_additive  by auto 
 from this and subresult6 have "snd (count (?subs1)) = 
 fst (count (?subs2))" by auto
 from this and subresult2 and subresult4 have
-"(strands ?B) \<and> (fst (count ?subs2) = snd (count ?subs1)) \<and> (fst (count e_cup) = 0)" by auto
+"(strands ?B) \<and> (fst (count ?subs2) = snd (count ?subs1)) \<and> (fst (count (cement cup)) = 0)" by auto
 
 from this  exI and tanglerel_compbelow_centerleft_def  
 have "tanglerel_compbelow_centerleft
- (Abs_diagram ((x1)\<circ>(basic (?subs1 \<otimes> e_cup))\<circ>(basic (?subs2\<otimes>?B))\<circ>
+ (Abs_diagram ((x1)\<circ>(basic (?subs1 \<otimes> (cement cup)))\<circ>(basic (?subs2\<otimes>?B))\<circ>
 ?z2))
- (Abs_diagram ((x1)\<circ>(basic (?subs1))\<circ>(basic (?subs2\<otimes>e_cup))\<circ>
+ (Abs_diagram ((x1)\<circ>(basic (?subs1))\<circ>(basic (?subs2\<otimes>(cement cup)))\<circ>
 ?z2))" by metis
 from this and leftright_associativity have
 "tanglerel_compbelow_centerleft
- (Abs_diagram ((x1)\<circ>(basic (e_cup\<otimes>y1 \<otimes> e_cup))\<circ>(basic (e_vert\<otimes>e_vert \<otimes> y2 \<otimes> e_vert \<otimes> e_vert))\<circ>
-(basic (e_vert\<otimes>e_vert\<otimes>y3\<otimes>e_vert\<otimes>e_vert))\<circ>(basic (e_vert\<otimes>e_cap\<otimes> w5)) 
-\<circ> (basic (w4\<otimes>e_cap\<otimes>e_vert))\<circ>z1))
- (Abs_diagram ((x1)\<circ>(basic (e_cup\<otimes>y1))\<circ>(basic (e_vert\<otimes>e_vert\<otimes>y2\<otimes>e_cup))\<circ>
-(basic (e_vert\<otimes>e_vert\<otimes>y3\<otimes>e_vert\<otimes>e_vert))\<circ>(basic (e_vert\<otimes>e_cap\<otimes> w5)) 
-\<circ> (basic (w4\<otimes>e_cap\<otimes>e_vert))\<circ>z1))"
+ (Abs_diagram ((x1)\<circ>(basic ((cement cup)\<otimes>y1 \<otimes> (cement cup)))\<circ>(basic ((cement vert)\<otimes>(cement vert) \<otimes> y2 \<otimes> (cement vert) \<otimes> (cement vert)))\<circ>
+(basic ((cement vert)\<otimes>(cement vert)\<otimes>y3\<otimes>(cement vert)\<otimes>(cement vert)))\<circ>(basic ((cement vert)\<otimes>(cement cap)\<otimes> w5)) 
+\<circ> (basic (w4\<otimes>(cement cap)\<otimes>(cement vert)))\<circ>z1))
+ (Abs_diagram ((x1)\<circ>(basic ((cement cup)\<otimes>y1))\<circ>(basic ((cement vert)\<otimes>(cement vert)\<otimes>y2\<otimes>(cement cup)))\<circ>
+(basic ((cement vert)\<otimes>(cement vert)\<otimes>y3\<otimes>(cement vert)\<otimes>(cement vert)))\<circ>(basic ((cement vert)\<otimes>(cement cap)\<otimes> w5)) 
+\<circ> (basic (w4\<otimes>(cement cap)\<otimes>(cement vert)))\<circ>z1))"
 by auto
 
 from this and tanglerel_compbelow_def have
 "tanglerel_compbelow
- (Abs_diagram ((x1)\<circ>(basic (e_cup\<otimes>y1 \<otimes> e_cup))\<circ>(basic (e_vert\<otimes>e_vert \<otimes> y2 \<otimes> e_vert \<otimes> e_vert))\<circ>
-(basic (e_vert\<otimes>e_vert\<otimes>y3\<otimes>e_vert\<otimes>e_vert))\<circ>(basic (e_vert\<otimes>e_cap\<otimes> w5)) 
-\<circ> (basic (w4\<otimes>e_cap\<otimes>e_vert))\<circ>z1))
- (Abs_diagram ((x1)\<circ>(basic (e_cup\<otimes>y1))\<circ>(basic (e_vert\<otimes>e_vert\<otimes>y2\<otimes>e_cup))\<circ>
-(basic (e_vert\<otimes>e_vert\<otimes>y3\<otimes>e_vert\<otimes>e_vert))\<circ>(basic (e_vert\<otimes>e_cap\<otimes> w5)) 
-\<circ> (basic (w4\<otimes>e_cap\<otimes>e_vert))\<circ>z1))"
+ (Abs_diagram ((x1)\<circ>(basic ((cement cup)\<otimes>y1 \<otimes> (cement cup)))\<circ>(basic ((cement vert)\<otimes>(cement vert) \<otimes> y2 \<otimes> (cement vert) \<otimes> (cement vert)))\<circ>
+(basic ((cement vert)\<otimes>(cement vert)\<otimes>y3\<otimes>(cement vert)\<otimes>(cement vert)))\<circ>(basic ((cement vert)\<otimes>(cement cap)\<otimes> w5)) 
+\<circ> (basic (w4\<otimes>(cement cap)\<otimes>(cement vert)))\<circ>z1))
+ (Abs_diagram ((x1)\<circ>(basic ((cement cup)\<otimes>y1))\<circ>(basic ((cement vert)\<otimes>(cement vert)\<otimes>y2\<otimes>(cement cup)))\<circ>
+(basic ((cement vert)\<otimes>(cement vert)\<otimes>y3\<otimes>(cement vert)\<otimes>(cement vert)))\<circ>(basic ((cement vert)\<otimes>(cement cap)\<otimes> w5)) 
+\<circ> (basic (w4\<otimes>(cement cap)\<otimes>(cement vert)))\<circ>z1))"
 by auto
 
 from this and tanglerel_compress_def and tanglerel_def have
 "tanglerel
- (Abs_diagram ((x1)\<circ>(basic (e_cup\<otimes>y1 \<otimes> e_cup))\<circ>(basic (e_vert\<otimes>e_vert \<otimes> y2 \<otimes> e_vert \<otimes> e_vert))\<circ>
-(basic (e_vert\<otimes>e_vert\<otimes>y3\<otimes>e_vert\<otimes>e_vert))\<circ>(basic (e_vert\<otimes>e_cap\<otimes> w5)) 
-\<circ> (basic (w4\<otimes>e_cap\<otimes>e_vert))\<circ>z1))
- (Abs_diagram ((x1)\<circ>(basic (e_cup\<otimes>y1))\<circ>(basic (e_vert\<otimes>e_vert\<otimes>y2\<otimes>e_cup))\<circ>
-(basic (e_vert\<otimes>e_vert\<otimes>y3\<otimes>e_vert\<otimes>e_vert))\<circ>(basic (e_vert\<otimes>e_cap\<otimes> w5)) 
-\<circ> (basic (w4\<otimes>e_cap\<otimes>e_vert))\<circ>z1))"
+ (Abs_diagram ((x1)\<circ>(basic ((cement cup)\<otimes>y1 \<otimes> (cement cup)))\<circ>(basic ((cement vert)\<otimes>(cement vert) \<otimes> y2 \<otimes> (cement vert) \<otimes> (cement vert)))\<circ>
+(basic ((cement vert)\<otimes>(cement vert)\<otimes>y3\<otimes>(cement vert)\<otimes>(cement vert)))\<circ>(basic ((cement vert)\<otimes>(cement cap)\<otimes> w5)) 
+\<circ> (basic (w4\<otimes>(cement cap)\<otimes>(cement vert)))\<circ>z1))
+ (Abs_diagram ((x1)\<circ>(basic ((cement cup)\<otimes>y1))\<circ>(basic ((cement vert)\<otimes>(cement vert)\<otimes>y2\<otimes>(cement cup)))\<circ>
+(basic ((cement vert)\<otimes>(cement vert)\<otimes>y3\<otimes>(cement vert)\<otimes>(cement vert)))\<circ>(basic ((cement vert)\<otimes>(cement cap)\<otimes> w5)) 
+\<circ> (basic (w4\<otimes>(cement cap)\<otimes>(cement vert)))\<circ>z1))"
 by auto
 from this and  tanglerel_equiv_def and  r_into_rtranclp have
 "tanglerel_equiv
- (Abs_diagram ((x1)\<circ>(basic (e_cup\<otimes>y1 \<otimes> e_cup))\<circ>(basic (e_vert\<otimes>e_vert \<otimes> y2 \<otimes> e_vert \<otimes> e_vert))\<circ>
-(basic (e_vert\<otimes>e_vert\<otimes>y3\<otimes>e_vert\<otimes>e_vert))\<circ>(basic (e_vert\<otimes>e_cap\<otimes> w5)) 
-\<circ> (basic (w4\<otimes>e_cap\<otimes>e_vert))\<circ>z1))
- (Abs_diagram ((x1)\<circ>(basic (e_cup\<otimes>y1))\<circ>(basic (e_vert\<otimes>e_vert\<otimes>y2\<otimes>e_cup))\<circ>
-(basic (e_vert\<otimes>e_vert\<otimes>y3\<otimes>e_vert\<otimes>e_vert))\<circ>(basic (e_vert\<otimes>e_cap\<otimes> w5)) 
-\<circ> (basic (w4\<otimes>e_cap\<otimes>e_vert))\<circ>z1))" by metis
+ (Abs_diagram ((x1)\<circ>(basic ((cement cup)\<otimes>y1 \<otimes> (cement cup)))\<circ>(basic ((cement vert)\<otimes>(cement vert) \<otimes> y2 \<otimes> (cement vert) \<otimes> (cement vert)))\<circ>
+(basic ((cement vert)\<otimes>(cement vert)\<otimes>y3\<otimes>(cement vert)\<otimes>(cement vert)))\<circ>(basic ((cement vert)\<otimes>(cement cap)\<otimes> w5)) 
+\<circ> (basic (w4\<otimes>(cement cap)\<otimes>(cement vert)))\<circ>z1))
+ (Abs_diagram ((x1)\<circ>(basic ((cement cup)\<otimes>y1))\<circ>(basic ((cement vert)\<otimes>(cement vert)\<otimes>y2\<otimes>(cement cup)))\<circ>
+(basic ((cement vert)\<otimes>(cement vert)\<otimes>y3\<otimes>(cement vert)\<otimes>(cement vert)))\<circ>(basic ((cement vert)\<otimes>(cement cap)\<otimes> w5)) 
+\<circ> (basic (w4\<otimes>(cement cap)\<otimes>(cement vert)))\<circ>z1))" by metis
 from this and subresult5 and r_into_rtranclp rtranclp_trans have
  "tanglerel_equiv
- (Abs_diagram ((x1)\<circ>(basic (e_cup\<otimes>y1 \<otimes> e_cup))\<circ>(basic (e_vert\<otimes>e_vert \<otimes> y2 \<otimes> e_vert \<otimes> e_vert))\<circ>
-(basic (e_vert\<otimes>e_vert\<otimes>y3\<otimes>e_vert\<otimes>e_vert))\<circ>(basic (e_vert\<otimes>e_cap\<otimes> w5)) 
-\<circ> (basic (w4\<otimes>e_cap\<otimes>e_vert))\<circ>z1))
+ (Abs_diagram ((x1)\<circ>(basic ((cement cup)\<otimes>y1 \<otimes> (cement cup)))\<circ>(basic ((cement vert)\<otimes>(cement vert) \<otimes> y2 \<otimes> (cement vert) \<otimes> (cement vert)))\<circ>
+(basic ((cement vert)\<otimes>(cement vert)\<otimes>y3\<otimes>(cement vert)\<otimes>(cement vert)))\<circ>(basic ((cement vert)\<otimes>(cement cap)\<otimes> w5)) 
+\<circ> (basic (w4\<otimes>(cement cap)\<otimes>(cement vert)))\<circ>z1))
  (Abs_diagram ((x1)\<circ>(basic y1)\<circ>(basic y2)\<circ>(basic y3)\<circ>z1))"
 by (metis Tangle.abs_eq_iff compose_Nil)
 from this show ?thesis by auto
 qed
+
+end
